@prefix : <https://w3id.org/mobility/transmodel/commons#> .
@prefix owl: <http://www.w3.org/2002/07/owl#> .
@prefix rdf: <http://www.w3.org/1999/02/22-rdf-syntax-ns#> .
@prefix xml: <http://www.w3.org/XML/1998/namespace> .
@prefix xsd: <http://www.w3.org/2001/XMLSchema#> .
@prefix rdfs: <http://www.w3.org/2000/01/rdf-schema#> .
@base <https://w3id.org/mobility/transmodel/commons#> .

<https://w3id.org/mobility/transmodel/commons#> rdf:type owl:Ontology ;
                                                 owl:versionIRI <https://w3id.org/mobility/transmodel/commons/0.2.1> ;
                                                 <http://creativecommons.org/ns#license> <http://creativecommons.org/licenses/by/4.0/> ;
                                                 <http://purl.org/dc/elements/1.1/creator> "Jhon Toledo (Ontology Engienering Group - Universidad Politécnica de Madrid)" ,
                                                                                           "Miguel Angel García (Ontology Engienering Group - Universidad Politécnica de Madrid)" ,
                                                                                           "Oscar Corcho (Ontology Engineering Group - Universidad Politécnica de Madrid)" ;
                                                 <http://purl.org/dc/elements/1.1/date> "2022-03-10"@en ;
                                                 <http://purl.org/dc/elements/1.1/description> "Module of the Transmodel Ontology focused on commons. This ontology provides support to the NeTEx model. Visit https://github.com/oeg-upm/transmodel-ontology"@en ;
                                                 <http://purl.org/dc/elements/1.1/identifier> "https://w3id.org/mobility/transmodel/commons"@en ;
                                                 <http://purl.org/dc/elements/1.1/rights> "Creative Commons Attribution 4.0 International (CC BY 4.0)" ;
                                                 <http://purl.org/dc/elements/1.1/title> "Transmodel Ontology - Commons"@en ;
                                                 <http://purl.org/vocab/vann/preferredNamespaceUri> <https://w3id.org/mobility/transmodel/commons#> ;
                                                 rdfs:comment "Module of the Transmodel Ontology focused on commons. This ontology provides support to the NeTEx model. Visit https://github.com/oeg-upm/mobility"@en ;
                                                 rdfs:label "Transmodel Ontology - Commons"@en ;
                                                 rdfs:seeAlso "https://github.com/oeg-upm/transmodel-ontology"@en ;
                                                 owl:versionInfo "This is the initial version of the module on Commons, after considering the UML models and XSD descriptions of Transmodel and NeTEx"@en .

#################################################################
#    Annotation properties
#################################################################

###  http://creativecommons.org/ns#license
<http://creativecommons.org/ns#license> rdf:type owl:AnnotationProperty .


###  http://purl.org/dc/elements/1.1/creator
<http://purl.org/dc/elements/1.1/creator> rdf:type owl:AnnotationProperty .


###  http://purl.org/dc/elements/1.1/date
<http://purl.org/dc/elements/1.1/date> rdf:type owl:AnnotationProperty .


###  http://purl.org/dc/elements/1.1/description
<http://purl.org/dc/elements/1.1/description> rdf:type owl:AnnotationProperty .


###  http://purl.org/dc/elements/1.1/identifier
<http://purl.org/dc/elements/1.1/identifier> rdf:type owl:AnnotationProperty .


###  http://purl.org/dc/elements/1.1/rights
<http://purl.org/dc/elements/1.1/rights> rdf:type owl:AnnotationProperty .


###  http://purl.org/dc/elements/1.1/title
<http://purl.org/dc/elements/1.1/title> rdf:type owl:AnnotationProperty .


###  http://purl.org/vocab/vann/preferredNamespaceUri
<http://purl.org/vocab/vann/preferredNamespaceUri> rdf:type owl:AnnotationProperty .


###  http://www.w3.org/2000/01/rdf-schema#label
rdfs:label rdfs:range xsd:string .


###  https://w3id.org/mobility/transmodel/commons#author
:author rdf:type owl:AnnotationProperty .


###  https://w3id.org/mobility/transmodel/commons#creator
:creator rdf:type owl:AnnotationProperty .


###  https://w3id.org/mobility/transmodel/commons#description
:description rdf:type owl:AnnotationProperty ;
             rdfs:range rdfs:Literal ;
             rdfs:domain <https://w3id.org/transmodel/commons#MeetingPointService> .


###  https://w3id.org/mobility/transmodel/commons#mbox
:mbox rdf:type owl:AnnotationProperty .


###  https://w3id.org/mobility/transmodel/commons#name
:name rdf:type owl:AnnotationProperty ;
      rdfs:range rdfs:Literal .


#################################################################
#    Object Properties
#################################################################

###  https://w3id.org/mobility/transmodel/commons#aClasificationFor
:aClasificationFor rdf:type owl:ObjectProperty ;
                   rdfs:range :GroupOfEntities .


###  https://w3id.org/mobility/transmodel/commons#locatedBy
:locatedBy rdf:type owl:ObjectProperty ;
           rdfs:domain :Point ;
           rdfs:range :Location .


###  https://w3id.org/mobility/transmodel/commons#referenceFor
:referenceFor rdf:type owl:ObjectProperty .


###  https://w3id.org/transmodel/journeys#aViewOf
<https://w3id.org/transmodel/journeys#aViewOf> rdf:type owl:ObjectProperty .


#################################################################
#    Data properties
#################################################################

###  http://purl.org/dc/terms/identifier
<http://purl.org/dc/terms/identifier> rdf:type owl:DatatypeProperty .


###  http://www.w3.org/2000/01/rdf-schema#comment
rdfs:comment rdf:type owl:DatatypeProperty ;
             rdfs:range xsd:string .


###  http://www.w3.org/2000/01/rdf-schema#label
rdfs:label rdf:type owl:DatatypeProperty .


###  http://www.w3.org/2003/01/geo/wgs84_pos#alt
<http://www.w3.org/2003/01/geo/wgs84_pos#alt> rdf:type owl:DatatypeProperty .


###  http://www.w3.org/2003/01/geo/wgs84_pos#lat
<http://www.w3.org/2003/01/geo/wgs84_pos#lat> rdf:type owl:DatatypeProperty .


###  http://www.w3.org/2003/01/geo/wgs84_pos#lat_long
<http://www.w3.org/2003/01/geo/wgs84_pos#lat_long> rdf:type owl:DatatypeProperty .


###  http://www.w3.org/2003/01/geo/wgs84_pos#long
<http://www.w3.org/2003/01/geo/wgs84_pos#long> rdf:type owl:DatatypeProperty .


###  https://w3id.org/mobility/transmodel/commons#borderCrossing
:borderCrossing rdf:type owl:DatatypeProperty ;
                rdfs:range xsd:boolean .


###  https://w3id.org/mobility/transmodel/commons#colour
:colour rdf:type owl:DatatypeProperty ;
        rdfs:range xsd:string .


###  https://w3id.org/mobility/transmodel/commons#precision
:precision rdf:type owl:DatatypeProperty ;
           rdfs:domain :Location ;
           rdfs:range xsd:string .


###  https://w3id.org/mobility/transmodel/commons#textColour
:textColour rdf:type owl:DatatypeProperty ;
            rdfs:range xsd:string .


###  https://w3id.org/transmodel/common#arrivalTime
<https://w3id.org/transmodel/common#arrivalTime> rdf:type owl:DatatypeProperty ;
                                                 rdfs:range xsd:dateTimeStamp .


###  https://w3id.org/transmodel/common#headway
<https://w3id.org/transmodel/common#headway> rdf:type owl:DatatypeProperty ;
                                             rdfs:range xsd:dateTimeStamp .


###  https://w3id.org/transmodel/common#layover
<https://w3id.org/transmodel/common#layover> rdf:type owl:DatatypeProperty ;
                                             rdfs:range xsd:dateTimeStamp .


###  https://w3id.org/transmodel/common#pointSequence
<https://w3id.org/transmodel/common#pointSequence> rdf:type owl:DatatypeProperty ;
                                                   rdfs:range xsd:nonNegativeInteger .


###  https://w3id.org/transmodel/common#runtime
<https://w3id.org/transmodel/common#runtime> rdf:type owl:DatatypeProperty ;
                                             rdfs:range xsd:nonNegativeInteger .


###  https://w3id.org/transmodel/common#startTime
<https://w3id.org/transmodel/common#startTime> rdf:type owl:DatatypeProperty ;
                                               rdfs:range xsd:string .


###  https://w3id.org/transmodel/common#time
<https://w3id.org/transmodel/common#time> rdf:type owl:DatatypeProperty ;
                                          rdfs:range xsd:dateTimeStamp .


###  https://w3id.org/transmodel/common#timeLink
<https://w3id.org/transmodel/common#timeLink> rdf:type owl:DatatypeProperty ;
                                              rdfs:range xsd:nonNegativeInteger .


###  https://w3id.org/transmodel/common#waitTime
<https://w3id.org/transmodel/common#waitTime> rdf:type owl:DatatypeProperty ;
                                              rdfs:range xsd:string .


#################################################################
#    Classes
#################################################################

###  http://www.w3.org/2004/02/skos/core#ConceptScheme
<http://www.w3.org/2004/02/skos/core#ConceptScheme> rdf:type owl:Class .


###  https://w3id.org/mobility/transmodel/commons#GroupOfEntities
:GroupOfEntities rdf:type owl:Class .


###  https://w3id.org/mobility/transmodel/commons#Layer
:Layer rdf:type owl:Class ;
       rdfs:subClassOf :GroupOfEntities .


###  https://w3id.org/mobility/transmodel/commons#LocatingSystem
:LocatingSystem rdf:type owl:Class ;
                rdfs:subClassOf [ rdf:type owl:Restriction ;
                                  owl:onProperty :referenceFor ;
                                  owl:someValuesFrom :Location
                                ] ,
                                [ rdf:type owl:Restriction ;
                                  owl:onProperty <http://purl.org/dc/terms/identifier> ;
                                  owl:someValuesFrom xsd:string
                                ] ,
                                [ rdf:type owl:Restriction ;
                                  owl:onProperty rdfs:label ;
                                  owl:someValuesFrom xsd:string
                                ] .


###  https://w3id.org/mobility/transmodel/commons#Location
:Location rdf:type owl:Class ;
          rdfs:subClassOf [ rdf:type owl:Restriction ;
                            owl:onProperty <http://purl.org/dc/terms/identifier> ;
                            owl:someValuesFrom xsd:string
                          ] ,
                          [ rdf:type owl:Restriction ;
                            owl:onProperty <http://www.w3.org/2003/01/geo/wgs84_pos#alt> ;
                            owl:maxQualifiedCardinality "1"^^xsd:nonNegativeInteger ;
                            owl:onDataRange xsd:float
                          ] ,
                          [ rdf:type owl:Restriction ;
                            owl:onProperty <http://www.w3.org/2003/01/geo/wgs84_pos#lat> ;
                            owl:maxQualifiedCardinality "1"^^xsd:nonNegativeInteger ;
                            owl:onDataRange xsd:float
                          ] ,
                          [ rdf:type owl:Restriction ;
                            owl:onProperty <http://www.w3.org/2003/01/geo/wgs84_pos#lat_long> ;
                            owl:maxQualifiedCardinality "1"^^xsd:nonNegativeInteger ;
                            owl:onDataRange xsd:string
                          ] ,
                          [ rdf:type owl:Restriction ;
                            owl:onProperty <http://www.w3.org/2003/01/geo/wgs84_pos#long> ;
                            owl:maxQualifiedCardinality "1"^^xsd:nonNegativeInteger ;
                            owl:onDataRange xsd:float
                          ] .


###  https://w3id.org/mobility/transmodel/commons#Place
:Place rdf:type owl:Class ;
       rdfs:subClassOf :Zone .


###  https://w3id.org/mobility/transmodel/commons#Point
:Point rdf:type owl:Class ;
       rdfs:subClassOf [ rdf:type owl:Restriction ;
                         owl:onProperty :locatedBy ;
                         owl:qualifiedCardinality "1"^^xsd:nonNegativeInteger ;
                         owl:onClass :Location
                       ] .


###  https://w3id.org/mobility/transmodel/commons#Presentation
:Presentation rdf:type owl:Class ;
              rdfs:subClassOf [ rdf:type owl:Restriction ;
                                owl:onProperty :colour ;
                                owl:allValuesFrom xsd:string
                              ] ,
                              [ rdf:type owl:Restriction ;
                                owl:onProperty :textColour ;
                                owl:allValuesFrom xsd:string
                              ] .


###  https://w3id.org/mobility/transmodel/commons#PurposeOfGrouping
:PurposeOfGrouping rdf:type owl:Class ;
                   rdfs:subClassOf [ rdf:type owl:Restriction ;
                                     owl:onProperty :aClasificationFor ;
                                     owl:allValuesFrom :GroupOfEntities
                                   ] .


###  https://w3id.org/mobility/transmodel/commons#Version
:Version rdf:type owl:Class .


###  https://w3id.org/mobility/transmodel/commons#VersionFrame
:VersionFrame rdf:type owl:Class ;
              rdfs:subClassOf [ rdf:type owl:Restriction ;
                                owl:onProperty rdfs:comment ;
                                owl:someValuesFrom xsd:string
                              ] ,
                              [ rdf:type owl:Restriction ;
                                owl:onProperty rdfs:label ;
                                owl:someValuesFrom xsd:string
                              ] .


###  https://w3id.org/mobility/transmodel/commons#Zone
:Zone rdf:type owl:Class .


#################################################################
#    Individuals
#################################################################

###  http://purl.org/dc/terms/identifier
<http://purl.org/dc/terms/identifier> rdf:type owl:NamedIndividual .


###  http://www.w3.org/2000/01/rdf-schema#label
rdfs:label rdf:type owl:NamedIndividual .


###  http://www.w3.org/2003/01/geo/wgs84_pos#alt
<http://www.w3.org/2003/01/geo/wgs84_pos#alt> rdf:type owl:NamedIndividual .


###  http://www.w3.org/2003/01/geo/wgs84_pos#lat
<http://www.w3.org/2003/01/geo/wgs84_pos#lat> rdf:type owl:NamedIndividual .


###  http://www.w3.org/2003/01/geo/wgs84_pos#lat_long
<http://www.w3.org/2003/01/geo/wgs84_pos#lat_long> rdf:type owl:NamedIndividual .


###  http://www.w3.org/2003/01/geo/wgs84_pos#long
<http://www.w3.org/2003/01/geo/wgs84_pos#long> rdf:type owl:NamedIndividual .


###  https://w3id.org/mobility/transmodel/commons#ClassInRepository
:ClassInRepository rdf:type owl:NamedIndividual ;
                   rdfs:comment "any entity name belonging to the repository.  e.g. day type, property of day, time band, vehicle type,  etc, are relevant instances of class in repository in the context of version management."@en .


###  https://w3id.org/mobility/transmodel/commons#Entity
:Entity rdf:type owl:NamedIndividual ;
        rdfs:comment "Any data instance to be managed in an operational version management system. when several data sources coexist (multimodality and/or interoperability), an entity has to be related to a given data source in which it is defined."@en .


###  https://w3id.org/mobility/transmodel/commons#EntityInVersion
:EntityInVersion rdf:type owl:NamedIndividual ;
                 rdfs:comment "The entity associated to a given version."@en .


###  https://w3id.org/mobility/transmodel/commons#GroupOfEntities
:GroupOfEntities rdf:type owl:NamedIndividual ;
                 rdfs:comment "A set of Entities grouped together according to a Purpose of Grouping, e.g. grouping of stops known to the public by a common name."@en .


###  https://w3id.org/mobility/transmodel/commons#Layer
:Layer rdf:type owl:NamedIndividual ;
       rdfs:comment "A user-defined group of entities, specified for a particular functional purpose, associating data referring to a particular locating system."@en .


###  https://w3id.org/mobility/transmodel/commons#LocatingSystem
:LocatingSystem rdf:type owl:NamedIndividual ;
                rdfs:comment "The system used as reference for location and graphical representation of the network and other spatial objects."@en .


###  https://w3id.org/mobility/transmodel/commons#Location
:Location rdf:type owl:NamedIndividual ;
          rdfs:comment "The position of a Point with a reference to a given Locating System  (e. g. coordinates)."@en ,
                       "The position of a point with a reference to a given locating system (e. g. coordinates)."@en ,
                       "the position of a Point with a reference to a given locating system (e. g. coordinates)."@en .


###  https://w3id.org/mobility/transmodel/commons#Place
:Place rdf:type owl:NamedIndividual ;
       rdfs:comment "A geographic place of any type which may be specified as the origin or destination of a trip. A Place may be represented as a Point (dimension 0), a road section (dimension 1) or a Zone (dimension 2)."@en .


###  https://w3id.org/mobility/transmodel/commons#Point
:Point rdf:type owl:NamedIndividual ;
       rdfs:comment "A Point is a 0-dimensional Node of the Network used for the spatial description of the network. Point may be located by a Location"@en ,
                    "TODO: Make it in that ontology a subclass of the W3C Geo Point"@en .


###  https://w3id.org/mobility/transmodel/commons#Presentation
:Presentation rdf:type owl:NamedIndividual ;
              rdfs:comment "This class is used to represent a Line, or any other object, in a map"@en .


###  https://w3id.org/mobility/transmodel/commons#PurposeOfGrouping
:PurposeOfGrouping rdf:type owl:NamedIndividual ;
                   rdfs:comment "functional purpose for which groups of elements are defined. the purpose of grouping may be restricted to one or more types of the given object."@en .


###  https://w3id.org/mobility/transmodel/commons#ValidityCondition
:ValidityCondition rdf:type owl:NamedIndividual ;
                   rdfs:comment "Condition used in order to characterise a given version of a version frame. a validity condition consists of a parameter (e.g. date, triggering event, etc.) and its type of application  (e.g. for,  from,  until, etc.)."@en .


###  https://w3id.org/mobility/transmodel/commons#Version
:Version rdf:type owl:NamedIndividual ;
         rdfs:comment "A group of operational data instances which share the same validity conditions. a version belongs to a unique version frame and is characterised by a unique type of version."@en .


###  https://w3id.org/mobility/transmodel/commons#VersionFrame
:VersionFrame rdf:type owl:NamedIndividual ;
              rdfs:comment "A set of versions referring to a same data source and belonging to the same type of frame. a frame may be restricted by validity conditions."@en .


###  https://w3id.org/mobility/transmodel/commons#Zone
:Zone rdf:type owl:NamedIndividual ;
      rdfs:comment """A two dimensional Place within the Service Area of an Operator or Serviced Operator. It can be:
- AdministrativeZone
- TariffZone
- AccessZone
- ..."""@en .


###  https://w3id.org/mobility/transmodel/commons#at
:at rdf:type owl:NamedIndividual ;
    rdfs:comment "This property sets the relationship between something and other thing related to it. It is used in multiple situations and modules of this ontology"@en .


###  https://w3id.org/mobility/transmodel/commons#borderCrossing
:borderCrossing rdf:type owl:NamedIndividual .


###  https://w3id.org/mobility/transmodel/commons#colour
:colour rdf:type owl:NamedIndividual ;
        rdfs:comment "The colour used to represent something with a Presentation (e.g., a Line)"@en .


###  https://w3id.org/mobility/transmodel/commons#in
:in rdf:type owl:NamedIndividual ;
    rdfs:comment "This property sets the relationship between something and other thing contained in the first. It is used in multiple situations and modules of this ontology (e.g., Quay in Stop Place)"@en .


###  https://w3id.org/mobility/transmodel/commons#precision
:precision rdf:type owl:NamedIndividual ;
           rdfs:comment "Precision of coordinates."@en .


###  https://w3id.org/mobility/transmodel/commons#referenceFor
:referenceFor rdf:type owl:NamedIndividual ;
              rdfs:comment "This property references for location"@en .


###  https://w3id.org/mobility/transmodel/commons#textColour
:textColour rdf:type owl:NamedIndividual ;
            rdfs:comment "The colour used to represent the text associated to something with a Presentation (e.g., a Line)"@en .


###  https://w3id.org/transmodel/common#ActivationLink
<https://w3id.org/transmodel/common#ActivationLink> rdf:type owl:NamedIndividual ;
                                                    rdfs:comment "A Link where a control process is activated when a vehicle passes it"@en .


###  https://w3id.org/transmodel/common#ActivationPoint
<https://w3id.org/transmodel/common#ActivationPoint> rdf:type owl:NamedIndividual ;
                                                     rdfs:comment "A Point where a control process is activated when a vehicle passes it. Equipment may be needed for activation" .


###  https://w3id.org/transmodel/common#HeadingInterval
<https://w3id.org/transmodel/common#HeadingInterval> rdf:type owl:NamedIndividual ;
                                                     rdfs:comment "A time interval or a duration defining a headway period and characterizing HeadwayJourneyGroup"@en .


###  https://w3id.org/transmodel/common#JourneyPatternLayover
<https://w3id.org/transmodel/common#JourneyPatternLayover> rdf:type owl:NamedIndividual ;
                                                           rdfs:comment "A JourneyPatternLayover is the time allowance at the end of each journey on a specified JourneyPattern to allow for delays and for other purposes. This layover supersedes any global layover and may be superseded by a specific VehicleJourneyLayover"@en .


###  https://w3id.org/transmodel/common#Passenger
<https://w3id.org/transmodel/common#Passenger> rdf:type owl:NamedIndividual ;
                                               rdfs:comment "A Passenger is someone who makes a Trip"@en ,
                                                            "When a Passenger makes a Journey it is a Trip; when a Vehicle does it is a VehicleJourney"@en .


###  https://w3id.org/transmodel/common#Point
<https://w3id.org/transmodel/common#Point> rdf:type owl:NamedIndividual ;
                                           rdfs:comment "A Point is a 0-dimensional Node of the Network used for the spatial description of the network. Point may be located by a Location"@en .


###  https://w3id.org/transmodel/common#Service
<https://w3id.org/transmodel/common#Service> rdf:type owl:NamedIndividual ;
                                             rdfs:comment """A ServiceJourney is a Passenger carrying VehicleJourney for one
specified DayType. The pattern of working is in principle defined
by a ServiceJourneyPattern."""@en .


###  https://w3id.org/transmodel/common#TimingLink
<https://w3id.org/transmodel/common#TimingLink> rdf:type owl:NamedIndividual .


###  https://w3id.org/transmodel/common#TimingLinkInJourneyPattern
<https://w3id.org/transmodel/common#TimingLinkInJourneyPattern> rdf:type owl:NamedIndividual ;
                                                                rdfs:comment """A TimingLinkInJourneyPattern is the position of a TimingLink in a
JourneyPattern. This entity is needed if a TimingLink is repeated
in the same JourneyPattern, and separate information is to be stored
about each iteration of the TimingLink"""@en .


###  https://w3id.org/transmodel/common#TimingPoint
<https://w3id.org/transmodel/common#TimingPoint> rdf:type owl:NamedIndividual ;
                                                 rdfs:comment """A TimingPoint is a Point against which the timing information necessary to build schedules may be
recorded. It's the same as TimingPointInJourneyPattern"""@en .


###  https://w3id.org/transmodel/common#Trip
<https://w3id.org/transmodel/common#Trip> rdf:type owl:NamedIndividual ;
                                          rdfs:comment "The physical spatial possibility for a passenger to travel from a Place (located Point) origin of the Trip to another place (located Point) destination of the Trip."@en .


###  https://w3id.org/transmodel/common#Vehicle
<https://w3id.org/transmodel/common#Vehicle> rdf:type owl:NamedIndividual ;
                                             rdfs:comment "A PublicTransportVehicle used for carrying Passengers"@en .


###  https://w3id.org/transmodel/common#VehicleJourneyLayover
<https://w3id.org/transmodel/common#VehicleJourneyLayover> rdf:type owl:NamedIndividual .


###  https://w3id.org/transmodel/common#arrivalTime
<https://w3id.org/transmodel/common#arrivalTime> rdf:type owl:NamedIndividual .


###  https://w3id.org/transmodel/common#canAlight
<https://w3id.org/transmodel/common#canAlight> rdf:type owl:NamedIndividual .


###  https://w3id.org/transmodel/common#canBoard
<https://w3id.org/transmodel/common#canBoard> rdf:type owl:NamedIndividual .


###  https://w3id.org/transmodel/common#destinationStop
<https://w3id.org/transmodel/common#destinationStop> rdf:type owl:NamedIndividual .


###  https://w3id.org/transmodel/common#followsJourneyPattern
<https://w3id.org/transmodel/common#followsJourneyPattern> rdf:type owl:NamedIndividual .


###  https://w3id.org/transmodel/common#hasAServiceJourneyPattern
<https://w3id.org/transmodel/common#hasAServiceJourneyPattern> rdf:type owl:NamedIndividual .


###  https://w3id.org/transmodel/common#headway
<https://w3id.org/transmodel/common#headway> rdf:type owl:NamedIndividual .


###  https://w3id.org/transmodel/common#journeyPatternPoint
<https://w3id.org/transmodel/common#journeyPatternPoint> rdf:type owl:NamedIndividual .


###  https://w3id.org/transmodel/common#layover
<https://w3id.org/transmodel/common#layover> rdf:type owl:NamedIndividual .


###  https://w3id.org/transmodel/common#makesAServiceJourney
<https://w3id.org/transmodel/common#makesAServiceJourney> rdf:type owl:NamedIndividual .


###  https://w3id.org/transmodel/common#originStop
<https://w3id.org/transmodel/common#originStop> rdf:type owl:NamedIndividual .


###  https://w3id.org/transmodel/common#pointSequence
<https://w3id.org/transmodel/common#pointSequence> rdf:type owl:NamedIndividual ;
                                                   rdfs:comment "Sequences of ScheduledStopPoint"@en .


###  https://w3id.org/transmodel/common#route
<https://w3id.org/transmodel/common#route> rdf:type owl:NamedIndividual .


###  https://w3id.org/transmodel/common#runtime
<https://w3id.org/transmodel/common#runtime> rdf:type owl:NamedIndividual .


###  https://w3id.org/transmodel/common#scheduledStopPoint
<https://w3id.org/transmodel/common#scheduledStopPoint> rdf:type owl:NamedIndividual .


###  https://w3id.org/transmodel/common#startTime
<https://w3id.org/transmodel/common#startTime> rdf:type owl:NamedIndividual .


###  https://w3id.org/transmodel/common#stopsAt
<https://w3id.org/transmodel/common#stopsAt> rdf:type owl:NamedIndividual .


###  https://w3id.org/transmodel/common#time
<https://w3id.org/transmodel/common#time> rdf:type owl:NamedIndividual .


###  https://w3id.org/transmodel/common#timeLink
<https://w3id.org/transmodel/common#timeLink> rdf:type owl:NamedIndividual ;
                                              rdfs:comment "Sequences of TimePoints"@en .


###  https://w3id.org/transmodel/common#timingLink
<https://w3id.org/transmodel/common#timingLink> rdf:type owl:NamedIndividual .


###  https://w3id.org/transmodel/common#timingLinkInJourneyPattern
<https://w3id.org/transmodel/common#timingLinkInJourneyPattern> rdf:type owl:NamedIndividual .


###  https://w3id.org/transmodel/common#vehicleJourney
<https://w3id.org/transmodel/common#vehicleJourney> rdf:type owl:NamedIndividual .


###  https://w3id.org/transmodel/common#vehicleJourneyDayType
<https://w3id.org/transmodel/common#vehicleJourneyDayType> rdf:type owl:NamedIndividual .


###  https://w3id.org/transmodel/common#vehicleJourneyRoute
<https://w3id.org/transmodel/common#vehicleJourneyRoute> rdf:type owl:NamedIndividual .


###  https://w3id.org/transmodel/common#waitTime
<https://w3id.org/transmodel/common#waitTime> rdf:type owl:NamedIndividual .


###  https://w3id.org/transmodel/kos/commons/all-modes
<https://w3id.org/transmodel/kos/commons/all-modes> rdf:type owl:NamedIndividual ,
                                                             <http://www.w3.org/2004/02/skos/core#ConceptScheme> .


###  https://w3id.org/transmodel/kos/commons/continous-mode
<https://w3id.org/transmodel/kos/commons/continous-mode> rdf:type owl:NamedIndividual ,
                                                                  <http://www.w3.org/2004/02/skos/core#ConceptScheme> .


###  https://w3id.org/transmodel/kos/commons/road-vehicle-mode
<https://w3id.org/transmodel/kos/commons/road-vehicle-mode> rdf:type owl:NamedIndividual ,
                                                                     <http://www.w3.org/2004/02/skos/core#ConceptScheme> ;
                                                            rdfs:label "road-vehicle-mode"@en .


###  https://w3id.org/transmodel/kos/commons/sites-access-mode
<https://w3id.org/transmodel/kos/commons/sites-access-mode> rdf:type owl:NamedIndividual ,
                                                                     <http://www.w3.org/2004/02/skos/core#ConceptScheme> .


###  https://w3id.org/transmodel/kos/commons/vehicle-mode
<https://w3id.org/transmodel/kos/commons/vehicle-mode> rdf:type owl:NamedIndividual ,
                                                                <http://www.w3.org/2004/02/skos/core#ConceptScheme> .


_:genid15 :mbox "adolfo.anton.bravo@upm.es"@en ;
          :name "Adolfo Anton-Bravo"@en .

#################################################################
#    Annotations
#################################################################

<http://purl.org/dc/terms/identifier> rdfs:label "identifier"@en .


rdfs:comment rdfs:label "description"@en .


rdfs:label rdfs:label "name"@en .


<http://www.w3.org/2003/01/geo/wgs84_pos#alt> rdfs:label "altitude"@en .


<http://www.w3.org/2003/01/geo/wgs84_pos#lat> rdfs:label "latitude"@en .


<http://www.w3.org/2003/01/geo/wgs84_pos#lat_long> rdfs:label "coordinates"@en .


<http://www.w3.org/2003/01/geo/wgs84_pos#long> rdfs:label "longitude"@en .


:GroupOfEntities rdfs:label "Group of Entities"@en .


:LocatingSystem rdfs:label "LocatingSystem"@en .


:Location rdfs:label "Location"@en .


:Place rdfs:label "Place"@en .


:Point rdfs:label "Point"@en .


:Presentation rdfs:label "Presentation"@en .


:Zone rdfs:label "Zone"@en .


:borderCrossing rdfs:label "This property determines whether the Point is on a border crossing"@en ,
                           "border crossing"@en .


:colour rdfs:label "colour"@en .


:precision rdfs:label "precision"@en .


:textColour rdfs:label "text colour"@en .


<https://w3id.org/transmodel/common#arrivalTime> rdfs:label "arrivalTime"@en .


<https://w3id.org/transmodel/common#headway> rdfs:label "headway"@en .


<https://w3id.org/transmodel/common#layover> rdfs:label "layover"@en .


<https://w3id.org/transmodel/common#pointSequence> rdfs:label "stopSequence"@en .


<https://w3id.org/transmodel/common#runtime> rdfs:label "runtime"@en .


<https://w3id.org/transmodel/common#startTime> rdfs:label "startTime"@en .


<https://w3id.org/transmodel/common#time> rdfs:label "time"@en .


<https://w3id.org/transmodel/common#timeLink> rdfs:label "timeLink"@en .


<https://w3id.org/transmodel/common#waitTime> rdfs:label "waitTime"@en .


###  Generated by the OWL API (version 5.1.18) https://github.com/owlcs/owlapi/
