@prefix dct: <http://purl.org/dc/terms/> .
@prefix rdf: <http://www.w3.org/1999/02/22-rdf-syntax-ns#> .
@prefix skos: <http://www.w3.org/2004/02/skos/core#> .
@prefix xsd: <http://www.w3.org/2001/XMLSchema#> .

<https://w3id.org/osdm/core/location> a skos:ConceptScheme;
  dct:description "Locations are resources representing a specific location in a trip:";
  dct:title "location";
  skos:hasTopConcept <https://w3id.org/osdm/core/Location/address>, <https://w3id.org/osdm/core/Location/connectionPoint>,
    <https://w3id.org/osdm/core/Location/geoCoordibnate>, <https://w3id.org/osdm/core/Location/poi>,
    <https://w3id.org/osdm/core/Location/station> .

<https://w3id.org/osdm/core/Location/address> a skos:Concept;
  skos:definition "Any street address can be represented here.";
  skos:inScheme <https://w3id.org/osdm/core/location>;
  skos:notation "address";
  skos:prefLabel "address";
  skos:topConceptOf <https://w3id.org/osdm/core/location> .

<https://w3id.org/osdm/core/Location/station> a skos:Concept;
  skos:definition "represent a train station. It is obviously the most relevant type for OSDM. Stations can be indicated as codes from different code sets.";
  skos:inScheme <https://w3id.org/osdm/core/location>;
  skos:notation "station";
  skos:prefLabel "station";
  skos:topConceptOf <https://w3id.org/osdm/core/location> .

<https://w3id.org/osdm/core/Location/poi> a skos:Concept;
  skos:definition "Represent a specific point of interest";
  skos:inScheme <https://w3id.org/osdm/core/location>;
  skos:notation "poi";
  skos:prefLabel "POI";
  skos:topConceptOf <https://w3id.org/osdm/core/location> .

<https://w3id.org/osdm/core/Location/geoCoordibnate> a skos:Concept;
  skos:definition "Providing any location on the globe using its geographical coordinates.";
  skos:inScheme <https://w3id.org/osdm/core/location>;
  skos:notation "geoCoordibnate";
  skos:prefLabel "GeoCoordibnate";
  skos:topConceptOf <https://w3id.org/osdm/core/location> .

<https://w3id.org/osdm/core/Location/connectionPoint> a skos:Concept;
  skos:definition "Allows to model virtual border points by defining stations within the connection point lies";
  skos:inScheme <https://w3id.org/osdm/core/location>;
  skos:notation "connectionPoint";
  skos:prefLabel "ConnectionPoint";
  skos:topConceptOf <https://w3id.org/osdm/core/location> .