@prefix : <https://w3id.org/mobility/transmodel/journeys#> .
@prefix owl: <http://www.w3.org/2002/07/owl#> .
@prefix rdf: <http://www.w3.org/1999/02/22-rdf-syntax-ns#> .
@prefix xml: <http://www.w3.org/XML/1998/namespace> .
@prefix xsd: <http://www.w3.org/2001/XMLSchema#> .
@prefix rdfs: <http://www.w3.org/2000/01/rdf-schema#> .
@base <https://w3id.org/mobility/transmodel/journeys#> .

<https://w3id.org/mobility/transmodel/journeys#> rdf:type owl:Ontology ;
                                                  owl:versionIRI <https://w3id.org/mobility/transmodel/journeys/0.3.0> ;
                                                  <http://creativecommons.org/ns#license> <http://creativecommons.org/licenses/by/4.0/> ;
                                                  <http://purl.org/dc/elements/1.1/abstract> ""@en ;
                                                  <http://purl.org/dc/elements/1.1/creator> "Jhon Toledo (Ontology Engienering Group - Universidad Politécnica de Madrid)"@en ,
                                                                                            "Miguel Angel García (Ontology Engienering Group - Universidad Politécnica de Madrid)"@en ,
                                                                                            "Oscar Corcho (Ontology Engineering Group - Universidad Politécnica de Madrid)" ;
                                                  <http://purl.org/dc/elements/1.1/date> "2022-03-09"@en ;
                                                  <http://purl.org/dc/elements/1.1/description> "Module of the Transmodel Ontology focused on journeys. This ontology provides support to the NeTEx model. Visit https://github.com/oeg-upm/mobility"@en ;
                                                  <http://purl.org/dc/elements/1.1/identifier> "https://w3id.org/mobility/transmodel/journeys"@en ;
                                                  <http://purl.org/dc/elements/1.1/rights> "Creative Commons Attribution 4.0 International (CC BY 4.0)" ;
                                                  <http://purl.org/dc/elements/1.1/title> "Transmodel Ontology - Journeys"@en ;
                                                  <http://purl.org/vocab/vann/preferredNamespaceUri> <https://w3id.org/mobility/transmodel/journeys#> ;
                                                  rdfs:comment "Module of the Transmodel Ontology focused on facilities. This ontology provides support to the NeTEx model. Visit https://github.com/oeg-upm/mobility"@en ;
                                                  rdfs:label "Transmodel Ontology - Journeys"@en ;
                                                  rdfs:seeAlso "https://github.com/oeg-upm/mobility"@en ;
                                                  owl:versionInfo "This is the initial version of the module on Journeys, after considering the UML models and XSD descriptions of Transmodel and NeTEx"@en .

#################################################################
#    Annotation properties
#################################################################

###  http://creativecommons.org/ns#license
<http://creativecommons.org/ns#license> rdf:type owl:AnnotationProperty .


###  http://purl.org/dc/elements/1.1/abstract
<http://purl.org/dc/elements/1.1/abstract> rdf:type owl:AnnotationProperty .


###  http://purl.org/dc/elements/1.1/creator
<http://purl.org/dc/elements/1.1/creator> rdf:type owl:AnnotationProperty .


###  http://purl.org/dc/elements/1.1/date
<http://purl.org/dc/elements/1.1/date> rdf:type owl:AnnotationProperty .


###  http://purl.org/dc/elements/1.1/description
<http://purl.org/dc/elements/1.1/description> rdf:type owl:AnnotationProperty .


###  http://purl.org/dc/elements/1.1/identifier
<http://purl.org/dc/elements/1.1/identifier> rdf:type owl:AnnotationProperty .


###  http://purl.org/dc/elements/1.1/rights
<http://purl.org/dc/elements/1.1/rights> rdf:type owl:AnnotationProperty .


###  http://purl.org/dc/elements/1.1/title
<http://purl.org/dc/elements/1.1/title> rdf:type owl:AnnotationProperty .


###  http://purl.org/dc/terms/bibliographicCitation
<http://purl.org/dc/terms/bibliographicCitation> rdf:type owl:AnnotationProperty .


###  http://purl.org/vocab/vann/preferredNamespaceUri
<http://purl.org/vocab/vann/preferredNamespaceUri> rdf:type owl:AnnotationProperty .


###  http://www.w3.org/2000/01/rdf-schema#comment
rdfs:comment rdfs:range xsd:string .


###  http://www.w3.org/2000/01/rdf-schema#label
rdfs:label rdfs:range xsd:string .


###  https://w3id.org/mobility/transmodel/journeys#author
:author rdf:type owl:AnnotationProperty .


###  https://w3id.org/mobility/transmodel/journeys#creator
:creator rdf:type owl:AnnotationProperty .


###  https://w3id.org/mobility/transmodel/journeys#description
:description rdf:type owl:AnnotationProperty ;
             rdfs:range rdfs:Literal ;
             rdfs:domain <https://w3id.org/mobility/transmodel/journeys#MeetingPointService> .


###  https://w3id.org/mobility/transmodel/journeys#mbox
:mbox rdf:type owl:AnnotationProperty .


###  https://w3id.org/mobility/transmodel/journeys#name
:name rdf:type owl:AnnotationProperty ;
      rdfs:range rdfs:Literal .


#################################################################
#    Datatypes
#################################################################

###  http://www.w3.org/2000/01/rdf-schema#range
rdfs:range rdf:type rdfs:Datatype .


###  http://www.w3.org/2001/XMLSchema#duration
xsd:duration rdf:type rdfs:Datatype .


###  http://www.w3.org/2001/XMLSchema#time
xsd:time rdf:type rdfs:Datatype .


#################################################################
#    Object Properties
#################################################################

###  http://www.w3.org/2004/02/skos/core#inScheme
<http://www.w3.org/2004/02/skos/core#inScheme> rdf:type owl:ObjectProperty .


###  https://w3id.org/mobility/transmodel/journeys#PROPS-TO-REVIEW
:PROPS-TO-REVIEW rdf:type owl:ObjectProperty .


###  https://w3id.org/mobility/transmodel/journeys#aViewOf
:aViewOf rdf:type owl:ObjectProperty ;
         rdfs:subPropertyOf owl:topObjectProperty ;
         owl:inverseOf :viewedAs ;
         rdfs:domain <https://w3id.org/mobility/transmodel/commons#Point> ;
         rdfs:range :PointInLinkSequence ,
                    <https://w3id.org/mobility/transmodel/commons#PointOnRoute> .


###  https://w3id.org/mobility/transmodel/journeys#accessMode
:accessMode rdf:type owl:ObjectProperty ;
            rdfs:subPropertyOf :PROPS-TO-REVIEW .


###  https://w3id.org/mobility/transmodel/journeys#accessPTS
:accessPTS rdf:type owl:ObjectProperty ;
           rdfs:subPropertyOf :PROPS-TO-REVIEW .


###  https://w3id.org/mobility/transmodel/journeys#allowedLineDirections
:allowedLineDirections rdf:type owl:ObjectProperty ;
                       rdfs:subPropertyOf :PROPS-TO-REVIEW ;
                       rdfs:domain :Route .


###  https://w3id.org/mobility/transmodel/journeys#beginsConnection
:beginsConnection rdf:type owl:ObjectProperty ;
                  rdfs:subPropertyOf :PROPS-TO-REVIEW ;
                  rdfs:range :ScheduledStopPoint .


###  https://w3id.org/mobility/transmodel/journeys#belongingTo
:belongingTo rdf:type owl:ObjectProperty ;
             rdfs:domain <https://w3id.org/mobility/transmodel/facilities#VehicleType> ;
             rdfs:range :VehicleMode .


###  https://w3id.org/mobility/transmodel/journeys#blockPart
:blockPart rdf:type owl:ObjectProperty ;
           rdfs:subPropertyOf :PROPS-TO-REVIEW .


###  https://w3id.org/mobility/transmodel/journeys#canAlight
:canAlight rdf:type owl:ObjectProperty ;
           rdfs:subPropertyOf :PROPS-TO-REVIEW ;
           rdfs:range :ScheduledStopPoint .


###  https://w3id.org/mobility/transmodel/journeys#canBoard
:canBoard rdf:type owl:ObjectProperty ;
          rdfs:subPropertyOf :PROPS-TO-REVIEW ;
          rdfs:range :ScheduledStopPoint .


###  https://w3id.org/mobility/transmodel/journeys#characterisedBy
:characterisedBy rdf:type owl:ObjectProperty ;
                 rdfs:domain :Journey ;
                 rdfs:range <https://w3id.org/mobility/transmodel/facilities#AccessibilityAssessment> .


###  https://w3id.org/mobility/transmodel/journeys#classifiedBy
:classifiedBy rdf:type owl:ObjectProperty ;
              rdfs:domain :Line ;
              rdfs:range [ owl:intersectionOf ( <http://www.w3.org/2004/02/skos/core#Concept>
                                                [ rdf:type owl:Restriction ;
                                                  owl:onProperty <http://www.w3.org/2004/02/skos/core#inScheme> ;
                                                  owl:hasValue <https://w3id.org/mobility/transmodel/kos/commons/all-modes>
                                                ]
                                              ) ;
                           rdf:type owl:Class
                         ] .


###  https://w3id.org/mobility/transmodel/journeys#composedOf
:composedOf rdf:type owl:ObjectProperty ;
            owl:inverseOf :runsOn ;
            rdfs:domain :VehicleJourney ;
            rdfs:range :JourneyFrequencyGroup .


###  https://w3id.org/mobility/transmodel/journeys#composedOfLink
:composedOfLink rdf:type owl:ObjectProperty ;
                rdfs:domain :GroupOfLinkSequences ;
                rdfs:range :LinkSequence .


###  https://w3id.org/mobility/transmodel/journeys#composedOfVehicle
:composedOfVehicle rdf:type owl:ObjectProperty .


###  https://w3id.org/mobility/transmodel/journeys#day
:day rdf:type owl:ObjectProperty ;
     rdfs:range [ owl:intersectionOf ( <http://www.w3.org/2004/02/skos/core#Concept>
                                       [ rdf:type owl:Restriction ;
                                         owl:onProperty <http://www.w3.org/2004/02/skos/core#inScheme> ;
                                         owl:hasValue <https://w3id.org/mobility/transmodel/kos/journeys/day-type>
                                       ]
                                     ) ;
                  rdf:type owl:Class
                ] .


###  https://w3id.org/mobility/transmodel/journeys#dayTypeAssignment
:dayTypeAssignment rdf:type owl:ObjectProperty ;
                   rdfs:subPropertyOf :PROPS-TO-REVIEW .


###  https://w3id.org/mobility/transmodel/journeys#defaultDeadRunRunTime
:defaultDeadRunRunTime rdf:type owl:ObjectProperty ;
                       rdfs:subPropertyOf :PROPS-TO-REVIEW ;
                       rdfs:domain :DeadRun .


###  https://w3id.org/mobility/transmodel/journeys#defaultInterchange
:defaultInterchange rdf:type owl:ObjectProperty ;
                    rdfs:subPropertyOf :PROPS-TO-REVIEW ;
                    rdfs:domain :ScheduledStopPoint .


###  https://w3id.org/mobility/transmodel/journeys#definedAs
:definedAs rdf:type owl:ObjectProperty ;
           rdfs:domain :PropertyOfDay ;
           rdfs:range [ owl:intersectionOf ( <http://www.w3.org/2004/02/skos/core#Concept>
                                             [ rdf:type owl:Restriction ;
                                               owl:onProperty <http://www.w3.org/2004/02/skos/core#inScheme> ;
                                               owl:hasValue <https://w3id.org/mobility/transmodel/kos/journeys/day-type>
                                             ]
                                           ) ;
                        rdf:type owl:Class
                      ] .


###  https://w3id.org/mobility/transmodel/journeys#defines
:defines rdf:type owl:ObjectProperty ;
         owl:inverseOf :isDefinedBy ;
         rdfs:domain :RhythmicalJourneyGroup ;
         rdfs:range :TemplateVehicleJourney .


###  https://w3id.org/mobility/transmodel/journeys#describedBy
:describedBy rdf:type owl:ObjectProperty ;
             rdfs:subPropertyOf owl:topObjectProperty ;
             rdfs:domain :DayType ;
             rdfs:range :PropertyOfDay .


###  https://w3id.org/mobility/transmodel/journeys#destinationDisplay
:destinationDisplay rdf:type owl:ObjectProperty ;
                    rdfs:range :DestinationDisplay .


###  https://w3id.org/mobility/transmodel/journeys#destinationStop
:destinationStop rdf:type owl:ObjectProperty ;
                 rdfs:subPropertyOf :PROPS-TO-REVIEW ;
                 rdfs:range :ScheduledStopPoint .


###  https://w3id.org/mobility/transmodel/journeys#determinedBy
:determinedBy rdf:type owl:ObjectProperty ;
              rdfs:domain :HeadwayJourneyGroup ;
              rdfs:range :HeadwayInterval .


###  https://w3id.org/mobility/transmodel/journeys#directionType
:directionType rdf:type owl:ObjectProperty ;
               rdfs:subPropertyOf owl:topObjectProperty ;
               rdfs:domain :ServiceJourney ;
               rdfs:range [ owl:intersectionOf ( <http://www.w3.org/2004/02/skos/core#Concept>
                                                 [ rdf:type owl:Restriction ;
                                                   owl:onProperty <http://www.w3.org/2004/02/skos/core#inScheme> ;
                                                   owl:hasValue <https://w3id.org/mobility/transmodel/kos/journeys/direction-type>
                                                 ]
                                               ) ;
                            rdf:type owl:Class
                          ] .


###  https://w3id.org/mobility/transmodel/journeys#directionType_old
:directionType_old rdf:type owl:ObjectProperty ;
                   rdfs:subPropertyOf :PROPS-TO-REVIEW .


###  https://w3id.org/mobility/transmodel/journeys#endOf
:endOf rdf:type owl:ObjectProperty .


###  https://w3id.org/mobility/transmodel/journeys#endOfBlock
:endOfBlock rdf:type owl:ObjectProperty ;
            rdfs:domain :ParkingPoint ;
            rdfs:range :Block .


###  https://w3id.org/mobility/transmodel/journeys#endingAt
:endingAt rdf:type owl:ObjectProperty ;
          rdfs:domain :OperatingPeriod ;
          rdfs:range :OperatingDay .


###  https://w3id.org/mobility/transmodel/journeys#endsConnection
:endsConnection rdf:type owl:ObjectProperty ;
                rdfs:subPropertyOf :PROPS-TO-REVIEW ;
                rdfs:range :ScheduledStopPoint .


###  https://w3id.org/mobility/transmodel/journeys#endsConnectionDefault
:endsConnectionDefault rdf:type owl:ObjectProperty ;
                       rdfs:subPropertyOf :endsConnection ;
                       rdfs:range :ScheduledStopPoint .


###  https://w3id.org/mobility/transmodel/journeys#followsDeadRunTime
:followsDeadRunTime rdf:type owl:ObjectProperty ;
                    rdfs:subPropertyOf :PROPS-TO-REVIEW ;
                    rdfs:domain :VehicleJourney ;
                    rdfs:range :DeadRunPattern .


###  https://w3id.org/mobility/transmodel/journeys#followsJourneyPattern
:followsJourneyPattern rdf:type owl:ObjectProperty ;
                       rdfs:subPropertyOf :PROPS-TO-REVIEW ;
                       rdfs:domain :VehicleJourney ;
                       rdfs:range :JourneyPattern .


###  https://w3id.org/mobility/transmodel/journeys#for
:for rdf:type owl:ObjectProperty ;
     rdfs:domain :StopAssignment .


###  https://w3id.org/mobility/transmodel/journeys#forServicedOrganisation
:forServicedOrganisation rdf:type owl:ObjectProperty ;
                         rdfs:domain :OrganisationDayType .


###  https://w3id.org/mobility/transmodel/journeys#holidayType
:holidayType rdf:type owl:ObjectProperty ;
             rdfs:range [ owl:intersectionOf ( <http://www.w3.org/2004/02/skos/core#Concept>
                                               [ rdf:type owl:Restriction ;
                                                 owl:onProperty <http://www.w3.org/2004/02/skos/core#inScheme> ;
                                                 owl:hasValue <https://w3id.org/mobility/transmodel/kos/journeys/day-type>
                                               ]
                                             ) ;
                          rdf:type owl:Class
                        ] .


###  https://w3id.org/mobility/transmodel/journeys#inLinkSequence
:inLinkSequence rdf:type owl:ObjectProperty ;
                rdfs:subPropertyOf owl:topObjectProperty ;
                owl:inverseOf :madeUpOf ;
                rdf:type owl:FunctionalProperty ;
                rdfs:domain :PointInLinkSequence ;
                rdfs:range :LinkSequence .


###  https://w3id.org/mobility/transmodel/journeys#isDefinedBy
:isDefinedBy rdf:type owl:ObjectProperty ;
             rdfs:domain :TemplateVehicleJourney ;
             rdfs:range :RhythmicalJourneyGroup .


###  https://w3id.org/mobility/transmodel/journeys#journeyPatternMadeUpOf
:journeyPatternMadeUpOf rdf:type owl:ObjectProperty ;
                        rdfs:subPropertyOf :PROPS-TO-REVIEW ;
                        rdfs:range :StopPointInJourneyPattern .


###  https://w3id.org/mobility/transmodel/journeys#journeyPatternPoint
:journeyPatternPoint rdf:type owl:ObjectProperty ;
                     rdfs:subPropertyOf :PROPS-TO-REVIEW ;
                     rdfs:domain :JourneyPattern ;
                     rdfs:range <https://w3id.org/mobility/transmodel/commons#Point> .


###  https://w3id.org/mobility/transmodel/journeys#journeyPatternRunTime
:journeyPatternRunTime rdf:type owl:ObjectProperty ;
                       rdfs:subPropertyOf :PROPS-TO-REVIEW ;
                       rdfs:domain :JourneyPattern .


###  https://w3id.org/mobility/transmodel/journeys#madeUpOf
:madeUpOf rdf:type owl:ObjectProperty ;
          rdfs:subPropertyOf owl:topObjectProperty ;
          rdfs:domain :LinkSequence ;
          rdfs:range :PointInLinkSequence .


###  https://w3id.org/mobility/transmodel/journeys#madeUsing
:madeUsing rdf:type owl:ObjectProperty ;
           rdfs:subPropertyOf owl:topObjectProperty ;
           rdfs:domain :ServiceJourney ;
           rdfs:range <https://w3id.org/mobility/transmodel/facilities#ServiceFacilitySet> .


###  https://w3id.org/mobility/transmodel/journeys#modeOfTransport
:modeOfTransport rdf:type owl:ObjectProperty ;
                 rdfs:subPropertyOf :PROPS-TO-REVIEW ;
                 rdfs:domain :Route .


###  https://w3id.org/mobility/transmodel/journeys#on
:on rdf:type owl:ObjectProperty ;
    rdfs:subPropertyOf owl:topObjectProperty .


###  https://w3id.org/mobility/transmodel/journeys#onLine
:onLine rdf:type owl:ObjectProperty ;
        rdfs:subPropertyOf :on ;
        rdfs:domain :Line ;
        rdfs:range :Route .


###  https://w3id.org/mobility/transmodel/journeys#onRoute
:onRoute rdf:type owl:ObjectProperty ;
         rdfs:subPropertyOf :on ;
         rdfs:domain :Route ;
         rdfs:range :ServiceJourneyPattern .


###  https://w3id.org/mobility/transmodel/journeys#operatedBy
:operatedBy rdf:type owl:ObjectProperty ;
            rdfs:domain :VehicleJourney ;
            rdfs:range <https://w3id.org/mobility/transmodel/facilities#VehicleType> .


###  https://w3id.org/mobility/transmodel/journeys#operatingPeriod
:operatingPeriod rdf:type owl:ObjectProperty ;
                 rdfs:range :OperatingPeriod .


###  https://w3id.org/mobility/transmodel/journeys#originStop
:originStop rdf:type owl:ObjectProperty ;
            rdfs:subPropertyOf :PROPS-TO-REVIEW ;
            rdfs:range :ScheduledStopPoint .


###  https://w3id.org/mobility/transmodel/journeys#overriding
:overriding rdf:type owl:ObjectProperty ;
            rdfs:domain :DynamicStopAssignment ;
            rdfs:range :PassengerStopAssignment .


###  https://w3id.org/mobility/transmodel/journeys#passengerConnection
:passengerConnection rdf:type owl:ObjectProperty ;
                     rdfs:subPropertyOf :PROPS-TO-REVIEW .


###  https://w3id.org/mobility/transmodel/journeys#passesAt
:passesAt rdf:type owl:ObjectProperty .


###  https://w3id.org/mobility/transmodel/journeys#passingTimeTimingPoint
:passingTimeTimingPoint rdf:type owl:ObjectProperty ;
                        rdfs:subPropertyOf :PROPS-TO-REVIEW ;
                        rdfs:range :TimingPoint .


###  https://w3id.org/mobility/transmodel/journeys#prescribing
:prescribing rdf:type owl:ObjectProperty ;
             rdfs:subPropertyOf owl:topObjectProperty ;
             rdfs:domain :PointInJourneyPattern ;
             rdfs:range :DestinationDisplay .


###  https://w3id.org/mobility/transmodel/journeys#presentedBy
:presentedBy rdf:type owl:ObjectProperty ;
             rdfs:domain :Line ;
             rdfs:range <https://w3id.org/mobility/transmodel/commons#Presentation> .


###  https://w3id.org/mobility/transmodel/journeys#primarilyAdvertisedWith
:primarilyAdvertisedWith rdf:type owl:ObjectProperty ;
                         rdfs:subPropertyOf owl:topObjectProperty ;
                         rdfs:domain :JourneyPattern ;
                         rdfs:range :DestinationDisplay .


###  https://w3id.org/mobility/transmodel/journeys#routeOnLine
:routeOnLine rdf:type owl:ObjectProperty ;
             rdfs:subPropertyOf :PROPS-TO-REVIEW ;
             rdfs:range :Route .


###  https://w3id.org/mobility/transmodel/journeys#runBy
:runBy rdf:type owl:ObjectProperty ;
       rdfs:subPropertyOf owl:topObjectProperty ;
       rdfs:domain :Line ;
       rdfs:range <https://w3id.org/mobility/transmodel/organisations#Operator> .


###  https://w3id.org/mobility/transmodel/journeys#runTimeOverrides
:runTimeOverrides rdf:type owl:ObjectProperty ;
                  rdfs:subPropertyOf :PROPS-TO-REVIEW .


###  https://w3id.org/mobility/transmodel/journeys#runsOn
:runsOn rdf:type owl:ObjectProperty ;
        rdfs:domain :JourneyFrequencyGroup ;
        rdfs:range :VehicleJourney .


###  https://w3id.org/mobility/transmodel/journeys#scheduledStopPoint
:scheduledStopPoint rdf:type owl:ObjectProperty ;
                    rdfs:subPropertyOf :PROPS-TO-REVIEW ;
                    rdfs:domain :Route ;
                    rdfs:range :ScheduledStopPoint .


###  https://w3id.org/mobility/transmodel/journeys#season
:season rdf:type owl:ObjectProperty ;
        rdfs:range [ owl:intersectionOf ( <http://www.w3.org/2004/02/skos/core#Concept>
                                          [ rdf:type owl:Restriction ;
                                            owl:onProperty <http://www.w3.org/2004/02/skos/core#inScheme> ;
                                            owl:hasValue <https://w3id.org/mobility/transmodel/kos/journeys/day-type>
                                          ]
                                        ) ;
                     rdf:type owl:Class
                   ] .


###  https://w3id.org/mobility/transmodel/journeys#serviceJourneyUsingPattern
:serviceJourneyUsingPattern rdf:type owl:ObjectProperty ;
                            rdfs:subPropertyOf :PROPS-TO-REVIEW ;
                            rdfs:domain :ServiceJourney ;
                            rdfs:range :ServiceJourneyPattern .


###  https://w3id.org/mobility/transmodel/journeys#specifying
:specifying rdf:type owl:ObjectProperty ;
            rdfs:subPropertyOf owl:topObjectProperty ;
            rdfs:domain :DayTypeAssignment ;
            rdfs:range :DayType .


###  https://w3id.org/mobility/transmodel/journeys#startOf
:startOf rdf:type owl:ObjectProperty .


###  https://w3id.org/mobility/transmodel/journeys#startOfBlock
:startOfBlock rdf:type owl:ObjectProperty ;
              rdfs:domain :ParkingPoint ;
              rdfs:range :Block .


###  https://w3id.org/mobility/transmodel/journeys#startingAt
:startingAt rdf:type owl:ObjectProperty ;
            rdfs:domain :OperatingPeriod ;
            rdfs:range :OperatingDay .


###  https://w3id.org/mobility/transmodel/journeys#stopUse
:stopUse rdf:type owl:ObjectProperty ;
         rdfs:subPropertyOf owl:topObjectProperty ;
         rdfs:domain :StopPointInJourneyPattern ;
         rdfs:range [ owl:intersectionOf ( <http://www.w3.org/2004/02/skos/core#Concept>
                                           [ rdf:type owl:Restriction ;
                                             owl:onProperty <http://www.w3.org/2004/02/skos/core#inScheme> ;
                                             owl:hasValue <https://w3id.org/mobility/transmodel/kos/journeys/stop-use-type>
                                           ]
                                         ) ;
                      rdf:type owl:Class
                    ] .


###  https://w3id.org/mobility/transmodel/journeys#stopsAt
:stopsAt rdf:type owl:ObjectProperty ;
         rdfs:subPropertyOf :PROPS-TO-REVIEW ;
         rdfs:range :ScheduledStopPoint .


###  https://w3id.org/mobility/transmodel/journeys#timedFrom
:timedFrom rdf:type owl:ObjectProperty .


###  https://w3id.org/mobility/transmodel/journeys#timingLink
:timingLink rdf:type owl:ObjectProperty ;
            rdfs:subPropertyOf :PROPS-TO-REVIEW ;
            rdfs:range :TimingPoint .


###  https://w3id.org/mobility/transmodel/journeys#timingLinkInJourneyPattern
:timingLinkInJourneyPattern rdf:type owl:ObjectProperty ;
                            rdfs:subPropertyOf :PROPS-TO-REVIEW ;
                            rdfs:domain :JourneyPattern .


###  https://w3id.org/mobility/transmodel/journeys#typeOfFlexibleService
:typeOfFlexibleService rdf:type owl:ObjectProperty ;
                       rdfs:subPropertyOf :PROPS-TO-REVIEW .


###  https://w3id.org/mobility/transmodel/journeys#usedToDefine
:usedToDefine rdf:type owl:ObjectProperty ;
              rdfs:subPropertyOf owl:topObjectProperty ;
              rdfs:domain :OperatingDay ;
              rdfs:range :DayTypeAssignment .


###  https://w3id.org/mobility/transmodel/journeys#vehicleJourney
:vehicleJourney rdf:type owl:ObjectProperty ;
                rdfs:subPropertyOf :PROPS-TO-REVIEW ;
                rdfs:range :VehicleJourney .


###  https://w3id.org/mobility/transmodel/journeys#vehicleJourneyPart
:vehicleJourneyPart rdf:type owl:ObjectProperty ;
                    rdfs:subPropertyOf :PROPS-TO-REVIEW .


###  https://w3id.org/mobility/transmodel/journeys#vehicleJourneyRoute
:vehicleJourneyRoute rdf:type owl:ObjectProperty ;
                     rdfs:subPropertyOf :PROPS-TO-REVIEW ;
                     rdfs:domain :VehicleJourney ;
                     rdfs:range :Route .


###  https://w3id.org/mobility/transmodel/journeys#vehicleJourneyRunTimeOverrides
:vehicleJourneyRunTimeOverrides rdf:type owl:ObjectProperty ;
                                rdfs:subPropertyOf :PROPS-TO-REVIEW .


###  https://w3id.org/mobility/transmodel/journeys#vehicleJourneys
:vehicleJourneys rdf:type owl:ObjectProperty ;
                 rdfs:subPropertyOf :PROPS-TO-REVIEW ;
                 rdfs:range :VehicleJourney .


###  https://w3id.org/mobility/transmodel/journeys#vehicleModeId
:vehicleModeId rdf:type owl:ObjectProperty ;
               rdfs:domain :VehicleMode ;
               rdfs:range [ owl:intersectionOf ( <http://www.w3.org/2004/02/skos/core#Concept>
                                                 [ rdf:type owl:Restriction ;
                                                   owl:onProperty <http://www.w3.org/2004/02/skos/core#inScheme> ;
                                                   owl:hasValue <https://w3id.org/mobility/transmodel/kos/journeys/day-type>
                                                 ]
                                               ) ;
                            rdf:type owl:Class
                          ] .


###  https://w3id.org/mobility/transmodel/journeys#vehiclePassingTime
:vehiclePassingTime rdf:type owl:ObjectProperty ;
                    rdfs:subPropertyOf :PROPS-TO-REVIEW .


###  https://w3id.org/mobility/transmodel/journeys#viewedAs
:viewedAs rdf:type owl:ObjectProperty ;
          rdfs:subPropertyOf owl:topObjectProperty ;
          rdf:type owl:FunctionalProperty ;
          rdfs:domain :PointInLinkSequence ;
          rdfs:range <https://w3id.org/mobility/transmodel/commons#Point> .


###  https://w3id.org/mobility/transmodel/journeys#workedOn
:workedOn rdf:type owl:ObjectProperty ;
          rdfs:domain :VehicleJourney ;
          rdfs:range :DayType .


###  https://w3id.org/mobility/transmodel/commons#aClasificationFor
<https://w3id.org/mobility/transmodel/commons#aClasificationFor> rdf:type owl:ObjectProperty ;
                                                        rdfs:domain <https://w3id.org/mobility/transmodel/commons#Mode> ;
                                                        rdfs:range <https://w3id.org/mobility/transmodel/commons#SubMode> .


###  https://w3id.org/mobility/transmodel/commons#accessMode
<https://w3id.org/mobility/transmodel/commons#accessMode> rdf:type owl:ObjectProperty ;
                                                 rdfs:subPropertyOf <https://w3id.org/mobility/transmodel/commons#transportType> .


###  https://w3id.org/mobility/transmodel/commons#at
<https://w3id.org/mobility/transmodel/commons#at> rdf:type owl:ObjectProperty ;
                                         rdfs:subPropertyOf owl:topObjectProperty .


###  https://w3id.org/mobility/transmodel/commons#clasifiedAs
<https://w3id.org/mobility/transmodel/commons#clasifiedAs> rdf:type owl:ObjectProperty ;
                                                  rdfs:domain <https://w3id.org/mobility/transmodel/facilities#VehicleType> ;
                                                  rdfs:range <https://w3id.org/mobility/transmodel/commons#Vehicle> ,
                                                             <https://w3id.org/mobility/transmodel/commons#VehicleModel> .


###  https://w3id.org/mobility/transmodel/commons#in
<https://w3id.org/mobility/transmodel/commons#in> rdf:type owl:ObjectProperty ;
                                         rdfs:subPropertyOf owl:topObjectProperty .


###  https://w3id.org/mobility/transmodel/commons#representationFor
<https://w3id.org/mobility/transmodel/commons#representationFor> rdf:type owl:ObjectProperty .


###  https://w3id.org/mobility/transmodel/commons#representedBy
<https://w3id.org/mobility/transmodel/commons#representedBy> rdf:type owl:ObjectProperty ;
                                                    rdfs:domain <https://w3id.org/mobility/transmodel/commons#Zone> ;
                                                    rdfs:range <https://w3id.org/mobility/transmodel/commons#Point> .


###  https://w3id.org/mobility/transmodel/commons#transportType
<https://w3id.org/mobility/transmodel/commons#transportType> rdf:type owl:ObjectProperty .


###  https://w3id.org/mobility/transmodel/commons#vehicleMode
<https://w3id.org/mobility/transmodel/commons#vehicleMode> rdf:type owl:ObjectProperty ;
                                                  rdfs:subPropertyOf <https://w3id.org/mobility/transmodel/commons#transportType> .


###  https://w3id.org/mobility/transmodel/facilities#defining
<https://w3id.org/mobility/transmodel/facilities#defining> rdf:type owl:ObjectProperty ;
                                                  rdfs:domain <https://w3id.org/mobility/transmodel/facilities#PurposeOfEquipmentProfile> ;
                                                  rdfs:range <https://w3id.org/mobility/transmodel/facilities#VehicleEquipmentProfile> .


###  https://w3id.org/mobility/transmodel/facilities#equippedWith
<https://w3id.org/mobility/transmodel/facilities#equippedWith> rdf:type owl:ObjectProperty ;
                                                      rdfs:domain <https://w3id.org/mobility/transmodel/commons#Vehicle> ;
                                                      rdfs:range <https://w3id.org/mobility/transmodel/facilities#ActualVehilceEquipment> .


###  https://w3id.org/mobility/transmodel/facilities#journeyPatternAdvertisedFor
<https://w3id.org/mobility/transmodel/facilities#journeyPatternAdvertisedFor> rdf:type owl:ObjectProperty ;
                                                                     rdfs:subPropertyOf :PROPS-TO-REVIEW ;
                                                                     rdfs:range :DestinationDisplay .


###  https://w3id.org/mobility/transmodel/facilities#suitable
<https://w3id.org/mobility/transmodel/facilities#suitable> rdf:type owl:ObjectProperty ;
                                                  rdfs:domain <https://w3id.org/mobility/transmodel/facilities#ActualVehilceEquipment> ;
                                                  rdfs:range <https://w3id.org/mobility/transmodel/facilities#AccessibilityAssessment> .


###  https://w3id.org/mobility/transmodel/organisations#passengerJourney
<https://w3id.org/mobility/transmodel/organisations#passengerJourney> rdf:type owl:ObjectProperty ;
                                                             rdfs:subPropertyOf :PROPS-TO-REVIEW .


###  https://w3id.org/mobility/transmodel/organisations#serviceJourneyServedByVehicleJourney
<https://w3id.org/mobility/transmodel/organisations#serviceJourneyServedByVehicleJourney> rdf:type owl:ObjectProperty ;
                                                                                 rdfs:subPropertyOf :PROPS-TO-REVIEW ;
                                                                                 rdfs:domain :ServiceJourney ;
                                                                                 rdfs:range :VehicleJourney .


###  https://w3id.org/mobility/transmodel/organisations#trip
<https://w3id.org/mobility/transmodel/organisations#trip> rdf:type owl:ObjectProperty ;
                                                 rdfs:subPropertyOf :PROPS-TO-REVIEW ;
                                                 rdfs:range :ServiceJourney .


#################################################################
#    Data properties
#################################################################

###  http://purl.org/dc/terms/identifier
<http://purl.org/dc/terms/identifier> rdf:type owl:DatatypeProperty ;
                                      rdfs:range xsd:string .


###  http://schema.org/url
<http://schema.org/url> rdf:type owl:DatatypeProperty ;
                        rdfs:range xsd:string .


###  http://www.w3.org/2000/01/rdf-schema#comment
rdfs:comment rdf:type owl:DatatypeProperty .


###  http://www.w3.org/2000/01/rdf-schema#label
rdfs:label rdf:type owl:DatatypeProperty .


###  https://w3id.org/mobility/transmodel/journeys#BorderCrossingPoint
:BorderCrossingPoint rdf:type owl:DatatypeProperty ;
                     rdfs:domain :StopPlace ;
                     rdfs:range xsd:boolean ;
                     rdfs:comment "whether stop place is a border crossing."@en .


###  https://w3id.org/mobility/transmodel/journeys#DATA-PROPERTIES-TO-REVIEW
:DATA-PROPERTIES-TO-REVIEW rdf:type owl:DatatypeProperty .


###  https://w3id.org/mobility/transmodel/journeys#arrivalDayOffset
:arrivalDayOffset rdf:type owl:DatatypeProperty ;
                  rdfs:range xsd:time .


###  https://w3id.org/mobility/transmodel/journeys#arrivalTime
:arrivalTime rdf:type owl:DatatypeProperty ;
             rdfs:range xsd:time .


###  https://w3id.org/mobility/transmodel/journeys#atCentre
:atCentre rdf:type owl:DatatypeProperty ;
          rdfs:domain :ScheduledStopPoint ;
          rdfs:range xsd:boolean ;
          rdfs:comment "whether stop point can be considered as being at the centre of a topographic place.  default is false."@en .


###  https://w3id.org/mobility/transmodel/journeys#changeOfDestinationDisplay
:changeOfDestinationDisplay rdf:type owl:DatatypeProperty ;
                            rdfs:subPropertyOf owl:topDataProperty ;
                            rdfs:domain :StopPointInJourneyPattern ;
                            rdfs:range xsd:boolean .


###  https://w3id.org/mobility/transmodel/journeys#changeOfServiceRequirements
:changeOfServiceRequirements rdf:type owl:DatatypeProperty ;
                             rdfs:subPropertyOf owl:topDataProperty ;
                             rdfs:domain :StopPointInJourneyPattern ;
                             rdfs:range xsd:boolean .


###  https://w3id.org/mobility/transmodel/journeys#date
:date rdf:type owl:DatatypeProperty ;
      rdfs:subPropertyOf owl:topDataProperty ;
      rdfs:domain :DayTypeAssignment ;
      rdfs:range xsd:dateTimeStamp .


###  https://w3id.org/mobility/transmodel/journeys#departureDayOffset
:departureDayOffset rdf:type owl:DatatypeProperty ;
                    rdfs:range xsd:time .


###  https://w3id.org/mobility/transmodel/journeys#departureTime
:departureTime rdf:type owl:DatatypeProperty ;
               rdfs:range xsd:time .


###  https://w3id.org/mobility/transmodel/journeys#distance
:distance rdf:type owl:DatatypeProperty ;
          rdfs:domain :LinkSequence ;
          rdfs:range xsd:float .


###  https://w3id.org/mobility/transmodel/journeys#distanceFromStart
:distanceFromStart rdf:type owl:DatatypeProperty ;
                   rdfs:range xsd:float .


###  https://w3id.org/mobility/transmodel/journeys#dynamic
:dynamic rdf:type owl:DatatypeProperty ;
         rdfs:range xsd:boolean ;
         rdfs:comment "when this journey should be visible to public in dynamic channels."@en .


###  https://w3id.org/mobility/transmodel/journeys#firstDayOffset
:firstDayOffset rdf:type owl:DatatypeProperty ;
                rdfs:domain :JourneyFrequencyGroup ;
                rdfs:range xsd:integer .


###  https://w3id.org/mobility/transmodel/journeys#firstDepartureTime
:firstDepartureTime rdf:type owl:DatatypeProperty ;
                    rdfs:domain :JourneyFrequencyGroup ;
                    rdfs:range xsd:time .


###  https://w3id.org/mobility/transmodel/journeys#forAlighting
:forAlighting rdf:type owl:DatatypeProperty ;
              rdfs:subPropertyOf owl:topDataProperty ;
              rdfs:domain :StopPointInJourneyPattern ;
              rdfs:range xsd:boolean .


###  https://w3id.org/mobility/transmodel/journeys#forBoarding
:forBoarding rdf:type owl:DatatypeProperty ;
             rdfs:subPropertyOf owl:topDataProperty ;
             rdfs:domain :StopPointInJourneyPattern ;
             rdfs:range xsd:boolean .


###  https://w3id.org/mobility/transmodel/journeys#hasLiftOrRamp
:hasLiftOrRamp rdf:type owl:DatatypeProperty ;
               rdfs:domain <https://w3id.org/mobility/transmodel/facilities#VehicleType> ;
               rdfs:range xsd:boolean ;
               rdfs:comment "Whether VEHICLE TYPE has lift or ramp for wheelchair access."@en .


###  https://w3id.org/mobility/transmodel/journeys#headway
:headway rdf:type owl:DatatypeProperty ;
         rdfs:subPropertyOf :DATA-PROPERTIES-TO-REVIEW ;
         rdfs:domain :JourneyPattern ,
                     :VehicleJourney ;
         rdfs:range xsd:dateTimeStamp .


###  https://w3id.org/mobility/transmodel/journeys#holidayType-old
:holidayType-old rdf:type owl:DatatypeProperty ;
                 rdfs:subPropertyOf owl:topDataProperty ;
                 rdfs:domain :OperatingPeriod .


###  https://w3id.org/mobility/transmodel/journeys#isAvailable
:isAvailable rdf:type owl:DatatypeProperty ;
             rdfs:subPropertyOf owl:topDataProperty ;
             rdfs:domain :DayTypeAssignment ;
             rdfs:range xsd:boolean .


###  https://w3id.org/mobility/transmodel/journeys#isFlexible
:isFlexible rdf:type owl:DatatypeProperty ;
            rdfs:domain :StopPointInJourneyPattern ;
            rdfs:range xsd:boolean .


###  https://w3id.org/mobility/transmodel/journeys#isServiceDay
:isServiceDay rdf:type owl:DatatypeProperty ;
              rdfs:domain :OrganisationDayType ;
              rdfs:range xsd:boolean .


###  https://w3id.org/mobility/transmodel/journeys#isWaitPoint
:isWaitPoint rdf:type owl:DatatypeProperty ;
             rdfs:subPropertyOf owl:topDataProperty ;
             rdf:type owl:FunctionalProperty ;
             rdfs:domain :TimingPointInJourneyPattern ;
             rdfs:range xsd:time .


###  https://w3id.org/mobility/transmodel/journeys#journeyDuration
:journeyDuration rdf:type owl:DatatypeProperty ;
                 rdfs:range xsd:float ;
                 rdfs:comment "duration of vehicle journey."@en .


###  https://w3id.org/mobility/transmodel/journeys#lastDayOffset
:lastDayOffset rdf:type owl:DatatypeProperty ;
               rdfs:domain :HeadwayJourneyGroup ;
               rdfs:range xsd:time .


###  https://w3id.org/mobility/transmodel/journeys#lastDepartureTime
:lastDepartureTime rdf:type owl:DatatypeProperty ;
                   rdfs:domain :HeadwayJourneyGroup ;
                   rdfs:range xsd:time .


###  https://w3id.org/mobility/transmodel/journeys#layover
:layover rdf:type owl:DatatypeProperty ;
         rdfs:subPropertyOf :DATA-PROPERTIES-TO-REVIEW ;
         rdfs:domain :JourneyPattern ,
                     :VehicleJourney ;
         rdfs:range xsd:dateTimeStamp .


###  https://w3id.org/mobility/transmodel/journeys#lineName
:lineName rdf:type owl:DatatypeProperty ;
          rdfs:subPropertyOf :DATA-PROPERTIES-TO-REVIEW ;
          rdfs:range rdfs:Literal .


###  https://w3id.org/mobility/transmodel/journeys#lineNumber
:lineNumber rdf:type owl:DatatypeProperty ;
            rdfs:subPropertyOf :DATA-PROPERTIES-TO-REVIEW ;
            rdfs:range xsd:nonNegativeInteger .


###  https://w3id.org/mobility/transmodel/journeys#lowFloor
:lowFloor rdf:type owl:DatatypeProperty ;
          rdfs:domain <https://w3id.org/mobility/transmodel/facilities#VehicleType> ;
          rdfs:range xsd:boolean ;
          rdfs:comment "Whether VEHICLE TYPE is low floor"@en .


###  https://w3id.org/mobility/transmodel/journeys#maximumHeadwayInterval
:maximumHeadwayInterval rdf:type owl:DatatypeProperty ;
                        rdfs:domain :HeadwayInterval ;
                        rdfs:range xsd:duration .


###  https://w3id.org/mobility/transmodel/journeys#minimumHeadwayInterval
:minimumHeadwayInterval rdf:type owl:DatatypeProperty ;
                        rdfs:domain :HeadwayInterval ;
                        rdfs:range xsd:duration .


###  https://w3id.org/mobility/transmodel/journeys#monitored
:monitored rdf:type owl:DatatypeProperty ;
           rdfs:subPropertyOf owl:topDataProperty ;
           rdfs:domain :Journey ;
           rdfs:range xsd:boolean .


###  https://w3id.org/mobility/transmodel/journeys#order
:order rdf:type owl:DatatypeProperty ;
       rdfs:subPropertyOf owl:topDataProperty ;
       rdfs:range xsd:nonNegativeInteger .


###  https://w3id.org/mobility/transmodel/journeys#positionOfTrainElement
:positionOfTrainElement rdf:type owl:DatatypeProperty ;
                        rdfs:domain :TrainStopAssignment ;
                        rdfs:range xsd:integer ;
                        rdfs:comment "The association of a TRAIN COMPONENT at a SCHEDULED STOP POINT with a specific STOP PLACE and also possibly a QUAY and BOARDING POSITION."@en .


###  https://w3id.org/mobility/transmodel/journeys#publicCode
:publicCode rdf:type owl:DatatypeProperty ;
            rdfs:domain :StopArea ;
            rdfs:range xsd:string ;
            rdfs:comment "public code for a stop area."@en .


###  https://w3id.org/mobility/transmodel/journeys#requestStop
:requestStop rdf:type owl:DatatypeProperty ;
             rdfs:subPropertyOf owl:topDataProperty ;
             rdfs:domain :StopPointInJourneyPattern ;
             rdfs:range xsd:boolean .


###  https://w3id.org/mobility/transmodel/journeys#reversingDirection
:reversingDirection rdf:type owl:DatatypeProperty ;
                    rdfs:domain <https://w3id.org/mobility/transmodel/facilities#VehicleType> ;
                    rdfs:range xsd:boolean ;
                    rdfs:comment "Whether  VEHICLE TYPE has a reversing direction."@en .


###  https://w3id.org/mobility/transmodel/journeys#runtime
:runtime rdf:type owl:DatatypeProperty ;
         rdfs:subPropertyOf :DATA-PROPERTIES-TO-REVIEW ;
         rdfs:domain :JourneyPattern ,
                     :VehicleJourney ;
         rdfs:range xsd:nonNegativeInteger .


###  https://w3id.org/mobility/transmodel/journeys#scheduledHeadwayInterval
:scheduledHeadwayInterval rdf:type owl:DatatypeProperty ;
                          rdfs:domain :HeadwayInterval ;
                          rdfs:range xsd:duration .


###  https://w3id.org/mobility/transmodel/journeys#seatingCapacity
:seatingCapacity rdf:type owl:DatatypeProperty ;
                 rdfs:domain <https://w3id.org/mobility/transmodel/facilities#VehicleType> ;
                 rdfs:range xsd:integer ;
                 rdfs:comment "Maximum number of seated passengers that can be carried by a Vehicle of this type"@en .


###  https://w3id.org/mobility/transmodel/journeys#selfPropelled
:selfPropelled rdf:type owl:DatatypeProperty ;
               rdfs:domain <https://w3id.org/mobility/transmodel/facilities#VehicleType> ;
               rdfs:range xsd:boolean ;
               rdfs:comment "Whether  VEHICLE TYPE is self-propelled."@en .


###  https://w3id.org/mobility/transmodel/journeys#specialClient
:specialClient rdf:type owl:DatatypeProperty ;
               rdfs:comment "client for special service."@en .


###  https://w3id.org/mobility/transmodel/journeys#specialPlaceCapacity
:specialPlaceCapacity rdf:type owl:DatatypeProperty ;
                      rdfs:domain <https://w3id.org/mobility/transmodel/facilities#VehicleType> ;
                      rdfs:range xsd:integer ;
                      rdfs:comment "Maximum number of  passengers needing special places  that can be carried by a Vehicle of this type"@en .


###  https://w3id.org/mobility/transmodel/journeys#standingCapacity
:standingCapacity rdf:type owl:DatatypeProperty ;
                  rdfs:domain <https://w3id.org/mobility/transmodel/facilities#VehicleType> ;
                  rdfs:range xsd:integer ;
                  rdfs:comment "Maximum number of standing passengers that can be carried by a Vehicle of this type"@en .


###  https://w3id.org/mobility/transmodel/journeys#startTime
:startTime rdf:type owl:DatatypeProperty ;
           rdfs:subPropertyOf :DATA-PROPERTIES-TO-REVIEW ;
           rdfs:range xsd:string .


###  https://w3id.org/mobility/transmodel/journeys#time
:time rdf:type owl:DatatypeProperty ;
      rdfs:subPropertyOf :DATA-PROPERTIES-TO-REVIEW ;
      rdfs:domain :TimingPoint ;
      rdfs:range xsd:dateTimeStamp .


###  https://w3id.org/mobility/transmodel/journeys#timeLink
:timeLink rdf:type owl:DatatypeProperty ;
          rdfs:subPropertyOf :DATA-PROPERTIES-TO-REVIEW ;
          rdfs:domain :TimingPoint ;
          rdfs:range xsd:nonNegativeInteger .


###  https://w3id.org/mobility/transmodel/journeys#timingLinkInJourneyPattern
:timingLinkInJourneyPattern rdf:type owl:DatatypeProperty ;
                            rdfs:subPropertyOf :DATA-PROPERTIES-TO-REVIEW .


###  https://w3id.org/mobility/transmodel/journeys#timingLinkPointSequence
:timingLinkPointSequence rdf:type owl:DatatypeProperty ;
                         rdfs:subPropertyOf :DATA-PROPERTIES-TO-REVIEW ;
                         rdfs:domain :TimingPoint ;
                         rdfs:range xsd:nonNegativeInteger .


###  https://w3id.org/mobility/transmodel/journeys#vehicleMode
:vehicleMode rdf:type owl:DatatypeProperty ;
             rdfs:domain :ServiceLink ;
             rdfs:range xsd:string .


###  https://w3id.org/mobility/transmodel/journeys#viaFlag
:viaFlag rdf:type owl:DatatypeProperty ;
         rdfs:domain :RoutePoint ;
         rdfs:range xsd:boolean .


###  https://w3id.org/mobility/transmodel/journeys#waitTime
:waitTime rdf:type owl:DatatypeProperty ;
          rdfs:subPropertyOf :DATA-PROPERTIES-TO-REVIEW ;
          rdfs:domain :JourneyPattern ,
                      :VehicleJourney ;
          rdfs:range xsd:string .


###  https://w3id.org/mobility/transmodel/journeys#wheelchairPlaceCapacity
:wheelchairPlaceCapacity rdf:type owl:DatatypeProperty ;
                         rdfs:domain <https://w3id.org/mobility/transmodel/facilities#VehicleType> ;
                         rdfs:range xsd:integer ;
                         rdfs:comment "Maximum number of  passengers needing special places  that can be carried by a Vehicle of this type"@en .


###  https://w3id.org/mobility/transmodel/commons#borderCrossing
<https://w3id.org/mobility/transmodel/commons#borderCrossing> rdf:type owl:DatatypeProperty .


###  https://w3id.org/mobility/transmodel/commons#driverDisplayText
<https://w3id.org/mobility/transmodel/commons#driverDisplayText> rdf:type owl:DatatypeProperty ;
                                                        rdfs:domain <https://w3id.org/mobility/transmodel/commons#DestinationDisplay> ;
                                                        rdfs:range xsd:string ;
                                                        rdfs:comment "Text to display  to DRIVER."@en .


###  https://w3id.org/mobility/transmodel/commons#frontText
<https://w3id.org/mobility/transmodel/commons#frontText> rdf:type owl:DatatypeProperty ;
                                                rdfs:domain <https://w3id.org/mobility/transmodel/commons#DestinationDisplay> ;
                                                rdfs:range xsd:string ;
                                                rdfs:comment "Front of vehicle  text associated of DESTINATION DISPLAY."@en .


###  https://w3id.org/mobility/transmodel/commons#sideText
<https://w3id.org/mobility/transmodel/commons#sideText> rdf:type owl:DatatypeProperty ;
                                               rdfs:domain <https://w3id.org/mobility/transmodel/commons#DestinationDisplay> ;
                                               rdfs:range xsd:string ;
                                               rdfs:comment "Text to display on  side of vehicle associated with DESTINATION DISPLAY."@en .


###  https://w3id.org/mobility/transmodel/commons#turnaroundDistance
<https://w3id.org/mobility/transmodel/commons#turnaroundDistance> rdf:type owl:DatatypeProperty ;
                                                         rdfs:domain <https://w3id.org/mobility/transmodel/commons#TurnStation> ;
                                                         rdfs:range xsd:float ;
                                                         rdfs:comment "A place (often a terminus)where a vehicle can reverse its direction (from a ROUTE to another of opposite DIRECTION)."@en .


###  https://w3id.org/mobility/transmodel/commons#viewedAs
<https://w3id.org/mobility/transmodel/commons#viewedAs> rdf:type owl:DatatypeProperty .


###  https://w3id.org/mobility/transmodel/core#capacity
<https://w3id.org/mobility/transmodel/core#capacity> rdf:type owl:DatatypeProperty ;
                                            rdfs:comment "Number of vehicles allowed at a given time at VEHICLE TYPE AT POINT."@en .


###  https://w3id.org/mobility/transmodel/core#overtakingWidth
<https://w3id.org/mobility/transmodel/core#overtakingWidth> rdf:type owl:DatatypeProperty ;
                                                   rdfs:domain <https://w3id.org/mobility/transmodel/core#OvertakingPossibility> ;
                                                   rdfs:range xsd:float ;
                                                   rdfs:comment "Width at overtaking point"@en .


###  https://w3id.org/mobility/transmodel/facilities#units
<https://w3id.org/mobility/transmodel/facilities#units> rdf:type owl:DatatypeProperty ;
                                               rdfs:domain <https://w3id.org/mobility/transmodel/facilities#VehicleEquipmentProfile> ;
                                               rdfs:range xsd:integer ;
                                               rdfs:comment "Units (number of instances of equipment), for  VEHICLE EQUIPMENT PROFILE."@en .


#################################################################
#    Classes
#################################################################

###  http://www.w3.org/2004/02/skos/core#Concept
<http://www.w3.org/2004/02/skos/core#Concept> rdf:type owl:Class .


###  http://www.w3.org/2004/02/skos/core#ConceptScheme
<http://www.w3.org/2004/02/skos/core#ConceptScheme> rdf:type owl:Class .


###  https://w3id.org/mobility/transmodel/journeys#ActivationPoint
:ActivationPoint rdf:type owl:Class ;
                 rdfs:subClassOf <https://w3id.org/mobility/transmodel/commons#Point> .


###  https://w3id.org/mobility/transmodel/journeys#BeaconPoint
:BeaconPoint rdf:type owl:Class ;
             rdfs:subClassOf <https://w3id.org/mobility/transmodel/commons#Point> .


###  https://w3id.org/mobility/transmodel/journeys#Block
:Block rdf:type owl:Class .


###  https://w3id.org/mobility/transmodel/journeys#BoardingPosition
:BoardingPosition rdf:type owl:Class .


###  https://w3id.org/mobility/transmodel/journeys#CompoundTrain
:CompoundTrain rdf:type owl:Class ;
               rdfs:subClassOf <https://w3id.org/mobility/transmodel/facilities#VehicleType> ,
                               [ rdf:type owl:Restriction ;
                                 owl:onProperty :composedOfVehicle ;
                                 owl:allValuesFrom :TrainInCompoundTrain
                               ] ;
               rdfs:comment "A VEHICLE TYPE composed of a sequence of more than one vehicles of the type TRAIN."@en .


###  https://w3id.org/mobility/transmodel/journeys#DatedBlock
:DatedBlock rdf:type owl:Class ;
            rdfs:subClassOf :Block .


###  https://w3id.org/mobility/transmodel/journeys#DatedVehicleJourney
:DatedVehicleJourney rdf:type owl:Class ;
                     rdfs:subClassOf :VehicleJourney .


###  https://w3id.org/mobility/transmodel/journeys#DayType
:DayType rdf:type owl:Class ;
         rdfs:subClassOf [ rdf:type owl:Restriction ;
                           owl:onProperty :describedBy ;
                           owl:allValuesFrom :PropertyOfDay
                         ] ,
                         [ rdf:type owl:Restriction ;
                           owl:onProperty :specifying ;
                           owl:allValuesFrom :DayType
                         ] ,
                         [ rdf:type owl:Restriction ;
                           owl:onProperty :season ;
                           owl:maxQualifiedCardinality "1"^^xsd:nonNegativeInteger ;
                           owl:onClass [ owl:intersectionOf ( <http://www.w3.org/2004/02/skos/core#Concept>
                                                              [ rdf:type owl:Restriction ;
                                                                owl:onProperty <http://www.w3.org/2004/02/skos/core#inScheme> ;
                                                                owl:hasValue <https://w3id.org/mobility/transmodel/kos/journeys/day-type>
                                                              ]
                                                            ) ;
                                         rdf:type owl:Class
                                       ]
                         ] .


###  https://w3id.org/mobility/transmodel/journeys#DayTypeAssignment
:DayTypeAssignment rdf:type owl:Class ;
                   rdfs:subClassOf [ rdf:type owl:Restriction ;
                                     owl:onProperty :operatingPeriod ;
                                     owl:allValuesFrom :OperatingPeriod
                                   ] .


###  https://w3id.org/mobility/transmodel/journeys#DeadRun
:DeadRun rdf:type owl:Class ;
         rdfs:subClassOf :VehicleJourney .


###  https://w3id.org/mobility/transmodel/journeys#DeadRunPattern
:DeadRunPattern rdf:type owl:Class ;
                rdfs:subClassOf :JourneyPattern .


###  https://w3id.org/mobility/transmodel/journeys#DestinationDisplay
:DestinationDisplay rdf:type owl:Class .


###  https://w3id.org/mobility/transmodel/journeys#DestinationDisplayVariant
:DestinationDisplayVariant rdf:type owl:Class ;
                           rdfs:subClassOf :DestinationDisplay .


###  https://w3id.org/mobility/transmodel/journeys#DynamicStopAssignment
:DynamicStopAssignment rdf:type owl:Class ;
                       rdfs:subClassOf :PassengerStopAssignment ,
                                       [ rdf:type owl:Restriction ;
                                         owl:onProperty :overriding ;
                                         owl:allValuesFrom :PassengerStopAssignment
                                       ] .


###  https://w3id.org/mobility/transmodel/journeys#FareDayType
:FareDayType rdf:type owl:Class ;
             rdfs:subClassOf :DayType .


###  https://w3id.org/mobility/transmodel/journeys#FarePointInJourneyPattern
:FarePointInJourneyPattern rdf:type owl:Class ;
                           rdfs:subClassOf :PointInJourneyPattern .


###  https://w3id.org/mobility/transmodel/journeys#FlexiblePoint
:FlexiblePoint rdf:type owl:Class ;
               rdfs:subClassOf <https://w3id.org/mobility/transmodel/commons#Point> .


###  https://w3id.org/mobility/transmodel/journeys#GaragePoint
:GaragePoint rdf:type owl:Class ;
             rdfs:subClassOf :ParkingPoint .


###  https://w3id.org/mobility/transmodel/journeys#GroupOfLinkSequences
:GroupOfLinkSequences rdf:type owl:Class ;
                      rdfs:subClassOf [ rdf:type owl:Restriction ;
                                        owl:onProperty :composedOfLink ;
                                        owl:qualifiedCardinality "1"^^xsd:nonNegativeInteger ;
                                        owl:onClass :LinkSequence
                                      ] ,
                                      [ rdf:type owl:Restriction ;
                                        owl:onProperty <http://purl.org/dc/terms/identifier> ;
                                        owl:someValuesFrom xsd:string
                                      ] .


###  https://w3id.org/mobility/transmodel/journeys#HeadwayInterval
:HeadwayInterval rdf:type owl:Class ;
                 rdfs:subClassOf [ rdf:type owl:Restriction ;
                                   owl:onProperty :maximumHeadwayInterval ;
                                   owl:maxQualifiedCardinality "1"^^xsd:nonNegativeInteger ;
                                   owl:onDataRange xsd:duration
                                 ] ,
                                 [ rdf:type owl:Restriction ;
                                   owl:onProperty :minimumHeadwayInterval ;
                                   owl:maxQualifiedCardinality "1"^^xsd:nonNegativeInteger ;
                                   owl:onDataRange xsd:duration
                                 ] ,
                                 [ rdf:type owl:Restriction ;
                                   owl:onProperty :scheduledHeadwayInterval ;
                                   owl:maxQualifiedCardinality "1"^^xsd:nonNegativeInteger ;
                                   owl:onDataRange xsd:duration
                                 ] .


###  https://w3id.org/mobility/transmodel/journeys#HeadwayJourneyGroup
:HeadwayJourneyGroup rdf:type owl:Class ;
                     rdfs:subClassOf :JourneyFrequencyGroup ,
                                     [ rdf:type owl:Restriction ;
                                       owl:onProperty :determinedBy ;
                                       owl:allValuesFrom :HeadwayInterval
                                     ] .


###  https://w3id.org/mobility/transmodel/journeys#InfrastructurePoint
:InfrastructurePoint rdf:type owl:Class ;
                     rdfs:subClassOf <https://w3id.org/mobility/transmodel/commons#Point> .


###  https://w3id.org/mobility/transmodel/journeys#Interchange
:Interchange rdf:type owl:Class ;
             rdfs:comment "The scheduled possibility for transfer of passengers at the same or different scheduled stop points."@en .


###  https://w3id.org/mobility/transmodel/journeys#Journey
:Journey rdf:type owl:Class .


###  https://w3id.org/mobility/transmodel/journeys#JourneyFrequencyGroup
:JourneyFrequencyGroup rdf:type owl:Class ;
                       rdfs:subClassOf [ rdf:type owl:Restriction ;
                                         owl:onProperty :composedOf ;
                                         owl:allValuesFrom :VehicleJourney
                                       ] ,
                                       [ rdf:type owl:Restriction ;
                                         owl:onProperty :firstDayOffset ;
                                         owl:allValuesFrom xsd:int
                                       ] ,
                                       [ rdf:type owl:Restriction ;
                                         owl:onProperty :firstDepartureTime ;
                                         owl:allValuesFrom xsd:time
                                       ] ,
                                       [ rdf:type owl:Restriction ;
                                         owl:onProperty :lastDayOffset ;
                                         owl:allValuesFrom xsd:int
                                       ] ,
                                       [ rdf:type owl:Restriction ;
                                         owl:onProperty :lastDepartureTime ;
                                         owl:allValuesFrom xsd:time
                                       ] .


###  https://w3id.org/mobility/transmodel/journeys#JourneyPattern
:JourneyPattern rdf:type owl:Class ;
                rdfs:subClassOf :LinkSequence ,
                                [ rdf:type owl:Restriction ;
                                  owl:onProperty :primarilyAdvertisedWith ;
                                  owl:allValuesFrom :DestinationDisplay
                                ] .


###  https://w3id.org/mobility/transmodel/journeys#Line
:Line rdf:type owl:Class ;
      rdfs:subClassOf [ rdf:type owl:Restriction ;
                        owl:onProperty :presentedBy ;
                        owl:allValuesFrom <https://w3id.org/mobility/transmodel/commons#Presentation>
                      ] ,
                      [ rdf:type owl:Restriction ;
                        owl:onProperty rdfs:comment ;
                        owl:someValuesFrom xsd:string
                      ] ,
                      [ rdf:type owl:Restriction ;
                        owl:onProperty rdfs:label ;
                        owl:someValuesFrom xsd:string
                      ] ,
                      [ rdf:type owl:Restriction ;
                        owl:onProperty <http://schema.org/url> ;
                        owl:maxQualifiedCardinality "1"^^xsd:nonNegativeInteger ;
                        owl:onDataRange xsd:string
                      ] .


###  https://w3id.org/mobility/transmodel/journeys#Link
:Link rdf:type owl:Class ;
      rdfs:subClassOf [ rdf:type owl:Restriction ;
                        owl:onProperty :endOf ;
                        owl:qualifiedCardinality "1"^^xsd:nonNegativeInteger ;
                        owl:onClass <https://w3id.org/mobility/transmodel/commons#Point>
                      ] ,
                      [ rdf:type owl:Restriction ;
                        owl:onProperty :startOf ;
                        owl:qualifiedCardinality "1"^^xsd:nonNegativeInteger ;
                        owl:onClass <https://w3id.org/mobility/transmodel/commons#Point>
                      ] .


###  https://w3id.org/mobility/transmodel/journeys#LinkInLinkSequence
:LinkInLinkSequence rdf:type owl:Class ;
                    rdfs:subClassOf [ rdf:type owl:Restriction ;
                                      owl:onProperty <http://purl.org/dc/terms/identifier> ;
                                      owl:someValuesFrom xsd:string
                                    ] .


###  https://w3id.org/mobility/transmodel/journeys#LinkSequence
:LinkSequence rdf:type owl:Class ;
              rdfs:subClassOf [ rdf:type owl:Restriction ;
                                owl:onProperty :madeUpOf ;
                                owl:allValuesFrom :LinkInLinkSequence
                              ] ,
                              [ rdf:type owl:Restriction ;
                                owl:onProperty :madeUpOf ;
                                owl:allValuesFrom :PointInLinkSequence
                              ] ,
                              [ rdf:type owl:Restriction ;
                                owl:onProperty rdfs:label ;
                                owl:someValuesFrom xsd:string
                              ] ,
                              [ rdf:type owl:Restriction ;
                                owl:onProperty :distance ;
                                owl:maxQualifiedCardinality "1"^^xsd:nonNegativeInteger ;
                                owl:onDataRange xsd:float
                              ] .


###  https://w3id.org/mobility/transmodel/journeys#MonitoredVehicleJourney
:MonitoredVehicleJourney rdf:type owl:Class ;
                         rdfs:subClassOf :VehicleJourney .


###  https://w3id.org/mobility/transmodel/journeys#OperatingDay
:OperatingDay rdf:type owl:Class .


###  https://w3id.org/mobility/transmodel/journeys#OperatingPeriod
:OperatingPeriod rdf:type owl:Class ;
                 rdfs:subClassOf [ rdf:type owl:Restriction ;
                                   owl:onProperty :endingAt ;
                                   owl:allValuesFrom :OperatingDay
                                 ] ,
                                 [ rdf:type owl:Restriction ;
                                   owl:onProperty :startingAt ;
                                   owl:allValuesFrom :OperatingDay
                                 ] .


###  https://w3id.org/mobility/transmodel/journeys#OperationalContext
:OperationalContext rdf:type owl:Class ;
                    rdfs:comment "Characterization of a set of operational objects, such as timing or links determined either by a department or by an organisational unit."@en .


###  https://w3id.org/mobility/transmodel/journeys#OrganisationDayType
:OrganisationDayType rdf:type owl:Class ;
                     rdfs:subClassOf :DayType ,
                                     [ rdf:type owl:Restriction ;
                                       owl:onProperty :isServiceDay ;
                                       owl:allValuesFrom xsd:boolean
                                     ] .


###  https://w3id.org/mobility/transmodel/journeys#ParkingPoint
:ParkingPoint rdf:type owl:Class ;
              rdfs:subClassOf :ReliefPoint ,
                              [ rdf:type owl:Restriction ;
                                owl:onProperty :endOfBlock ;
                                owl:allValuesFrom :Block
                              ] ,
                              [ rdf:type owl:Restriction ;
                                owl:onProperty :startOfBlock ;
                                owl:allValuesFrom :Block
                              ] .


###  https://w3id.org/mobility/transmodel/journeys#PassengerStopAssignment
:PassengerStopAssignment rdf:type owl:Class ;
                         rdfs:subClassOf :StopAssignment .


###  https://w3id.org/mobility/transmodel/journeys#PointInJourneyPattern
:PointInJourneyPattern rdf:type owl:Class ;
                       rdfs:subClassOf :PointInLinkSequence ,
                                       [ rdf:type owl:Restriction ;
                                         owl:onProperty :passesAt ;
                                         owl:allValuesFrom :TimetabledPassingTime
                                       ] ,
                                       [ rdf:type owl:Restriction ;
                                         owl:onProperty :prescribing ;
                                         owl:allValuesFrom :DestinationDisplay
                                       ] .


###  https://w3id.org/mobility/transmodel/journeys#PointInLinkSequence
:PointInLinkSequence rdf:type owl:Class ;
                     rdfs:subClassOf [ rdf:type owl:Restriction ;
                                       owl:onProperty :inLinkSequence ;
                                       owl:qualifiedCardinality "1"^^xsd:nonNegativeInteger ;
                                       owl:onClass :LinkSequence
                                     ] ,
                                     [ rdf:type owl:Restriction ;
                                       owl:onProperty :viewedAs ;
                                       owl:qualifiedCardinality "1"^^xsd:nonNegativeInteger ;
                                       owl:onClass <https://w3id.org/mobility/transmodel/commons#Point>
                                     ] ,
                                     [ rdf:type owl:Restriction ;
                                       owl:onProperty <http://purl.org/dc/terms/identifier> ;
                                       owl:someValuesFrom xsd:string
                                     ] ,
                                     [ rdf:type owl:Restriction ;
                                       owl:onProperty :distanceFromStart ;
                                       owl:qualifiedCardinality "1"^^xsd:nonNegativeInteger ;
                                       owl:onDataRange xsd:float
                                     ] ,
                                     [ rdf:type owl:Restriction ;
                                       owl:onProperty :order ;
                                       owl:qualifiedCardinality "1"^^xsd:nonNegativeInteger ;
                                       owl:onDataRange xsd:nonNegativeInteger
                                     ] .


###  https://w3id.org/mobility/transmodel/journeys#PointOnRoute
:PointOnRoute rdf:type owl:Class ;
              rdfs:subClassOf :PointInLinkSequence ,
                              [ rdf:type owl:Restriction ;
                                owl:onProperty <https://w3id.org/mobility/transmodel/commons#in> ;
                                owl:allValuesFrom :Route
                              ] ,
                              [ rdf:type owl:Restriction ;
                                owl:onProperty :inLinkSequence ;
                                owl:qualifiedCardinality "1"^^xsd:nonNegativeInteger ;
                                owl:onClass :Route
                              ] ,
                              [ rdf:type owl:Restriction ;
                                owl:onProperty :viewedAs ;
                                owl:qualifiedCardinality "1"^^xsd:nonNegativeInteger ;
                                owl:onClass :RoutePoint
                              ] .


###  https://w3id.org/mobility/transmodel/journeys#PropertyOfDay
:PropertyOfDay rdf:type owl:Class ;
               rdfs:subClassOf [ rdf:type owl:Restriction ;
                                 owl:onProperty :definedAs ;
                                 owl:allValuesFrom [ owl:intersectionOf ( <http://www.w3.org/2004/02/skos/core#Concept>
                                                                          [ rdf:type owl:Restriction ;
                                                                            owl:onProperty <http://www.w3.org/2004/02/skos/core#inScheme> ;
                                                                            owl:hasValue <https://w3id.org/mobility/transmodel/kos/journeys/day-type>
                                                                          ]
                                                                        ) ;
                                                     rdf:type owl:Class
                                                   ]
                               ] .


###  https://w3id.org/mobility/transmodel/journeys#RailwayJunction
:RailwayJunction rdf:type owl:Class ;
                 rdfs:subClassOf :InfrastructurePoint .


###  https://w3id.org/mobility/transmodel/journeys#ReliefPoint
:ReliefPoint rdf:type owl:Class ;
             rdfs:subClassOf :TimingPoint .


###  https://w3id.org/mobility/transmodel/journeys#RhythmicalJourneyGroup
:RhythmicalJourneyGroup rdf:type owl:Class ;
                        rdfs:subClassOf :JourneyFrequencyGroup ,
                                        [ rdf:type owl:Restriction ;
                                          owl:onProperty :defines ;
                                          owl:allValuesFrom :TemplateVehicleJourney
                                        ] .


###  https://w3id.org/mobility/transmodel/journeys#RoadJunction
:RoadJunction rdf:type owl:Class ;
              rdfs:subClassOf :InfrastructurePoint .


###  https://w3id.org/mobility/transmodel/journeys#Route
:Route rdf:type owl:Class ;
       rdfs:subClassOf :LinkSequence .


###  https://w3id.org/mobility/transmodel/journeys#RouteLink
:RouteLink rdf:type owl:Class ;
           rdfs:subClassOf :Link ,
                           [ rdf:type owl:Restriction ;
                             owl:onProperty :endOf ;
                             owl:qualifiedCardinality "1"^^xsd:nonNegativeInteger ;
                             owl:onClass :RoutePoint
                           ] ,
                           [ rdf:type owl:Restriction ;
                             owl:onProperty :startOf ;
                             owl:qualifiedCardinality "1"^^xsd:nonNegativeInteger ;
                             owl:onClass :RoutePoint
                           ] .


###  https://w3id.org/mobility/transmodel/journeys#RoutePoint
:RoutePoint rdf:type owl:Class ;
            rdfs:subClassOf <https://w3id.org/mobility/transmodel/commons#Point> ,
                            [ rdf:type owl:Restriction ;
                              owl:onProperty :aViewOf ;
                              owl:allValuesFrom <https://w3id.org/mobility/transmodel/commons#PointOnRoute>
                            ] ,
                            [ rdf:type owl:Restriction ;
                              owl:onProperty :viaFlag ;
                              owl:maxQualifiedCardinality "1"^^xsd:nonNegativeInteger ;
                              owl:onDataRange xsd:boolean
                            ] ,
                            [ rdf:type owl:Restriction ;
                              owl:onProperty <https://w3id.org/mobility/transmodel/commons#borderCrossing> ;
                              owl:maxQualifiedCardinality "1"^^xsd:nonNegativeInteger ;
                              owl:onDataRange xsd:boolean
                            ] .


###  https://w3id.org/mobility/transmodel/journeys#ScheduledStopPoint
:ScheduledStopPoint rdf:type owl:Class ;
                    rdfs:subClassOf <https://w3id.org/mobility/transmodel/commons#Point> ,
                                    [ rdf:type owl:Restriction ;
                                      owl:onProperty :aViewOf ;
                                      owl:allValuesFrom :StopPointInJourneyPattern
                                    ] ,
                                    [ rdf:type owl:Restriction ;
                                      owl:onProperty :atCentre ;
                                      owl:maxQualifiedCardinality "1"^^xsd:nonNegativeInteger ;
                                      owl:onDataRange xsd:boolean
                                    ] .


###  https://w3id.org/mobility/transmodel/journeys#ServiceJourney
:ServiceJourney rdf:type owl:Class ;
                rdfs:subClassOf :VehicleJourney ,
                                [ rdf:type owl:Restriction ;
                                  owl:onProperty :directionType_old ;
                                  owl:allValuesFrom [ owl:intersectionOf ( <http://www.w3.org/2004/02/skos/core#Concept>
                                                                           [ rdf:type owl:Restriction ;
                                                                             owl:onProperty <http://www.w3.org/2004/02/skos/core#inScheme> ;
                                                                             owl:hasValue <https://w3id.org/mobility/transmodel/kos/journeys/direction-type>
                                                                           ]
                                                                         ) ;
                                                      rdf:type owl:Class
                                                    ]
                                ] ,
                                [ rdf:type owl:Restriction ;
                                  owl:onProperty :madeUsing ;
                                  owl:allValuesFrom <https://w3id.org/mobility/transmodel/facilities#ServiceFacilitySet>
                                ] .


###  https://w3id.org/mobility/transmodel/journeys#ServiceJourneyInterchange
:ServiceJourneyInterchange rdf:type owl:Class ;
                           rdfs:subClassOf :Interchange ,
                                           [ rdf:type owl:Restriction ;
                                             owl:onProperty :endOf ;
                                             owl:allValuesFrom :ScheduledStopPoint
                                           ] ,
                                           [ rdf:type owl:Restriction ;
                                             owl:onProperty :startOf ;
                                             owl:allValuesFrom :ScheduledStopPoint
                                           ] ;
                           rdfs:comment "the scheduled possibility for transfer of passengers between two service journeys at the same or different scheduled stop points."@en .


###  https://w3id.org/mobility/transmodel/journeys#ServiceJourneyPattern
:ServiceJourneyPattern rdf:type owl:Class ;
                       rdfs:subClassOf :JourneyPattern .


###  https://w3id.org/mobility/transmodel/journeys#ServiceJourneyPatternInterchange
:ServiceJourneyPatternInterchange rdf:type owl:Class ;
                                  rdfs:subClassOf :Interchange ,
                                                  [ rdf:type owl:Restriction ;
                                                    owl:onProperty :endOf ;
                                                    owl:allValuesFrom :JourneyPattern
                                                  ] ,
                                                  [ rdf:type owl:Restriction ;
                                                    owl:onProperty :endOf ;
                                                    owl:allValuesFrom :ScheduledStopPoint
                                                  ] ,
                                                  [ rdf:type owl:Restriction ;
                                                    owl:onProperty :startOf ;
                                                    owl:allValuesFrom :JourneyPattern
                                                  ] ,
                                                  [ rdf:type owl:Restriction ;
                                                    owl:onProperty :startOf ;
                                                    owl:allValuesFrom :ScheduledStopPoint
                                                  ] ;
                                  rdfs:comment "A recognised/organised possibility for passengers to change public transport vehicles using two scheduled stop points (which may be identical) on two particular service journey patterns, including the maximum wait duration allowed and the standard to be aimed at. these may supersede the times given for the default interchange. schedulers may use this entity for synchronisation of journeys."@en .


###  https://w3id.org/mobility/transmodel/journeys#ServiceLink
:ServiceLink rdf:type owl:Class ;
             rdfs:subClassOf :Link ,
                             [ rdf:type owl:Restriction ;
                               owl:onProperty :vehicleMode ;
                               owl:maxQualifiedCardinality "1"^^xsd:nonNegativeInteger ;
                               owl:onDataRange xsd:string
                             ] ;
             rdfs:comment "A LINK between an ordered pair of SCHEDULED STOP POINTs."@en .


###  https://w3id.org/mobility/transmodel/journeys#SpecialService
:SpecialService rdf:type owl:Class ;
                rdfs:subClassOf :Journey ,
                                [ rdf:type owl:Restriction ;
                                  owl:onProperty :dynamic ;
                                  owl:maxQualifiedCardinality "1"^^xsd:nonNegativeInteger ;
                                  owl:onDataRange xsd:boolean
                                ] ,
                                [ rdf:type owl:Restriction ;
                                  owl:onProperty :journeyDuration ;
                                  owl:maxQualifiedCardinality "1"^^xsd:nonNegativeInteger ;
                                  owl:onDataRange xsd:float
                                ] ,
                                [ rdf:type owl:Restriction ;
                                  owl:onProperty :specialClient ;
                                  owl:maxQualifiedCardinality "1"^^xsd:nonNegativeInteger ;
                                  owl:onDataRange xsd:boolean
                                ] ;
                rdfs:comment "A work of a vehicle that is not planned in a classical way, i.e. that is generally not based on vehicle journeys using journey patterns. it involves specific characteristics (such as specific access rights) and/or may be operated under specific circumstances."@en .


###  https://w3id.org/mobility/transmodel/journeys#StopArea
:StopArea rdf:type owl:Class ;
          rdfs:subClassOf [ rdf:type owl:Restriction ;
                            owl:onProperty :publicCode ;
                            owl:maxQualifiedCardinality "1"^^xsd:nonNegativeInteger ;
                            owl:onDataRange xsd:string
                          ] .


###  https://w3id.org/mobility/transmodel/journeys#StopAssignment
:StopAssignment rdf:type owl:Class ;
                rdfs:subClassOf [ rdf:type owl:Restriction ;
                                  owl:onProperty :for ;
                                  owl:allValuesFrom [ rdf:type owl:Class ;
                                                      owl:unionOf ( :ScheduledStopPoint
                                                                    <https://w3id.org/mobility/transmodel/facilities#BoardingPosition>
                                                                    <https://w3id.org/mobility/transmodel/facilities#Quay>
                                                                    <https://w3id.org/mobility/transmodel/facilities#StopPlace>
                                                                  )
                                                    ]
                                ] .


###  https://w3id.org/mobility/transmodel/journeys#StopPlace
:StopPlace rdf:type owl:Class ;
           rdfs:subClassOf [ rdf:type owl:Restriction ;
                             owl:onProperty :BorderCrossingPoint ;
                             owl:maxQualifiedCardinality "1"^^xsd:nonNegativeInteger ;
                             owl:onDataRange xsd:boolean
                           ] ;
           rdfs:comment "A place comprising one or more locations where vehicles may stop and where passengers may board or leave vehicles or prepare their trip. A stop place will usually have one or more wellknown names."@en .


###  https://w3id.org/mobility/transmodel/journeys#StopPointInJourneyPattern
:StopPointInJourneyPattern rdf:type owl:Class ;
                           rdfs:subClassOf :PointInJourneyPattern ,
                                           [ rdf:type owl:Restriction ;
                                             owl:onProperty :inLinkSequence ;
                                             owl:qualifiedCardinality "1"^^xsd:nonNegativeInteger ;
                                             owl:onClass :JourneyPattern
                                           ] ,
                                           [ rdf:type owl:Restriction ;
                                             owl:onProperty :viewedAs ;
                                             owl:qualifiedCardinality "1"^^xsd:nonNegativeInteger ;
                                             owl:onClass :ScheduledStopPoint
                                           ] ,
                                           [ rdf:type owl:Restriction ;
                                             owl:onProperty :stopUse ;
                                             owl:maxQualifiedCardinality "1"^^xsd:nonNegativeInteger ;
                                             owl:onClass [ owl:intersectionOf ( <http://www.w3.org/2004/02/skos/core#Concept>
                                                                                [ rdf:type owl:Restriction ;
                                                                                  owl:onProperty <http://www.w3.org/2004/02/skos/core#inScheme> ;
                                                                                  owl:hasValue <https://w3id.org/mobility/transmodel/kos/journeys/stop-use-type>
                                                                                ]
                                                                              ) ;
                                                           rdf:type owl:Class
                                                         ]
                                           ] ,
                                           [ rdf:type owl:Restriction ;
                                             owl:onProperty :changeOfDestinationDisplay ;
                                             owl:maxQualifiedCardinality "1"^^xsd:nonNegativeInteger ;
                                             owl:onDataRange xsd:boolean
                                           ] ,
                                           [ rdf:type owl:Restriction ;
                                             owl:onProperty :changeOfServiceRequirements ;
                                             owl:maxQualifiedCardinality "1"^^xsd:nonNegativeInteger ;
                                             owl:onDataRange xsd:boolean
                                           ] ,
                                           [ rdf:type owl:Restriction ;
                                             owl:onProperty :forAlighting ;
                                             owl:maxQualifiedCardinality "1"^^xsd:nonNegativeInteger ;
                                             owl:onDataRange xsd:boolean
                                           ] ,
                                           [ rdf:type owl:Restriction ;
                                             owl:onProperty :forBoarding ;
                                             owl:maxQualifiedCardinality "1"^^xsd:nonNegativeInteger ;
                                             owl:onDataRange xsd:boolean
                                           ] ,
                                           [ rdf:type owl:Restriction ;
                                             owl:onProperty :isFlexible ;
                                             owl:maxQualifiedCardinality "1"^^xsd:nonNegativeInteger ;
                                             owl:onDataRange xsd:boolean
                                           ] ,
                                           [ rdf:type owl:Restriction ;
                                             owl:onProperty :requestStop ;
                                             owl:maxQualifiedCardinality "1"^^xsd:nonNegativeInteger ;
                                             owl:onDataRange xsd:boolean
                                           ] .


###  https://w3id.org/mobility/transmodel/journeys#TemplateServiceJourney
:TemplateServiceJourney rdf:type owl:Class ;
                        rdfs:subClassOf :ServiceJourney ,
                                        :TemplateVehicleJourney .


###  https://w3id.org/mobility/transmodel/journeys#TemplateVehicleJourney
:TemplateVehicleJourney rdf:type owl:Class ;
                        rdfs:subClassOf :VehicleJourney ,
                                        [ rdf:type owl:Restriction ;
                                          owl:onProperty :isDefinedBy ;
                                          owl:allValuesFrom :RhythmicalJourneyGroup
                                        ] .


###  https://w3id.org/mobility/transmodel/journeys#TimetabledPassingTime
:TimetabledPassingTime rdf:type owl:Class ;
                       rdfs:subClassOf [ rdf:type owl:Restriction ;
                                         owl:onProperty :passesAt ;
                                         owl:allValuesFrom :PointInJourneyPattern
                                       ] ,
                                       [ rdf:type owl:Restriction ;
                                         owl:onProperty :arrivalDayOffset ;
                                         owl:allValuesFrom xsd:time
                                       ] ,
                                       [ rdf:type owl:Restriction ;
                                         owl:onProperty :arrivalTime ;
                                         owl:allValuesFrom xsd:time
                                       ] ,
                                       [ rdf:type owl:Restriction ;
                                         owl:onProperty :departureDayOffset ;
                                         owl:allValuesFrom xsd:time
                                       ] ,
                                       [ rdf:type owl:Restriction ;
                                         owl:onProperty :departureTime ;
                                         owl:allValuesFrom xsd:time
                                       ] .


###  https://w3id.org/mobility/transmodel/journeys#TimetabledVehicleJourney
:TimetabledVehicleJourney rdf:type owl:Class ;
                          rdfs:subClassOf :VehicleJourney .


###  https://w3id.org/mobility/transmodel/journeys#TimingLink
:TimingLink rdf:type owl:Class ;
            rdfs:subClassOf :Link ,
                            [ rdf:type owl:Restriction ;
                              owl:onProperty :endOf ;
                              owl:qualifiedCardinality "1"^^xsd:nonNegativeInteger ;
                              owl:onClass :TimingPoint
                            ] ,
                            [ rdf:type owl:Restriction ;
                              owl:onProperty :startOf ;
                              owl:qualifiedCardinality "1"^^xsd:nonNegativeInteger ;
                              owl:onClass :TimingPoint
                            ] .


###  https://w3id.org/mobility/transmodel/journeys#TimingPoint
:TimingPoint rdf:type owl:Class ;
             rdfs:subClassOf <https://w3id.org/mobility/transmodel/commons#Point> ,
                             [ rdf:type owl:Restriction ;
                               owl:onProperty :aViewOf ;
                               owl:allValuesFrom :TimingPointInJourneyPattern
                             ] .


###  https://w3id.org/mobility/transmodel/journeys#TimingPointInJourneyPattern
:TimingPointInJourneyPattern rdf:type owl:Class ;
                             rdfs:subClassOf :PointInJourneyPattern ,
                                             [ rdf:type owl:Restriction ;
                                               owl:onProperty :viewedAs ;
                                               owl:qualifiedCardinality "1"^^xsd:nonNegativeInteger ;
                                               owl:onClass :TimingPoint
                                             ] ,
                                             [ rdf:type owl:Restriction ;
                                               owl:onProperty :isWaitPoint ;
                                               owl:allValuesFrom xsd:boolean
                                             ] .


###  https://w3id.org/mobility/transmodel/journeys#TrafficControlPoint
:TrafficControlPoint rdf:type owl:Class ;
                     rdfs:subClassOf <https://w3id.org/mobility/transmodel/commons#Point> .


###  https://w3id.org/mobility/transmodel/journeys#Train
:Train rdf:type owl:Class ;
       rdfs:subClassOf <https://w3id.org/mobility/transmodel/facilities#VehicleType> ,
                       [ rdf:type owl:Restriction ;
                         owl:onProperty :composedOfVehicle ;
                         owl:allValuesFrom :TrainComponet
                       ] ;
       rdfs:comment "A VEHICLE TYPE composed of TRAIN ELEMENTs in a certain order, i.e. of wagons assembled together and propelled by a locomotive or one of the wagons."@en .


###  https://w3id.org/mobility/transmodel/journeys#TrainComponet
:TrainComponet rdf:type owl:Class ;
               rdfs:comment "A specification of the order of TRAIN ELEMENTs in a TRAIN."@en .


###  https://w3id.org/mobility/transmodel/journeys#TrainElement
:TrainElement rdf:type owl:Class ;
              rdfs:comment "An elementary component of a TRAIN (e.g. wagon, locomotive)."@en .


###  https://w3id.org/mobility/transmodel/journeys#TrainInCompoundTrain
:TrainInCompoundTrain rdf:type owl:Class ;
                      rdfs:comment "The specification of the order of TRAINs in a COMPOUND TRAIN."@en .


###  https://w3id.org/mobility/transmodel/journeys#TrainNumber
:TrainNumber rdf:type owl:Class ;
             rdfs:comment "Specification of codes assigned to particular vehicle journeys when operated by trains or compound trains according to a functional purpose (passenger information, operation follow-up, etc)"@en .


###  https://w3id.org/mobility/transmodel/journeys#TrainStopAssignment
:TrainStopAssignment rdf:type owl:Class ;
                     rdfs:subClassOf :StopAssignment ,
                                     [ rdf:type owl:Restriction ;
                                       owl:onProperty :positionOfTrainElement ;
                                       owl:maxQualifiedCardinality "1"^^xsd:nonNegativeInteger ;
                                       owl:onDataRange xsd:integer
                                     ] ;
                     rdfs:comment "The association of a TRAIN COMPONENT at a SCHEDULED STOP POINT with a specific STOP PLACE and also possibly a QUAY and BOARDING POSITION."@en .


###  https://w3id.org/mobility/transmodel/journeys#VehicleJourney
:VehicleJourney rdf:type owl:Class ;
                rdfs:subClassOf :Journey ,
                                [ rdf:type owl:Restriction ;
                                  owl:onProperty :passesAt ;
                                  owl:allValuesFrom :TimetabledPassingTime
                                ] ,
                                [ rdf:type owl:Restriction ;
                                  owl:onProperty :runsOn ;
                                  owl:allValuesFrom :JourneyFrequencyGroup
                                ] ,
                                [ rdf:type owl:Restriction ;
                                  owl:onProperty <https://w3id.org/mobility/transmodel/commons#in> ;
                                  owl:allValuesFrom :Block
                                ] .


###  https://w3id.org/mobility/transmodel/journeys#VehicleMode
:VehicleMode rdf:type owl:Class ;
             rdfs:subClassOf <https://w3id.org/mobility/transmodel/commons#Mode> .


###  https://w3id.org/mobility/transmodel/journeys#WireJunction
:WireJunction rdf:type owl:Class ;
              rdfs:subClassOf :InfrastructurePoint .


###  https://w3id.org/mobility/transmodel/commons#AllowedLineDirection
<https://w3id.org/mobility/transmodel/commons#AllowedLineDirection> rdf:type owl:Class ;
                                                           rdfs:comment "An allowed DIRECTION that can be used on a given ROUTE. This can be used to validate the selection of allowed values."@en .


###  https://w3id.org/mobility/transmodel/commons#ComplexFeature
<https://w3id.org/mobility/transmodel/commons#ComplexFeature> rdf:type owl:Class ;
                                                     rdfs:subClassOf [ rdf:type owl:Restriction ;
                                                                       owl:onProperty <https://w3id.org/mobility/transmodel/commons#representationFor> ;
                                                                       owl:maxQualifiedCardinality "1"^^xsd:nonNegativeInteger ;
                                                                       owl:onClass <https://w3id.org/mobility/transmodel/commons#Point>
                                                                     ] ,
                                                                     [ rdf:type owl:Restriction ;
                                                                       owl:onProperty <http://purl.org/dc/terms/identifier> ;
                                                                       owl:maxQualifiedCardinality "1"^^xsd:nonNegativeInteger ;
                                                                       owl:onDataRange xsd:string
                                                                     ] .


###  https://w3id.org/mobility/transmodel/commons#DestinationDisplay
<https://w3id.org/mobility/transmodel/commons#DestinationDisplay> rdf:type owl:Class ;
                                                         rdfs:subClassOf [ rdf:type owl:Restriction ;
                                                                           owl:onProperty <https://w3id.org/mobility/transmodel/commons#driverDisplayText> ;
                                                                           owl:maxQualifiedCardinality "1"^^xsd:nonNegativeInteger ;
                                                                           owl:onDataRange xsd:string
                                                                         ] ,
                                                                         [ rdf:type owl:Restriction ;
                                                                           owl:onProperty <https://w3id.org/mobility/transmodel/commons#frontText> ;
                                                                           owl:maxQualifiedCardinality "1"^^xsd:nonNegativeInteger ;
                                                                           owl:onDataRange xsd:string
                                                                         ] ,
                                                                         [ rdf:type owl:Restriction ;
                                                                           owl:onProperty <https://w3id.org/mobility/transmodel/commons#sideText> ;
                                                                           owl:maxQualifiedCardinality "1"^^xsd:nonNegativeInteger ;
                                                                           owl:onDataRange xsd:string
                                                                         ] ;
                                                         rdfs:comment "An advertised destination of a specific JOURNEY PATTERN, usually displayed on a headsign or at other on-board locations."@en .


###  https://w3id.org/mobility/transmodel/commons#Direction
<https://w3id.org/mobility/transmodel/commons#Direction> rdf:type owl:Class ;
                                                rdfs:subClassOf [ rdf:type owl:Restriction ;
                                                                  owl:onProperty rdfs:label ;
                                                                  owl:maxQualifiedCardinality "1"^^xsd:nonNegativeInteger ;
                                                                  owl:onDataRange xsd:string
                                                                ] ;
                                                rdfs:comment "A classification for the general orientation of ROUTEs."@en .


###  https://w3id.org/mobility/transmodel/commons#GroupOfLines
<https://w3id.org/mobility/transmodel/commons#GroupOfLines> rdf:type owl:Class ;
                                                   rdfs:comment "A grouping of lines which will be commonly referenced for a specific purpose."@en .


###  https://w3id.org/mobility/transmodel/commons#InfrastructureLink
<https://w3id.org/mobility/transmodel/commons#InfrastructureLink> rdf:type owl:Class ;
                                                         rdfs:subClassOf :Link ,
                                                                         [ rdf:type owl:Restriction ;
                                                                           owl:onProperty :endOf ;
                                                                           owl:allValuesFrom :InfrastructurePoint
                                                                         ] ,
                                                                         [ rdf:type owl:Restriction ;
                                                                           owl:onProperty :startOf ;
                                                                           owl:allValuesFrom :InfrastructurePoint
                                                                         ] ;
                                                         rdfs:comment "A super-type including all LINKs of the physical network (e.g. RAILWAY ELEMENT)."@en .


###  https://w3id.org/mobility/transmodel/commons#Mode
<https://w3id.org/mobility/transmodel/commons#Mode> rdf:type owl:Class ;
                                           rdfs:subClassOf [ rdf:type owl:Restriction ;
                                                             owl:onProperty <https://w3id.org/mobility/transmodel/commons#aClasificationFor> ;
                                                             owl:allValuesFrom <https://w3id.org/mobility/transmodel/commons#SubMode>
                                                           ] ,
                                                           [ rdf:type owl:Restriction ;
                                                             owl:onProperty <https://w3id.org/mobility/transmodel/commons#transportType> ;
                                                             owl:allValuesFrom [ owl:intersectionOf ( <http://www.w3.org/2004/02/skos/core#Concept>
                                                                                                      [ rdf:type owl:Restriction ;
                                                                                                        owl:onProperty <http://www.w3.org/2004/02/skos/core#inScheme> ;
                                                                                                        owl:hasValue <https://w3id.org/mobility/transmodel/kos/commons/all-modes>
                                                                                                      ]
                                                                                                    ) ;
                                                                                 rdf:type owl:Class
                                                                               ]
                                                           ] ;
                                           rdfs:comment "Any means of transport."@en .


###  https://w3id.org/mobility/transmodel/commons#Network
<https://w3id.org/mobility/transmodel/commons#Network> rdf:type owl:Class ;
                                              rdfs:subClassOf <https://w3id.org/mobility/transmodel/commons#GroupOfLines> ,
                                                              [ rdf:type owl:Restriction ;
                                                                owl:onProperty rdfs:label ;
                                                                owl:someValuesFrom xsd:string
                                                              ] ;
                                              rdfs:comment "A named grouping of LINEs under which a transport network is known."@en .


###  https://w3id.org/mobility/transmodel/commons#Point
<https://w3id.org/mobility/transmodel/commons#Point> rdf:type owl:Class ;
                                            rdfs:subClassOf [ rdf:type owl:Restriction ;
                                                              owl:onProperty :presentedBy ;
                                                              owl:qualifiedCardinality "1"^^xsd:nonNegativeInteger ;
                                                              owl:onClass <https://w3id.org/mobility/transmodel/commons#Zone>
                                                            ] ;
                                            rdfs:comment "A 0-dimensional node of the network used for the spatial description of the network. POINTs may be located by a LOCATION in a given LOCATING SYSTEM."@en .


###  https://w3id.org/mobility/transmodel/commons#PointOnRoute
<https://w3id.org/mobility/transmodel/commons#PointOnRoute> rdf:type owl:Class ;
                                                   rdfs:subClassOf [ rdf:type owl:Restriction ;
                                                                     owl:onProperty rdfs:comment ;
                                                                     owl:maxQualifiedCardinality "1"^^xsd:nonNegativeInteger ;
                                                                     owl:onDataRange xsd:string
                                                                   ] ;
                                                   rdfs:comment "A POINT used to define the shape of a ROUTE through the network."@en .


###  https://w3id.org/mobility/transmodel/commons#Presentation
<https://w3id.org/mobility/transmodel/commons#Presentation> rdf:type owl:Class .


###  https://w3id.org/mobility/transmodel/commons#RailwayElement
<https://w3id.org/mobility/transmodel/commons#RailwayElement> rdf:type owl:Class ;
                                                     rdfs:subClassOf <https://w3id.org/mobility/transmodel/commons#InfrastructureLink> ;
                                                     rdfs:comment "A type of INFRASTRUCTURE LINK used to describe a railway network."@en .


###  https://w3id.org/mobility/transmodel/commons#RoadElement
<https://w3id.org/mobility/transmodel/commons#RoadElement> rdf:type owl:Class ;
                                                  rdfs:subClassOf <https://w3id.org/mobility/transmodel/commons#InfrastructureLink> ;
                                                  rdfs:comment "A type of INFRASTRUCTURE LINK used to describe a road network."@en .


###  https://w3id.org/mobility/transmodel/commons#SimpleFeature
<https://w3id.org/mobility/transmodel/commons#SimpleFeature> rdf:type owl:Class ;
                                                    rdfs:subClassOf [ rdf:type owl:Restriction ;
                                                                      owl:onProperty :viewedAs ;
                                                                      owl:maxQualifiedCardinality "1"^^xsd:nonNegativeInteger ;
                                                                      owl:onClass :Link
                                                                    ] ,
                                                                    [ rdf:type owl:Restriction ;
                                                                      owl:onProperty :viewedAs ;
                                                                      owl:maxQualifiedCardinality "1"^^xsd:nonNegativeInteger ;
                                                                      owl:onClass <https://w3id.org/mobility/transmodel/commons#Point>
                                                                    ] ,
                                                                    [ rdf:type owl:Restriction ;
                                                                      owl:onProperty :viewedAs ;
                                                                      owl:maxQualifiedCardinality "1"^^xsd:nonNegativeInteger ;
                                                                      owl:onClass <https://w3id.org/mobility/transmodel/commons#Zone>
                                                                    ] ,
                                                                    [ rdf:type owl:Restriction ;
                                                                      owl:onProperty <http://purl.org/dc/terms/identifier> ;
                                                                      owl:maxQualifiedCardinality "1"^^xsd:nonNegativeInteger ;
                                                                      owl:onDataRange xsd:string
                                                                    ] .


###  https://w3id.org/mobility/transmodel/commons#SubMode
<https://w3id.org/mobility/transmodel/commons#SubMode> rdf:type owl:Class ;
                                              rdfs:comment "A variant of a mode, as for instance international or domestic rail (rail being the MODE)."@en .


###  https://w3id.org/mobility/transmodel/commons#TurnStation
<https://w3id.org/mobility/transmodel/commons#TurnStation> rdf:type owl:Class ;
                                                  rdfs:subClassOf [ rdf:type owl:Restriction ;
                                                                    owl:onProperty <https://w3id.org/mobility/transmodel/commons#turnaroundDistance> ;
                                                                    owl:maxQualifiedCardinality "1"^^xsd:nonNegativeInteger ;
                                                                    owl:onDataRange xsd:float
                                                                  ] ;
                                                  rdfs:comment "A place (often a terminus)where a vehicle can reverse its direction (from a ROUTE to another of opposite DIRECTION)."@en .


###  https://w3id.org/mobility/transmodel/commons#ValidityCondition
<https://w3id.org/mobility/transmodel/commons#ValidityCondition> rdf:type owl:Class ;
                                                        rdfs:comment "Condition used in order to characterise a given version of a version frame. a validity condition consists of a parameter (e.g. date, triggering event, etc.) and its type of application  (e.g. for,  from,  until, etc.)."@en .


###  https://w3id.org/mobility/transmodel/commons#Vehicle
<https://w3id.org/mobility/transmodel/commons#Vehicle> rdf:type owl:Class ;
                                              rdfs:subClassOf [ rdf:type owl:Restriction ;
                                                                owl:onProperty <https://w3id.org/mobility/transmodel/facilities#equippedWith> ;
                                                                owl:allValuesFrom <https://w3id.org/mobility/transmodel/facilities#ActualVehilceEquipment>
                                                              ] ;
                                              rdfs:comment "A public transport vehicle used for carrying passengers."@en .


###  https://w3id.org/mobility/transmodel/commons#VehicleModel
<https://w3id.org/mobility/transmodel/commons#VehicleModel> rdf:type owl:Class ;
                                                   rdfs:subClassOf [ rdf:type owl:Restriction ;
                                                                     owl:onProperty <https://w3id.org/mobility/transmodel/commons#clasifiedAs> ;
                                                                     owl:allValuesFrom <https://w3id.org/mobility/transmodel/commons#Vehicle>
                                                                   ] ;
                                                   rdfs:comment "A classification of public transport vehicles of the same VEHICLE TYPE, e.g. according to equipment specifications or model generation."@en .


###  https://w3id.org/mobility/transmodel/commons#Via
<https://w3id.org/mobility/transmodel/commons#Via> rdf:type owl:Class ;
                                          rdfs:subClassOf [ rdf:type owl:Restriction ;
                                                            owl:onProperty rdfs:label ;
                                                            owl:someValuesFrom xsd:string
                                                          ] ;
                                          rdfs:comment "A secondary heading relevant for a certain part of the JOURNEY PATTERN advertising an onward intermediate destination to supplement the advertised (final) destination of DESTINATION DISPLAY."@en .


###  https://w3id.org/mobility/transmodel/commons#WireElement
<https://w3id.org/mobility/transmodel/commons#WireElement> rdf:type owl:Class ;
                                                  rdfs:subClassOf <https://w3id.org/mobility/transmodel/commons#InfrastructureLink> ;
                                                  rdfs:comment "A type of INFRASTRUCTURE LINK used to describe a wire network."@en .


###  https://w3id.org/mobility/transmodel/commons#Zone
<https://w3id.org/mobility/transmodel/commons#Zone> rdf:type owl:Class ;
                                           rdfs:subClassOf [ rdf:type owl:Restriction ;
                                                             owl:onProperty <http://purl.org/dc/terms/identifier> ;
                                                             owl:someValuesFrom xsd:string
                                                           ] ,
                                                           [ rdf:type owl:Restriction ;
                                                             owl:onProperty rdfs:comment ;
                                                             owl:maxQualifiedCardinality "1"^^xsd:nonNegativeInteger ;
                                                             owl:onDataRange xsd:string
                                                           ] ,
                                                           [ rdf:type owl:Restriction ;
                                                             owl:onProperty rdfs:label ;
                                                             owl:maxQualifiedCardinality "1"^^xsd:nonNegativeInteger ;
                                                             owl:onDataRange xsd:string
                                                           ] .


###  https://w3id.org/mobility/transmodel/core#ImpossibleManoeuvre
<https://w3id.org/mobility/transmodel/core#ImpossibleManoeuvre> rdf:type owl:Class ;
                                                       rdfs:subClassOf <https://w3id.org/mobility/transmodel/core#NetworkRestrictions> ,
                                                                       [ rdf:type owl:Restriction ;
                                                                         owl:onProperty :endOf ;
                                                                         owl:allValuesFrom <https://w3id.org/mobility/transmodel/commons#InfrastructureLink>
                                                                       ] ,
                                                                       [ rdf:type owl:Restriction ;
                                                                         owl:onProperty :startOf ;
                                                                         owl:allValuesFrom <https://w3id.org/mobility/transmodel/commons#InfrastructureLink>
                                                                       ] ,
                                                                       [ rdf:type owl:Restriction ;
                                                                         owl:onProperty <http://purl.org/dc/terms/identifier> ;
                                                                         owl:someValuesFrom xsd:string
                                                                       ] ;
                                                       rdfs:comment "A specification of impossible move for a certain type of vehicle. It specifies from which INFRASTRUCTURE LINK to which other (adjacent) INFRASTRUCTURE LINK a certain VEHICLE TYPE cannot proceed, due to physical restrictions."@en .


###  https://w3id.org/mobility/transmodel/core#MeetingRestriction
<https://w3id.org/mobility/transmodel/core#MeetingRestriction> rdf:type owl:Class ;
                                                      rdfs:subClassOf <https://w3id.org/mobility/transmodel/core#NetworkRestrictions> ;
                                                      rdfs:comment "A pair of INFRASTRUCTURE LINKs where vehicles of specified VEHICLE TYPEs are not allowed to meet."@en .


###  https://w3id.org/mobility/transmodel/core#NetworkRestrictions
<https://w3id.org/mobility/transmodel/core#NetworkRestrictions> rdf:type owl:Class .


###  https://w3id.org/mobility/transmodel/core#OvertakingPossibility
<https://w3id.org/mobility/transmodel/core#OvertakingPossibility> rdf:type owl:Class ;
                                                         rdfs:subClassOf <https://w3id.org/mobility/transmodel/core#NetworkRestrictions> ,
                                                                         [ rdf:type owl:Restriction ;
                                                                           owl:onProperty <https://w3id.org/mobility/transmodel/core#overtakingWidth> ;
                                                                           owl:maxQualifiedCardinality "1"^^xsd:nonNegativeInteger ;
                                                                           owl:onDataRange xsd:float
                                                                         ] ;
                                                         rdfs:comment "NETWORK RESTRICTION specifying a POINT or a LINK where vehicles of specified VEHICLE TYPEs are or are  not allowed to overtake each other."@en .


###  https://w3id.org/mobility/transmodel/core#VehicleTypeAtPoint
<https://w3id.org/mobility/transmodel/core#VehicleTypeAtPoint> rdf:type owl:Class ;
                                                      rdfs:subClassOf <https://w3id.org/mobility/transmodel/core#NetworkRestrictions> ,
                                                                      [ rdf:type owl:Restriction ;
                                                                        owl:onProperty <https://w3id.org/mobility/transmodel/core#capacity> ;
                                                                        owl:maxQualifiedCardinality "1"^^xsd:nonNegativeInteger ;
                                                                        owl:onDataRange xsd:integer
                                                                      ] ;
                                                      rdfs:comment "The number of vehicles of a specified VEHICLE TYPE which may wait at a specified POINT at any one time. If the capacity is 0, then that type of vehicle may not stop there."@en .


###  https://w3id.org/mobility/transmodel/facilities#AccessibilityAssessment
<https://w3id.org/mobility/transmodel/facilities#AccessibilityAssessment> rdf:type owl:Class .


###  https://w3id.org/mobility/transmodel/facilities#ActualVehilceEquipment
<https://w3id.org/mobility/transmodel/facilities#ActualVehilceEquipment> rdf:type owl:Class ;
                                                                rdfs:subClassOf [ rdf:type owl:Restriction ;
                                                                                  owl:onProperty <https://w3id.org/mobility/transmodel/facilities#suitable> ;
                                                                                  owl:allValuesFrom <https://w3id.org/mobility/transmodel/facilities#AccessibilityAssessment>
                                                                                ] ;
                                                                rdfs:comment "Actual Vehicle Equipment"@en .


###  https://w3id.org/mobility/transmodel/facilities#BoardingPosition
<https://w3id.org/mobility/transmodel/facilities#BoardingPosition> rdf:type owl:Class .


###  https://w3id.org/mobility/transmodel/facilities#PurposeOfEquipmentProfile
<https://w3id.org/mobility/transmodel/facilities#PurposeOfEquipmentProfile> rdf:type owl:Class ;
                                                                   rdfs:subClassOf [ rdf:type owl:Restriction ;
                                                                                     owl:onProperty <https://w3id.org/mobility/transmodel/facilities#defining> ;
                                                                                     owl:allValuesFrom <https://w3id.org/mobility/transmodel/facilities#VehicleEquipmentProfile>
                                                                                   ] ,
                                                                                   [ rdf:type owl:Restriction ;
                                                                                     owl:onProperty <http://purl.org/dc/terms/identifier> ;
                                                                                     owl:someValuesFrom xsd:string
                                                                                   ] ;
                                                                   rdfs:comment "A functional purpose which requires a certain set of equipment of different types put together in a VEHICLE EQUIPMENT PROFILE."@en .


###  https://w3id.org/mobility/transmodel/facilities#Quay
<https://w3id.org/mobility/transmodel/facilities#Quay> rdf:type owl:Class .


###  https://w3id.org/mobility/transmodel/facilities#ServiceFacilitySet
<https://w3id.org/mobility/transmodel/facilities#ServiceFacilitySet> rdf:type owl:Class ;
                                                            rdfs:subClassOf [ rdf:type owl:Restriction ;
                                                                              owl:onProperty :madeUsing ;
                                                                              owl:allValuesFrom <https://w3id.org/mobility/transmodel/facilities#ServiceFacilitySet>
                                                                            ] .


###  https://w3id.org/mobility/transmodel/facilities#StopPlace
<https://w3id.org/mobility/transmodel/facilities#StopPlace> rdf:type owl:Class .


###  https://w3id.org/mobility/transmodel/facilities#VehicleEquipmentProfile
<https://w3id.org/mobility/transmodel/facilities#VehicleEquipmentProfile> rdf:type owl:Class ;
                                                                 rdfs:subClassOf [ rdf:type owl:Restriction ;
                                                                                   owl:onProperty <https://w3id.org/mobility/transmodel/facilities#units> ;
                                                                                   owl:maxQualifiedCardinality "1"^^xsd:nonNegativeInteger ;
                                                                                   owl:onDataRange xsd:integer
                                                                                 ] ;
                                                                 rdfs:comment "Each instantiation of this entity gives the number of items of one TYPE OF EQUIPMENT a VEHICLE MODEL should contain for a given PURPOSE OF EQUIPMENT PROFILE. The set of instantiations for one VEHICLE MODEL and one purpose gives one complete 'profile'."@en .


###  https://w3id.org/mobility/transmodel/facilities#VehicleType
<https://w3id.org/mobility/transmodel/facilities#VehicleType> rdf:type owl:Class ;
                                                     rdfs:subClassOf [ rdf:type owl:Restriction ;
                                                                       owl:onProperty <https://w3id.org/mobility/transmodel/commons#clasifiedAs> ;
                                                                       owl:allValuesFrom <https://w3id.org/mobility/transmodel/commons#Vehicle>
                                                                     ] ,
                                                                     [ rdf:type owl:Restriction ;
                                                                       owl:onProperty <https://w3id.org/mobility/transmodel/commons#clasifiedAs> ;
                                                                       owl:allValuesFrom <https://w3id.org/mobility/transmodel/commons#VehicleModel>
                                                                     ] ,
                                                                     [ rdf:type owl:Restriction ;
                                                                       owl:onProperty :hasLiftOrRamp ;
                                                                       owl:maxQualifiedCardinality "1"^^xsd:nonNegativeInteger ;
                                                                       owl:onDataRange xsd:boolean
                                                                     ] ,
                                                                     [ rdf:type owl:Restriction ;
                                                                       owl:onProperty :lowFloor ;
                                                                       owl:maxQualifiedCardinality "1"^^xsd:nonNegativeInteger ;
                                                                       owl:onDataRange xsd:boolean
                                                                     ] ,
                                                                     [ rdf:type owl:Restriction ;
                                                                       owl:onProperty :reversingDirection ;
                                                                       owl:maxQualifiedCardinality "1"^^xsd:nonNegativeInteger ;
                                                                       owl:onDataRange xsd:boolean
                                                                     ] ,
                                                                     [ rdf:type owl:Restriction ;
                                                                       owl:onProperty :seatingCapacity ;
                                                                       owl:maxQualifiedCardinality "1"^^xsd:nonNegativeInteger ;
                                                                       owl:onDataRange xsd:integer
                                                                     ] ,
                                                                     [ rdf:type owl:Restriction ;
                                                                       owl:onProperty :selfPropelled ;
                                                                       owl:maxQualifiedCardinality "1"^^xsd:nonNegativeInteger ;
                                                                       owl:onDataRange xsd:boolean
                                                                     ] ,
                                                                     [ rdf:type owl:Restriction ;
                                                                       owl:onProperty :specialPlaceCapacity ;
                                                                       owl:maxQualifiedCardinality "1"^^xsd:nonNegativeInteger ;
                                                                       owl:onDataRange xsd:integer
                                                                     ] ,
                                                                     [ rdf:type owl:Restriction ;
                                                                       owl:onProperty :standingCapacity ;
                                                                       owl:maxQualifiedCardinality "1"^^xsd:nonNegativeInteger ;
                                                                       owl:onDataRange xsd:integer
                                                                     ] ,
                                                                     [ rdf:type owl:Restriction ;
                                                                       owl:onProperty :wheelchairPlaceCapacity ;
                                                                       owl:maxQualifiedCardinality "1"^^xsd:nonNegativeInteger ;
                                                                       owl:onDataRange xsd:integer
                                                                     ] .


###  https://w3id.org/mobility/transmodel/organisations#Operator
<https://w3id.org/mobility/transmodel/organisations#Operator> rdf:type owl:Class .


#################################################################
#    Individuals
#################################################################

###  http://purl.org/dc/terms/identifier
<http://purl.org/dc/terms/identifier> rdf:type owl:NamedIndividual .


###  http://schema.org/url
<http://schema.org/url> rdf:type owl:NamedIndividual .


###  http://www.w3.org/2000/01/rdf-schema#comment
rdfs:comment rdf:type owl:NamedIndividual .


###  http://www.w3.org/2000/01/rdf-schema#label
rdfs:label rdf:type owl:NamedIndividual .


###  https://w3id.org/mobility/transmodel/journeys#Access
:Access rdf:type owl:NamedIndividual .


###  https://w3id.org/mobility/transmodel/journeys#AccessMode
:AccessMode rdf:type owl:NamedIndividual .


###  https://w3id.org/mobility/transmodel/journeys#AccessZone
:AccessZone rdf:type owl:NamedIndividual .


###  https://w3id.org/mobility/transmodel/journeys#ActivationPoint
:ActivationPoint rdf:type owl:NamedIndividual .


###  https://w3id.org/mobility/transmodel/journeys#Address
:Address rdf:type owl:NamedIndividual .


###  https://w3id.org/mobility/transmodel/journeys#AddressablePlace
:AddressablePlace rdf:type owl:NamedIndividual .


###  https://w3id.org/mobility/transmodel/journeys#AllowedLineDirections
:AllowedLineDirections rdf:type owl:NamedIndividual .


###  https://w3id.org/mobility/transmodel/journeys#BeaconPoint
:BeaconPoint rdf:type owl:NamedIndividual .


###  https://w3id.org/mobility/transmodel/journeys#Block
:Block rdf:type owl:NamedIndividual .


###  https://w3id.org/mobility/transmodel/journeys#BlockPart
:BlockPart rdf:type owl:NamedIndividual .


###  https://w3id.org/mobility/transmodel/journeys#BoardingPosition
:BoardingPosition rdf:type owl:NamedIndividual .


###  https://w3id.org/mobility/transmodel/journeys#BothDirections
:BothDirections rdf:type owl:NamedIndividual ;
                rdfs:label "BothDirections"@en .


###  https://w3id.org/mobility/transmodel/journeys#Bus
:Bus rdf:type owl:NamedIndividual ;
     rdfs:label "Bus"@en .


###  https://w3id.org/mobility/transmodel/journeys#CableCar
:CableCar rdf:type owl:NamedIndividual ;
          rdfs:label "CableCar"@en .


###  https://w3id.org/mobility/transmodel/journeys#CompoundBlock
:CompoundBlock rdf:type owl:NamedIndividual .


###  https://w3id.org/mobility/transmodel/journeys#Connection
:Connection rdf:type owl:NamedIndividual .


###  https://w3id.org/mobility/transmodel/journeys#CorridorService
:CorridorService rdf:type owl:NamedIndividual ;
                 rdfs:label "CorridorService"@en .


###  https://w3id.org/mobility/transmodel/journeys#CoupledJourney
:CoupledJourney rdf:type owl:NamedIndividual .


###  https://w3id.org/mobility/transmodel/journeys#CourseOfJourneys
:CourseOfJourneys rdf:type owl:NamedIndividual .


###  https://w3id.org/mobility/transmodel/journeys#DatedBlock
:DatedBlock rdf:type owl:NamedIndividual .


###  https://w3id.org/mobility/transmodel/journeys#DatedVehicleJourney
:DatedVehicleJourney rdf:type owl:NamedIndividual .


###  https://w3id.org/mobility/transmodel/journeys#DayType
:DayType rdf:type owl:NamedIndividual .


###  https://w3id.org/mobility/transmodel/journeys#DayTypeAssignment
:DayTypeAssignment rdf:type owl:NamedIndividual .


###  https://w3id.org/mobility/transmodel/journeys#DeadRun
:DeadRun rdf:type owl:NamedIndividual .


###  https://w3id.org/mobility/transmodel/journeys#DeadRunPattern
:DeadRunPattern rdf:type owl:NamedIndividual .


###  https://w3id.org/mobility/transmodel/journeys#DefaultConnection
:DefaultConnection rdf:type owl:NamedIndividual .


###  https://w3id.org/mobility/transmodel/journeys#DefaultDeadRunRunTime
:DefaultDeadRunRunTime rdf:type owl:NamedIndividual .


###  https://w3id.org/mobility/transmodel/journeys#DefaultInterchange
:DefaultInterchange rdf:type owl:NamedIndividual .


###  https://w3id.org/mobility/transmodel/journeys#DefaultInterchangeMaximum
:DefaultInterchangeMaximum rdf:type owl:NamedIndividual ;
                           rdfs:label "DefaultInterchangeStandard"@en .


###  https://w3id.org/mobility/transmodel/journeys#DefaultInterchangeStandard
:DefaultInterchangeStandard rdf:type owl:NamedIndividual ;
                            rdfs:label "DefaultInterchangeMaximum"@en .


###  https://w3id.org/mobility/transmodel/journeys#DefaultServiceJourneyRunTime
:DefaultServiceJourneyRunTime rdf:type owl:NamedIndividual .


###  https://w3id.org/mobility/transmodel/journeys#DestinationDisplay
:DestinationDisplay rdf:type owl:NamedIndividual .


###  https://w3id.org/mobility/transmodel/journeys#DestinationDisplayVariant
:DestinationDisplayVariant rdf:type owl:NamedIndividual .


###  https://w3id.org/mobility/transmodel/journeys#DynamicStopAssignment
:DynamicStopAssignment rdf:type owl:NamedIndividual .


###  https://w3id.org/mobility/transmodel/journeys#FareDayType
:FareDayType rdf:type owl:NamedIndividual .


###  https://w3id.org/mobility/transmodel/journeys#FarePointInJourneyPattern
:FarePointInJourneyPattern rdf:type owl:NamedIndividual .


###  https://w3id.org/mobility/transmodel/journeys#Ferry
:Ferry rdf:type owl:NamedIndividual ;
       rdfs:label "Ferry"@en .


###  https://w3id.org/mobility/transmodel/journeys#FixedStopAreaWideFlexibleService
:FixedStopAreaWideFlexibleService rdf:type owl:NamedIndividual ;
                                  rdfs:label "FixedStopAreaWideFlexibleService"@en .


###  https://w3id.org/mobility/transmodel/journeys#FlexibleLine
:FlexibleLine rdf:type owl:NamedIndividual .


###  https://w3id.org/mobility/transmodel/journeys#FlexiblePoint
:FlexiblePoint rdf:type owl:NamedIndividual .


###  https://w3id.org/mobility/transmodel/journeys#FlexibleRoute
:FlexibleRoute rdf:type owl:NamedIndividual .


###  https://w3id.org/mobility/transmodel/journeys#FlexibleServiceWithMainRoute
:FlexibleServiceWithMainRoute rdf:type owl:NamedIndividual ;
                              rdfs:label "FlexibleServiceWithMainRoute"@en .


###  https://w3id.org/mobility/transmodel/journeys#FreeAreaWideFlexibleService
:FreeAreaWideFlexibleService rdf:type owl:NamedIndividual ;
                             rdfs:label "FreeAreaWideFlexibleService"@en .


###  https://w3id.org/mobility/transmodel/journeys#Friday
:Friday rdf:type owl:NamedIndividual ;
        rdfs:label "Friday"@en .


###  https://w3id.org/mobility/transmodel/journeys#FromOriginToSSP
:FromOriginToSSP rdf:type owl:NamedIndividual .


###  https://w3id.org/mobility/transmodel/journeys#FromSSPtoDestination
:FromSSPtoDestination rdf:type owl:NamedIndividual .


###  https://w3id.org/mobility/transmodel/journeys#Funicular
:Funicular rdf:type owl:NamedIndividual ;
           rdfs:label "Funicular"@en .


###  https://w3id.org/mobility/transmodel/journeys#GaragePoint
:GaragePoint rdf:type owl:NamedIndividual .


###  https://w3id.org/mobility/transmodel/journeys#Gondola
:Gondola rdf:type owl:NamedIndividual ;
         rdfs:label "Gondola"@en .


###  https://w3id.org/mobility/transmodel/journeys#GroupOfLinkSequences
:GroupOfLinkSequences rdf:type owl:NamedIndividual .


###  https://w3id.org/mobility/transmodel/journeys#GroupOfTimingLinks
:GroupOfTimingLinks rdf:type owl:NamedIndividual .


###  https://w3id.org/mobility/transmodel/journeys#HeadwayInterval
:HeadwayInterval rdf:type owl:NamedIndividual .


###  https://w3id.org/mobility/transmodel/journeys#HeadwayJourneyGroup
:HeadwayJourneyGroup rdf:type owl:NamedIndividual .


###  https://w3id.org/mobility/transmodel/journeys#InfrastructurePoint
:InfrastructurePoint rdf:type owl:NamedIndividual .


###  https://w3id.org/mobility/transmodel/journeys#Journey
:Journey rdf:type owl:NamedIndividual .


###  https://w3id.org/mobility/transmodel/journeys#JourneyFrequencyGroup
:JourneyFrequencyGroup rdf:type owl:NamedIndividual .


###  https://w3id.org/mobility/transmodel/journeys#JourneyPart
:JourneyPart rdf:type owl:NamedIndividual .


###  https://w3id.org/mobility/transmodel/journeys#JourneyPartCouple
:JourneyPartCouple rdf:type owl:NamedIndividual .


###  https://w3id.org/mobility/transmodel/journeys#JourneyPattern
:JourneyPattern rdf:type owl:NamedIndividual .


###  https://w3id.org/mobility/transmodel/journeys#JourneyPatternLayover
:JourneyPatternLayover rdf:type owl:NamedIndividual .


###  https://w3id.org/mobility/transmodel/journeys#JourneyPatternRunTime
:JourneyPatternRunTime rdf:type owl:NamedIndividual .


###  https://w3id.org/mobility/transmodel/journeys#Line
:Line rdf:type owl:NamedIndividual .


###  https://w3id.org/mobility/transmodel/journeys#Line-old
:Line-old rdf:type owl:NamedIndividual .


###  https://w3id.org/mobility/transmodel/journeys#Link
:Link rdf:type owl:NamedIndividual .


###  https://w3id.org/mobility/transmodel/journeys#LinkInLinkSequence
:LinkInLinkSequence rdf:type owl:NamedIndividual .


###  https://w3id.org/mobility/transmodel/journeys#LinkSequence
:LinkSequence rdf:type owl:NamedIndividual .


###  https://w3id.org/mobility/transmodel/journeys#MeanOfTransport
:MeanOfTransport rdf:type owl:NamedIndividual .


###  https://w3id.org/mobility/transmodel/journeys#Metro
:Metro rdf:type owl:NamedIndividual ;
       rdfs:label "Metro"@en .


###  https://w3id.org/mobility/transmodel/journeys#MixedTypeOfFlexibleAndRegularServices
:MixedTypeOfFlexibleAndRegularServices rdf:type owl:NamedIndividual ;
                                       rdfs:label "MixedTypeOfFlexibleAndRegularServices"@en .


###  https://w3id.org/mobility/transmodel/journeys#MixedTypesOfFlexibleService
:MixedTypesOfFlexibleService rdf:type owl:NamedIndividual ;
                             rdfs:label "MixedTypesOfFlexibleService"@en .


###  https://w3id.org/mobility/transmodel/journeys#Monday
:Monday rdf:type owl:NamedIndividual ;
        rdfs:label "Monday"@en .


###  https://w3id.org/mobility/transmodel/journeys#MonitoredVehicleJourney
:MonitoredVehicleJourney rdf:type owl:NamedIndividual .


###  https://w3id.org/mobility/transmodel/journeys#OneDirection
:OneDirection rdf:type owl:NamedIndividual ;
              rdfs:label "OneDirection"@en .


###  https://w3id.org/mobility/transmodel/journeys#OperatingDay
:OperatingDay rdf:type owl:NamedIndividual .


###  https://w3id.org/mobility/transmodel/journeys#OperatingPeriod
:OperatingPeriod rdf:type owl:NamedIndividual .


###  https://w3id.org/mobility/transmodel/journeys#OrganisationDayType
:OrganisationDayType rdf:type owl:NamedIndividual .


###  https://w3id.org/mobility/transmodel/journeys#OtherDirections
:OtherDirections rdf:type owl:NamedIndividual ;
                 rdfs:label "OtherDirections"@en .


###  https://w3id.org/mobility/transmodel/journeys#OutboundRoute
:OutboundRoute rdf:type owl:NamedIndividual ;
               rdfs:label "Outbound"@en .


###  https://w3id.org/mobility/transmodel/journeys#ParkingPoint
:ParkingPoint rdf:type owl:NamedIndividual .


###  https://w3id.org/mobility/transmodel/journeys#PassengerStopAssignment
:PassengerStopAssignment rdf:type owl:NamedIndividual .


###  https://w3id.org/mobility/transmodel/journeys#Place
:Place rdf:type owl:NamedIndividual .


###  https://w3id.org/mobility/transmodel/journeys#PointInJourneyPattern
:PointInJourneyPattern rdf:type owl:NamedIndividual .


###  https://w3id.org/mobility/transmodel/journeys#PointInLinkSequence
:PointInLinkSequence rdf:type owl:NamedIndividual .


###  https://w3id.org/mobility/transmodel/journeys#PointOnRoute
:PointOnRoute rdf:type owl:NamedIndividual .


###  https://w3id.org/mobility/transmodel/journeys#PostalAddress
:PostalAddress rdf:type owl:NamedIndividual .


###  https://w3id.org/mobility/transmodel/journeys#PrivateBike
:PrivateBike rdf:type owl:NamedIndividual .


###  https://w3id.org/mobility/transmodel/journeys#PropertyOfDay
:PropertyOfDay rdf:type owl:NamedIndividual .


###  https://w3id.org/mobility/transmodel/journeys#Rail
:Rail rdf:type owl:NamedIndividual ;
      rdfs:label "Rail"@en .


###  https://w3id.org/mobility/transmodel/journeys#RailwayJunction
:RailwayJunction rdf:type owl:NamedIndividual .


###  https://w3id.org/mobility/transmodel/journeys#ReliefPoint
:ReliefPoint rdf:type owl:NamedIndividual .


###  https://w3id.org/mobility/transmodel/journeys#ReturnRoute
:ReturnRoute rdf:type owl:NamedIndividual ;
             rdfs:label "ReturnRoute"@en .


###  https://w3id.org/mobility/transmodel/journeys#RhythmicalJourneyGroup
:RhythmicalJourneyGroup rdf:type owl:NamedIndividual .


###  https://w3id.org/mobility/transmodel/journeys#RoadAddress
:RoadAddress rdf:type owl:NamedIndividual .


###  https://w3id.org/mobility/transmodel/journeys#RoadJunction
:RoadJunction rdf:type owl:NamedIndividual .


###  https://w3id.org/mobility/transmodel/journeys#RoundTrip
:RoundTrip rdf:type owl:NamedIndividual ;
           rdfs:label "RoundTrip"@en .


###  https://w3id.org/mobility/transmodel/journeys#Route
:Route rdf:type owl:NamedIndividual .


###  https://w3id.org/mobility/transmodel/journeys#RouteLink
:RouteLink rdf:type owl:NamedIndividual .


###  https://w3id.org/mobility/transmodel/journeys#RoutePoint
:RoutePoint rdf:type owl:NamedIndividual .


###  https://w3id.org/mobility/transmodel/journeys#Saturday
:Saturday rdf:type owl:NamedIndividual ;
          rdfs:label "Saturday"@en .


###  https://w3id.org/mobility/transmodel/journeys#ScheduledStopPoint
:ScheduledStopPoint rdf:type owl:NamedIndividual .


###  https://w3id.org/mobility/transmodel/journeys#ServiceCalendar
:ServiceCalendar rdf:type owl:NamedIndividual .


###  https://w3id.org/mobility/transmodel/journeys#ServiceJourney
:ServiceJourney rdf:type owl:NamedIndividual .


###  https://w3id.org/mobility/transmodel/journeys#ServiceJourneyPattern
:ServiceJourneyPattern rdf:type owl:NamedIndividual .


###  https://w3id.org/mobility/transmodel/journeys#StopArea
:StopArea rdf:type owl:NamedIndividual .


###  https://w3id.org/mobility/transmodel/journeys#StopAssignment
:StopAssignment rdf:type owl:NamedIndividual .


###  https://w3id.org/mobility/transmodel/journeys#StopPointInJourneyPattern
:StopPointInJourneyPattern rdf:type owl:NamedIndividual .


###  https://w3id.org/mobility/transmodel/journeys#Sunday
:Sunday rdf:type owl:NamedIndividual ;
        rdfs:label "Sunday"@en .


###  https://w3id.org/mobility/transmodel/journeys#TemplateServiceJourney
:TemplateServiceJourney rdf:type owl:NamedIndividual .


###  https://w3id.org/mobility/transmodel/journeys#TemplateVehicleJourney
:TemplateVehicleJourney rdf:type owl:NamedIndividual .


###  https://w3id.org/mobility/transmodel/journeys#Thursday
:Thursday rdf:type owl:NamedIndividual ;
          rdfs:label "Thursday"@en .


###  https://w3id.org/mobility/transmodel/journeys#TimeBand
:TimeBand rdf:type owl:NamedIndividual .


###  https://w3id.org/mobility/transmodel/journeys#TimeDemandType
:TimeDemandType rdf:type owl:NamedIndividual .


###  https://w3id.org/mobility/transmodel/journeys#TimetabledPassingTime
:TimetabledPassingTime rdf:type owl:NamedIndividual .


###  https://w3id.org/mobility/transmodel/journeys#TimetabledVehicleJourney
:TimetabledVehicleJourney rdf:type owl:NamedIndividual .


###  https://w3id.org/mobility/transmodel/journeys#TimingLink
:TimingLink rdf:type owl:NamedIndividual .


###  https://w3id.org/mobility/transmodel/journeys#TimingLinkInJourneyPattern
:TimingLinkInJourneyPattern rdf:type owl:NamedIndividual .


###  https://w3id.org/mobility/transmodel/journeys#TimingPoint
:TimingPoint rdf:type owl:NamedIndividual .


###  https://w3id.org/mobility/transmodel/journeys#TimingPointInJourneyPattern
:TimingPointInJourneyPattern rdf:type owl:NamedIndividual .


###  https://w3id.org/mobility/transmodel/journeys#TopographicPlace
:TopographicPlace rdf:type owl:NamedIndividual .


###  https://w3id.org/mobility/transmodel/journeys#TrafficControlPoint
:TrafficControlPoint rdf:type owl:NamedIndividual .


###  https://w3id.org/mobility/transmodel/journeys#Tram
:Tram rdf:type owl:NamedIndividual ;
      rdfs:label "Tram"@en .


###  https://w3id.org/mobility/transmodel/journeys#Trip
:Trip rdf:type owl:NamedIndividual .


###  https://w3id.org/mobility/transmodel/journeys#Tuesday
:Tuesday rdf:type owl:NamedIndividual ;
         rdfs:label "Tuesday"@en .


###  https://w3id.org/mobility/transmodel/journeys#Vehicle
:Vehicle rdf:type owl:NamedIndividual ;
         rdfs:label "Vehicle"@en .


###  https://w3id.org/mobility/transmodel/journeys#VehicleJourney
:VehicleJourney rdf:type owl:NamedIndividual .


###  https://w3id.org/mobility/transmodel/journeys#VehicleJourneyLayover
:VehicleJourneyLayover rdf:type owl:NamedIndividual .


###  https://w3id.org/mobility/transmodel/journeys#VehicleJourneyRunTime
:VehicleJourneyRunTime rdf:type owl:NamedIndividual .


###  https://w3id.org/mobility/transmodel/journeys#VehicleMode
:VehicleMode rdf:type owl:NamedIndividual .


###  https://w3id.org/mobility/transmodel/journeys#Walking
:Walking rdf:type owl:NamedIndividual .


###  https://w3id.org/mobility/transmodel/journeys#Wednesday
:Wednesday rdf:type owl:NamedIndividual ;
           rdfs:label "Wednesday"@en .


###  https://w3id.org/mobility/transmodel/journeys#WeekdayInSchoolHolidays
:WeekdayInSchoolHolidays rdf:type owl:NamedIndividual ;
                         rdfs:label "WeekdayInSchoolHolidays"@en .


###  https://w3id.org/mobility/transmodel/journeys#WireJunction
:WireJunction rdf:type owl:NamedIndividual .


###  https://w3id.org/mobility/transmodel/journeys#aViewOf
:aViewOf rdf:type owl:NamedIndividual .


###  https://w3id.org/mobility/transmodel/journeys#accessMode
:accessMode rdf:type owl:NamedIndividual .


###  https://w3id.org/mobility/transmodel/journeys#accessPTS
:accessPTS rdf:type owl:NamedIndividual .


###  https://w3id.org/mobility/transmodel/journeys#allowedLineDirections
:allowedLineDirections rdf:type owl:NamedIndividual .


###  https://w3id.org/mobility/transmodel/journeys#arrivalDayOffset
:arrivalDayOffset rdf:type owl:NamedIndividual .


###  https://w3id.org/mobility/transmodel/journeys#arrivalTime
:arrivalTime rdf:type owl:NamedIndividual .


###  https://w3id.org/mobility/transmodel/journeys#beginsConnection
:beginsConnection rdf:type owl:NamedIndividual .


###  https://w3id.org/mobility/transmodel/journeys#belongingTo
:belongingTo rdf:type owl:NamedIndividual .


###  https://w3id.org/mobility/transmodel/journeys#blockPart
:blockPart rdf:type owl:NamedIndividual .


###  https://w3id.org/mobility/transmodel/journeys#canAlight
:canAlight rdf:type owl:NamedIndividual .


###  https://w3id.org/mobility/transmodel/journeys#canBoard
:canBoard rdf:type owl:NamedIndividual .


###  https://w3id.org/mobility/transmodel/journeys#changeOfDestinationDisplay
:changeOfDestinationDisplay rdf:type owl:NamedIndividual .


###  https://w3id.org/mobility/transmodel/journeys#changeOfServiceRequirements
:changeOfServiceRequirements rdf:type owl:NamedIndividual .


###  https://w3id.org/mobility/transmodel/journeys#characterisedBy
:characterisedBy rdf:type owl:NamedIndividual .


###  https://w3id.org/mobility/transmodel/journeys#classifiedBy
:classifiedBy rdf:type owl:NamedIndividual .


###  https://w3id.org/mobility/transmodel/journeys#composedOf
:composedOf rdf:type owl:NamedIndividual .


###  https://w3id.org/mobility/transmodel/journeys#composedOfLink
:composedOfLink rdf:type owl:NamedIndividual .


###  https://w3id.org/mobility/transmodel/journeys#date
:date rdf:type owl:NamedIndividual .


###  https://w3id.org/mobility/transmodel/journeys#day
:day rdf:type owl:NamedIndividual .


###  https://w3id.org/mobility/transmodel/journeys#dayTypeAssignment
:dayTypeAssignment rdf:type owl:NamedIndividual .


###  https://w3id.org/mobility/transmodel/journeys#defaultDeadRunRunTime
:defaultDeadRunRunTime rdf:type owl:NamedIndividual .


###  https://w3id.org/mobility/transmodel/journeys#defaultInterchange
:defaultInterchange rdf:type owl:NamedIndividual .


###  https://w3id.org/mobility/transmodel/journeys#definedAs
:definedAs rdf:type owl:NamedIndividual .


###  https://w3id.org/mobility/transmodel/journeys#defines
:defines rdf:type owl:NamedIndividual .


###  https://w3id.org/mobility/transmodel/journeys#departureDayOffset
:departureDayOffset rdf:type owl:NamedIndividual .


###  https://w3id.org/mobility/transmodel/journeys#departureTime
:departureTime rdf:type owl:NamedIndividual .


###  https://w3id.org/mobility/transmodel/journeys#describedBy
:describedBy rdf:type owl:NamedIndividual .


###  https://w3id.org/mobility/transmodel/journeys#destinationDisplay
:destinationDisplay rdf:type owl:NamedIndividual .


###  https://w3id.org/mobility/transmodel/journeys#destinationStop
:destinationStop rdf:type owl:NamedIndividual .


###  https://w3id.org/mobility/transmodel/journeys#directionType
:directionType rdf:type owl:NamedIndividual .


###  https://w3id.org/mobility/transmodel/journeys#directionType_old
:directionType_old rdf:type owl:NamedIndividual .


###  https://w3id.org/mobility/transmodel/journeys#distanceFromStart
:distanceFromStart rdf:type owl:NamedIndividual .


###  https://w3id.org/mobility/transmodel/journeys#endOf
:endOf rdf:type owl:NamedIndividual .


###  https://w3id.org/mobility/transmodel/journeys#endOfBlock
:endOfBlock rdf:type owl:NamedIndividual .


###  https://w3id.org/mobility/transmodel/journeys#endingAt
:endingAt rdf:type owl:NamedIndividual .


###  https://w3id.org/mobility/transmodel/journeys#endsConnection
:endsConnection rdf:type owl:NamedIndividual .


###  https://w3id.org/mobility/transmodel/journeys#endsConnectionDefault
:endsConnectionDefault rdf:type owl:NamedIndividual .


###  https://w3id.org/mobility/transmodel/journeys#firstDayOffset
:firstDayOffset rdf:type owl:NamedIndividual .


###  https://w3id.org/mobility/transmodel/journeys#firstDepartureTime
:firstDepartureTime rdf:type owl:NamedIndividual .


###  https://w3id.org/mobility/transmodel/journeys#followsDeadRunTime
:followsDeadRunTime rdf:type owl:NamedIndividual .


###  https://w3id.org/mobility/transmodel/journeys#followsJourneyPattern
:followsJourneyPattern rdf:type owl:NamedIndividual .


###  https://w3id.org/mobility/transmodel/journeys#for
:for rdf:type owl:NamedIndividual .


###  https://w3id.org/mobility/transmodel/journeys#forAlighting
:forAlighting rdf:type owl:NamedIndividual .


###  https://w3id.org/mobility/transmodel/journeys#forBoarding
:forBoarding rdf:type owl:NamedIndividual .


###  https://w3id.org/mobility/transmodel/journeys#forServicedOrganisation
:forServicedOrganisation rdf:type owl:NamedIndividual .


###  https://w3id.org/mobility/transmodel/journeys#headway
:headway rdf:type owl:NamedIndividual .


###  https://w3id.org/mobility/transmodel/journeys#holidayType
:holidayType rdf:type owl:NamedIndividual .


###  https://w3id.org/mobility/transmodel/journeys#holidayType-old
:holidayType-old rdf:type owl:NamedIndividual .


###  https://w3id.org/mobility/transmodel/journeys#inLinkSequence
:inLinkSequence rdf:type owl:NamedIndividual .


###  https://w3id.org/mobility/transmodel/journeys#isAvailable
:isAvailable rdf:type owl:NamedIndividual .


###  https://w3id.org/mobility/transmodel/journeys#isDefinedBy
:isDefinedBy rdf:type owl:NamedIndividual .


###  https://w3id.org/mobility/transmodel/journeys#isFlexible
:isFlexible rdf:type owl:NamedIndividual .


###  https://w3id.org/mobility/transmodel/journeys#isServiceDay
:isServiceDay rdf:type owl:NamedIndividual .


###  https://w3id.org/mobility/transmodel/journeys#isWaitPoint
:isWaitPoint rdf:type owl:NamedIndividual .


###  https://w3id.org/mobility/transmodel/journeys#journeyPatternMadeUpOf
:journeyPatternMadeUpOf rdf:type owl:NamedIndividual .


###  https://w3id.org/mobility/transmodel/journeys#journeyPatternPoint
:journeyPatternPoint rdf:type owl:NamedIndividual .


###  https://w3id.org/mobility/transmodel/journeys#journeyPatternRunTime
:journeyPatternRunTime rdf:type owl:NamedIndividual .


###  https://w3id.org/mobility/transmodel/journeys#lastDayOffset
:lastDayOffset rdf:type owl:NamedIndividual .


###  https://w3id.org/mobility/transmodel/journeys#lastDepartureTime
:lastDepartureTime rdf:type owl:NamedIndividual .


###  https://w3id.org/mobility/transmodel/journeys#layover
:layover rdf:type owl:NamedIndividual .


###  https://w3id.org/mobility/transmodel/journeys#lineName
:lineName rdf:type owl:NamedIndividual .


###  https://w3id.org/mobility/transmodel/journeys#lineNumber
:lineNumber rdf:type owl:NamedIndividual .


###  https://w3id.org/mobility/transmodel/journeys#madeUpOf
:madeUpOf rdf:type owl:NamedIndividual .


###  https://w3id.org/mobility/transmodel/journeys#madeUsing
:madeUsing rdf:type owl:NamedIndividual .


###  https://w3id.org/mobility/transmodel/journeys#maximumHeadwayInterval
:maximumHeadwayInterval rdf:type owl:NamedIndividual .


###  https://w3id.org/mobility/transmodel/journeys#minimumHeadwayInterval
:minimumHeadwayInterval rdf:type owl:NamedIndividual .


###  https://w3id.org/mobility/transmodel/journeys#monitored
:monitored rdf:type owl:NamedIndividual .


###  https://w3id.org/mobility/transmodel/journeys#on
:on rdf:type owl:NamedIndividual .


###  https://w3id.org/mobility/transmodel/journeys#onLine
:onLine rdf:type owl:NamedIndividual .


###  https://w3id.org/mobility/transmodel/journeys#onRoute
:onRoute rdf:type owl:NamedIndividual .


###  https://w3id.org/mobility/transmodel/journeys#operatedBy
:operatedBy rdf:type owl:NamedIndividual .


###  https://w3id.org/mobility/transmodel/journeys#operatingPeriod
:operatingPeriod rdf:type owl:NamedIndividual .


###  https://w3id.org/mobility/transmodel/journeys#order
:order rdf:type owl:NamedIndividual .


###  https://w3id.org/mobility/transmodel/journeys#originStop
:originStop rdf:type owl:NamedIndividual .


###  https://w3id.org/mobility/transmodel/journeys#overriding
:overriding rdf:type owl:NamedIndividual .


###  https://w3id.org/mobility/transmodel/journeys#passengerConnection
:passengerConnection rdf:type owl:NamedIndividual .


###  https://w3id.org/mobility/transmodel/journeys#passesAt
:passesAt rdf:type owl:NamedIndividual .


###  https://w3id.org/mobility/transmodel/journeys#passingTimeTimingPoint
:passingTimeTimingPoint rdf:type owl:NamedIndividual .


###  https://w3id.org/mobility/transmodel/journeys#prescribing
:prescribing rdf:type owl:NamedIndividual .


###  https://w3id.org/mobility/transmodel/journeys#presentedBy
:presentedBy rdf:type owl:NamedIndividual .


###  https://w3id.org/mobility/transmodel/journeys#primarilyAdvertisedWith
:primarilyAdvertisedWith rdf:type owl:NamedIndividual .


###  https://w3id.org/mobility/transmodel/journeys#requestStop
:requestStop rdf:type owl:NamedIndividual .


###  https://w3id.org/mobility/transmodel/journeys#routeOnLine
:routeOnLine rdf:type owl:NamedIndividual .


###  https://w3id.org/mobility/transmodel/journeys#runBy
:runBy rdf:type owl:NamedIndividual .


###  https://w3id.org/mobility/transmodel/journeys#runTimeOverrides
:runTimeOverrides rdf:type owl:NamedIndividual .


###  https://w3id.org/mobility/transmodel/journeys#runsOn
:runsOn rdf:type owl:NamedIndividual .


###  https://w3id.org/mobility/transmodel/journeys#runtime
:runtime rdf:type owl:NamedIndividual .


###  https://w3id.org/mobility/transmodel/journeys#scheduledHeadwayInterval
:scheduledHeadwayInterval rdf:type owl:NamedIndividual .


###  https://w3id.org/mobility/transmodel/journeys#scheduledStopPoint
:scheduledStopPoint rdf:type owl:NamedIndividual .


###  https://w3id.org/mobility/transmodel/journeys#season
:season rdf:type owl:NamedIndividual .


###  https://w3id.org/mobility/transmodel/journeys#serviceJourneyUsingPattern
:serviceJourneyUsingPattern rdf:type owl:NamedIndividual .


###  https://w3id.org/mobility/transmodel/journeys#specifying
:specifying rdf:type owl:NamedIndividual .


###  https://w3id.org/mobility/transmodel/journeys#startOf
:startOf rdf:type owl:NamedIndividual .


###  https://w3id.org/mobility/transmodel/journeys#startOfBlock
:startOfBlock rdf:type owl:NamedIndividual .


###  https://w3id.org/mobility/transmodel/journeys#startTime
:startTime rdf:type owl:NamedIndividual .


###  https://w3id.org/mobility/transmodel/journeys#startingAt
:startingAt rdf:type owl:NamedIndividual .


###  https://w3id.org/mobility/transmodel/journeys#stopUse
:stopUse rdf:type owl:NamedIndividual .


###  https://w3id.org/mobility/transmodel/journeys#stopsAt
:stopsAt rdf:type owl:NamedIndividual .


###  https://w3id.org/mobility/transmodel/journeys#time
:time rdf:type owl:NamedIndividual .


###  https://w3id.org/mobility/transmodel/journeys#timeLink
:timeLink rdf:type owl:NamedIndividual .


###  https://w3id.org/mobility/transmodel/journeys#timedFrom
:timedFrom rdf:type owl:NamedIndividual .


###  https://w3id.org/mobility/transmodel/journeys#timingLink
:timingLink rdf:type owl:NamedIndividual .


###  https://w3id.org/mobility/transmodel/journeys#timingLinkInJourneyPattern
:timingLinkInJourneyPattern rdf:type owl:NamedIndividual .


###  https://w3id.org/mobility/transmodel/journeys#typeOfFlexibleService
:typeOfFlexibleService rdf:type owl:NamedIndividual .


###  https://w3id.org/mobility/transmodel/journeys#usedToDefine
:usedToDefine rdf:type owl:NamedIndividual .


###  https://w3id.org/mobility/transmodel/journeys#vehicleJourney
:vehicleJourney rdf:type owl:NamedIndividual .


###  https://w3id.org/mobility/transmodel/journeys#vehicleJourneyPart
:vehicleJourneyPart rdf:type owl:NamedIndividual .


###  https://w3id.org/mobility/transmodel/journeys#vehicleJourneyRoute
:vehicleJourneyRoute rdf:type owl:NamedIndividual .


###  https://w3id.org/mobility/transmodel/journeys#vehicleJourneyRunTimeOverrides
:vehicleJourneyRunTimeOverrides rdf:type owl:NamedIndividual .


###  https://w3id.org/mobility/transmodel/journeys#vehicleJourneys
:vehicleJourneys rdf:type owl:NamedIndividual .


###  https://w3id.org/mobility/transmodel/journeys#vehicleModeId
:vehicleModeId rdf:type owl:NamedIndividual .


###  https://w3id.org/mobility/transmodel/journeys#vehiclePassingTime
:vehiclePassingTime rdf:type owl:NamedIndividual .


###  https://w3id.org/mobility/transmodel/journeys#viaFlag
:viaFlag rdf:type owl:NamedIndividual .


###  https://w3id.org/mobility/transmodel/journeys#viewedAs
:viewedAs rdf:type owl:NamedIndividual .


###  https://w3id.org/mobility/transmodel/journeys#virtualLineService
:virtualLineService rdf:type owl:NamedIndividual ;
                    rdfs:label "VirtualLineService"@en .


###  https://w3id.org/mobility/transmodel/journeys#waitTime
:waitTime rdf:type owl:NamedIndividual .


###  https://w3id.org/mobility/transmodel/journeys#workedOn
:workedOn rdf:type owl:NamedIndividual .


###  https://w3id.org/mobility/transmodel/commons#ComplexFeature
<https://w3id.org/mobility/transmodel/commons#ComplexFeature> rdf:type owl:NamedIndividual .


###  https://w3id.org/mobility/transmodel/commons#SimpleFeature
<https://w3id.org/mobility/transmodel/commons#SimpleFeature> rdf:type owl:NamedIndividual .


###  https://w3id.org/mobility/transmodel/commons#Zone
<https://w3id.org/mobility/transmodel/commons#Zone> rdf:type owl:NamedIndividual .


###  https://w3id.org/mobility/transmodel/facilities#AccessibilityAssessment
<https://w3id.org/mobility/transmodel/facilities#AccessibilityAssessment> rdf:type owl:NamedIndividual .


###  https://w3id.org/mobility/transmodel/facilities#ServiceFacilitySet
<https://w3id.org/mobility/transmodel/facilities#ServiceFacilitySet> rdf:type owl:NamedIndividual .


###  https://w3id.org/mobility/transmodel/facilities#VehicleType
<https://w3id.org/mobility/transmodel/facilities#VehicleType> rdf:type owl:NamedIndividual .


###  https://w3id.org/mobility/transmodel/facilities#journeyPatternAdvertisedFor
<https://w3id.org/mobility/transmodel/facilities#journeyPatternAdvertisedFor> rdf:type owl:NamedIndividual .


###  https://w3id.org/mobility/transmodel/kos/commons/all-modes
<https://w3id.org/mobility/transmodel/kos/commons/all-modes> rdf:type owl:NamedIndividual ,
                                                             <http://www.w3.org/2004/02/skos/core#ConceptScheme> .


###  https://w3id.org/mobility/transmodel/kos/journeys/day-type
<https://w3id.org/mobility/transmodel/kos/journeys/day-type> rdf:type owl:NamedIndividual ,
                                                             <http://www.w3.org/2004/02/skos/core#ConceptScheme> ;
                                                    rdfs:comment "Concept scheme where all the codelists for the types of datatype properties that are included in the Transmodel ontology"@en ;
                                                    rdfs:label "day type"@en .


###  https://w3id.org/mobility/transmodel/kos/journeys/direction-type
<https://w3id.org/mobility/transmodel/kos/journeys/direction-type> rdf:type owl:NamedIndividual ,
                                                                   <http://www.w3.org/2004/02/skos/core#ConceptScheme> ;
                                                          rdfs:comment "Concept scheme for types of directions (inbound, outbound, clockwise, anticlockwise)"@en .


###  https://w3id.org/mobility/transmodel/kos/journeys/entrance-type
<https://w3id.org/mobility/transmodel/kos/journeys/entrance-type> rdf:type owl:NamedIndividual ,
                                                                  <http://www.w3.org/2004/02/skos/core#ConceptScheme> ;
                                                         rdfs:comment "Concept scheme where all the codelists for the types of entrance types that are included in the Transmodel ontology"@en .


###  https://w3id.org/mobility/transmodel/kos/journeys/interchange-weighting-type
<https://w3id.org/mobility/transmodel/kos/journeys/interchange-weighting-type> rdf:type owl:NamedIndividual ,
                                                                               <http://www.w3.org/2004/02/skos/core#ConceptScheme> ;
                                                                      rdfs:comment "Concept scheme where all the codelists for the types of interchange weighting types that are included in the Transmodel ontology"@en .


###  https://w3id.org/mobility/transmodel/kos/journeys/limited-use-type
<https://w3id.org/mobility/transmodel/kos/journeys/limited-use-type> rdf:type owl:NamedIndividual ,
                                                                     <http://www.w3.org/2004/02/skos/core#ConceptScheme> ;
                                                            rdfs:comment "Concept scheme where all the codelists for the types of limited use that are included in the Transmodel ontology"@en .


###  https://w3id.org/mobility/transmodel/kos/journeys/mobility-limitation
<https://w3id.org/mobility/transmodel/kos/journeys/mobility-limitation> rdf:type owl:NamedIndividual ,
                                                                        <http://www.w3.org/2004/02/skos/core#ConceptScheme> ;
                                                               rdfs:comment "Concept scheme  for types of mobility limitations"@en ;
                                                               rdfs:label "mobility-limitation"@en .


###  https://w3id.org/mobility/transmodel/kos/journeys/quay-type
<https://w3id.org/mobility/transmodel/kos/journeys/quay-type> rdf:type owl:NamedIndividual ,
                                                              <http://www.w3.org/2004/02/skos/core#ConceptScheme> ;
                                                     rdfs:comment "Concept scheme where all the codelists for the types of quay types that are included in the Transmodel ontology"@en .


###  https://w3id.org/mobility/transmodel/kos/journeys/stop-place
<https://w3id.org/mobility/transmodel/kos/journeys/stop-place> rdf:type owl:NamedIndividual ,
                                                               <http://www.w3.org/2004/02/skos/core#ConceptScheme> ;
                                                      rdfs:comment "Concept scheme  for types of stop place"@en ;
                                                      rdfs:label "stop-place"@en .


###  https://w3id.org/mobility/transmodel/kos/journeys/stop-place-component-type
<https://w3id.org/mobility/transmodel/kos/journeys/stop-place-component-type> rdf:type owl:NamedIndividual ,
                                                                              <http://www.w3.org/2004/02/skos/core#ConceptScheme> ;
                                                                     rdfs:comment "Concept scheme where all the codelists for the types of stop place component types that are included in the Transmodel ontology"@en .


###  https://w3id.org/mobility/transmodel/kos/journeys/stop-use-type
<https://w3id.org/mobility/transmodel/kos/journeys/stop-use-type> rdf:type owl:NamedIndividual ,
                                                                  <http://www.w3.org/2004/02/skos/core#ConceptScheme> ;
                                                         rdfs:comment "Concept scheme  for types of use of stops (e.g., access, interchange only, pass through or non boarding alighting)"@en ;
                                                         rdfs:label "stop-use-type"@en .


###  https://w3id.org/mobility/transmodel/organisations#Operator
<https://w3id.org/mobility/transmodel/organisations#Operator> rdf:type owl:NamedIndividual .


###  https://w3id.org/mobility/transmodel/organisations#passengerJourney
<https://w3id.org/mobility/transmodel/organisations#passengerJourney> rdf:type owl:NamedIndividual .


###  https://w3id.org/mobility/transmodel/organisations#serviceJourneyServedByVehicleJourney
<https://w3id.org/mobility/transmodel/organisations#serviceJourneyServedByVehicleJourney> rdf:type owl:NamedIndividual .


###  https://w3id.org/mobility/transmodel/organisations#trip
<https://w3id.org/mobility/transmodel/organisations#trip> rdf:type owl:NamedIndividual .


_:genid195 :mbox "adolfo.anton.bravo@upm.es"@en ;
           :name "Adolfo Anton-Bravo"@en .

#################################################################
#    Annotations
#################################################################

<http://purl.org/dc/terms/identifier> rdfs:label "id"@en .


<http://schema.org/url> rdfs:comment "A URL associated"@en ;
                        rdfs:label "url"@en .


rdfs:comment rdfs:label "description"@en .


rdfs:label rdfs:label "name"@en .


:ActivationPoint rdfs:comment "A Point where a control process is activated when a vehicle passes it. Equipment may be needed for the activation."@en ;
                 rdfs:label "Activation Point"@en .


:BeaconPoint rdfs:comment "A Point where a beacon or similar device to support the automatic detection of Vehicles passing by is located"@en ;
             rdfs:label "BeaconPoint"@en .


:Block rdfs:comment "The work of a vehicle from the time it leaves a Parking Point after parking until its next return to park at a Parking Point. Any subsequent departure from a Parking Point after parking marks the start of a new Block. The period of a Block must be covered by Duties."@en ;
       rdfs:label "Block"@en .


:BoardingPosition rdfs:comment "A location within a Quay from which Passenger may directly board, or onto which passengers may directly alight from a Vehicle"@en ;
                  rdfs:label "Boarding Position"@en .


:DatedBlock rdfs:comment "The work of a Vehicle on a particular Operating Day from the time it leaves a Parking Point after parking until its next return to park at a Parking Point"@en ;
            rdfs:label "DatedBlock"@en .


:DatedVehicleJourney rdfs:comment "A particular Journey of a Vehicle on a particular OperatingDay including all modifications possibly decided by the control staff"@en ;
                     rdfs:label "Dated Vehicle Journey"@en .


:DayType rdfs:comment "A Day Type is a type of day characterised by one or more properties which affect public transport operation"@en ;
         rdfs:label "Day Type"@en ,
                    "TODO: Check season and complete with other properties"@en .


:DayTypeAssignment rdfs:comment "The assignment of operational characteristics, expressed by Day Type to particular Operating Day within a Service Calendar"@en ;
                   rdfs:label "Day Type Assignment"@en .


:DeadRun rdfs:comment "A non-service VehicleJourney"@en ;
         rdfs:label "Dead Run"@en .


:DeadRunPattern rdfs:comment "A JourneyPattern to be used for DeadRun"@en ;
                rdfs:label "DeadRunPattern"@en .


:DestinationDisplay rdfs:comment "An advertised destination of a specific Journey Pattern usually displayed on a headsign or other on-board locations"@en ;
                    rdfs:label "Destination Display"@en .


:DestinationDisplayVariant rdfs:comment "An advertised destination of a specific Journey Pattern, usually displayed on a headsign (Heading Sign) or at other on-board locations"@en ;
                           rdfs:label "Destination Display Variant"@en .


:DynamicStopAssignment rdfs:comment "The dynamic association of a Scheduled Stop Point with the next available Stop Place, Quay or Boarding Position within a Stop Place."@en ;
                       rdfs:label "Dynamic Stop Assignment"@en .


:FareDayType rdfs:comment "A type of day used in the fare collection domain, characterised by one or more properties which affect the definition of access rights and prices in the fare system."@en ,
                          "TODO: Add information on the relationship with PricingParameterSet"@en ;
             rdfs:label "Fare Day Type"@en .


:FarePointInJourneyPattern rdfs:comment "TODO: Add all relevant properties here"@en ,
                                        "TODO: This should be probably moved to the Fares module, unless we make a link from that fares module into this one."@en .


:FlexiblePoint rdfs:comment "A specialisation of Point for Flexible Service"@en ;
               rdfs:label "Flexible Point"@en .


:GaragePoint rdfs:comment "A subtype of Parking Point located in a Garage."@en ,
                          "TODO: Complete all properties"@en ;
             rdfs:label "Garage Point"@en .


:GroupOfLinkSequences rdfs:comment "A grouping of Link Sequences."@en ;
                      rdfs:label "Group of Link Sequences"@en .


:HeadwayInterval rdfs:comment "A time interval or a duration defining a headway period and characterizing Headway Journey Groups (e.g. every 10 min, every  4-6 min)."@en ;
                 rdfs:label "Headway Interval"@en .


:HeadwayJourneyGroup rdfs:comment "A group of Vehicle Journeys following the same Journey Pattern having the same Headway Interval between a specified start and end time (for example, every 10 min). This is especially useful for passenger information."@en ,
                                  "TODO Define the TimeBand class that is describing the time band for this type of journey group, and hence can be related to this class or to its superclass."@en ,
                                  "TODO: Include the class Time Demand Type, which is used to specify traffic conditions or other factors which may affect vehicle run or wait times, and relate it to this class"@en ;
                     rdfs:label "Headway Journey Group"@en .


:InfrastructurePoint rdfs:comment "A super-type including all Points of the physical network (e.g. Railway Junction)."@en ;
                     rdfs:label "Infrastructure Point"@en .


:Journey rdfs:comment "Common properties of Vehicle Journey and Special Service, e.g. their link to accounting characteristics"@en ;
         rdfs:label "Journey"@en .


:JourneyFrequencyGroup rdfs:comment "A group of Journeys defined in order to describe special behaviour like frequency based services or rhythmical services (e.g., runs all xxh10, xxh25 and xxh45). This is especially useful for passenger information)."@en ;
                       rdfs:label "Journey Frequency Group"@en .


:JourneyPattern rdfs:comment "An ordered list of Scheduled Stop Points and Timing Points on a single Route, describing the pattern of working for public transport vehicles. A Journey Pattern may pass through the same Point more than once. The first Point of a Journey Pattern is the origin. The last Point is the destination."@en ;
                rdfs:label "Journey Pattern"@en .


:Line rdfs:comment "A Line is a group of Routes which is generally known to the public by a similar name or number."@en ;
      rdfs:label "Line"@en .


:Link rdfs:comment "An oriented spatial object of dimension 1 with view to the overall description of a network,  describing a connection between two POINTs."@en .


:LinkInLinkSequence rdfs:comment "The order of a Link in a Link Sequence  to which it belongs."@en .


:LinkSequence rdfs:comment "An ordered sequence either of POINTs or of LINKs, defining a path through the network"@en ;
              rdfs:label "Link Sequence"@en .


:MonitoredVehicleJourney rdfs:comment "A VehicleJourney that is run under real-time tracking system and so for which real-time observations and predictions and other data are available"@en ;
                         rdfs:label "Monitored Vehicle Journey"@en .


:OperatingDay rdfs:comment "A day of public transport operation of which the characteristics are defined within in a specific ServiceCalendar. An OperatingDay may last more than 24 hours."@en ;
              rdfs:label "Operating Day"@en .


:OperatingPeriod rdfs:comment "A continuous interval of time between two Operating Day which will be used to define validities"@en ;
                 rdfs:label "Operating Period"@en .


:OrganisationDayType rdfs:comment "Day Type that is defined in terms of operation or not operation of a referenced Serviced Organisation."@en ;
                     rdfs:label "Organisation Day Type"@en ,
                                "TODO: Add constraint: :forServicedOrganisation only tmorg:ServicedOrganisation"@en .


:ParkingPoint rdfs:comment "A Parking Point where Vehicles may stay unattended for a long time. A vehicle's return to the Parking Point marks the end of a Block"@en ;
              rdfs:label "Parking Point"@en .


:PassengerStopAssignment rdfs:comment "The allocation of a Scheduled Stop Point to a specific Stop Place for a Service Journey, and also possibly a Quay and Boarding Position"@en ;
                         rdfs:label "Passenger Stop Assignment"@en .


:PointInJourneyPattern rdfs:comment "A Scheduled Stop Point OR Timing Point in a Journey Pattern with its order in that Journey Pattern"@en ;
                       rdfs:label "Point In Journey Pattern"@en .


:PointInLinkSequence rdfs:comment "A point in a Link Sequence indicating its order in that particular Link Sequence"@en ;
                     rdfs:label "Point In Link Sequence"@en .


:PointOnRoute rdfs:comment "A Route Point used to define a Route with its order on that Route."@en ;
              rdfs:label "Point on Route"@en .


:PropertyOfDay rdfs:comment "A property which a day may possess, such as school holiday, weekday, summer, winter, etc."@en ;
               rdfs:label "Property Of Day"@en .


:RailwayJunction rdfs:comment "A type of INFRASTRUCTURE POINT used to describe a railway network."@en ;
                 rdfs:label "Railway Junction"@en .


:ReliefPoint rdfs:comment "A Timing Point where a relief is possible, i.e. a driver may take on or hand over a vehicle. The vehicle may sometimes be left unattended."@en ,
                          "TODO: Complete all properties"@en ;
             rdfs:label "Relief Point"@en .


:RhythmicalJourneyGroup rdfs:comment "A group of Vehicle Journeys following  the same Journey Pattern having the same \"rhythm\" every hour (for example runs at xxh10, xxh25 and xxh45... ) between a specified start and end time."@en ,
                                     "TODO Define the TimeBand class that is describing the time band for this type of journey group, and hence can be related to this class or to its superclass."@en ;
                        rdfs:label "Rhythmical Journey Group"@en .


:RoadJunction rdfs:comment "A type of INFRASTRUCTURE POINT used to describe a road network."@en ;
              rdfs:label "Road Junction"@en .


:Route rdfs:comment "A Route is and ordered list of located Points defining one single path through the road (or rail) network."@en ;
       rdfs:label "Route"@en .


:RouteLink rdfs:comment "An oriented link between two ROUTE POINTs allowing the definition of a unique path through the network."@en .


:RoutePoint rdfs:comment "A Point used to define the shape of a Route through the network."@en ;
            rdfs:label "Route Point"@en .


:ScheduledStopPoint rdfs:comment "A Scheduled Stop Point is a Point where a Passenger can board or alight from a Vehicle."@en ;
                    rdfs:label "Scheduled Stop Point"@en .


:ServiceJourney rdfs:comment "A Service Journey is a passenger-carrying Vehicle Journey for one specified Day Type. The pattern of working is in principle defined by a Service Journey Pattern."@en ;
                rdfs:label "Service Journey"@en .


:ServiceJourneyPattern rdfs:comment "The Journey Pattern for (a Passenger carrying) Service Journeys"@en ;
                       rdfs:label "Service Journey Pattern"@en .


:StopArea rdfs:comment "A group of Scheduled Stop Points close to each other"@en ;
          rdfs:label "Stop Area"@en .


:StopAssignment rdfs:comment "The allocation of a Scheduled Stop Point (i.e. a Scheduled Stop Point of a Service Pattern or Journey Pattner) to a specific Stop Place, for either a Service Journey or Vehicle Service."@en ;
                rdfs:label "Stop Assignment"@en .


:StopPointInJourneyPattern rdfs:comment "A Point in Journey Pattern that is a Scheduled Stop Point"@en ;
                           rdfs:label "Stop Point In Journey Pattern"@en .


:TemplateServiceJourney rdfs:comment "A passenger-carrying Template Vehicle Journey. It may represent multiple journeys."@en ;
                        rdfs:label "Template Service Journey"@en .


:TemplateVehicleJourney rdfs:comment "A repeating Vehicle Journey for which a frequency has been specified, either as a Headway Journey Group (e.g. every 20 minutes) or a Rhythmical Journey Group (e.g. at 15, 27 and 40 minutes past the hour). It may thus represent multiple journeys."@en ;
                        rdfs:label "Template Vehicle Journey"@en .


:TimetabledPassingTime rdfs:comment "Long-term planned time data concerning public transport Vehicles passing a particular POINT IN JOURNEY PATTERN on a specified VEHICLE JOURNEY for a certain DAY TYPE."@en ;
                       rdfs:label "Timetabled Passing Time"@en .


:TimetabledVehicleJourney rdfs:comment "The planned movement of a Public Transport Vehicle on a Day Type from the start point to the end point of a Journey Pattern on a specified Route."@en ;
                          rdfs:label "Timetabled Vehicle Journey"@en .


:TimingLink rdfs:comment "A TimingLink is an ordered pair of Timing Point for which run times may be recorded."@en ;
            rdfs:label "TimingLink"@en .


:TimingPoint rdfs:comment """A Timing Point is a Point against which the timing information necessary to build schedules may be recorded.

It's the same as Timing Point In Journey Pattern"""@en ;
             rdfs:label "Timing Point"@en .


:TimingPointInJourneyPattern rdfs:comment "A Point in a Journey Pattern which is a Timing Point"@en ;
                             rdfs:label "Timing Point In Journey Pattern"@en .


:TrafficControlPoint rdfs:comment "A Point where the traffic flow can be influenced. Examples are: traffic lights (lanterns), barriers."@en ,
                                  "TODO: Complete with all relevant properties"@en ;
                     rdfs:label "Traffic Control Point"@en .


:VehicleJourney rdfs:comment """A Vehicle Journey is the journey made by the Vehicle.

A Service Journey is made of Vehicle Journeys

Within VehicleJourney there are several types:
- Timetabled Vehicle Journey in a general timetable that will run on a specific time on a Day Type throughout the period of applicability of the schedule.
- Dated Vehicle Journey, a specific Vehicle Journey that runs on a spcific calendar date;
- Monitored Vehicle Journey, a Vehicle Journey run under real-time tracking system and so for which real-time observations and predictions and other data are available.
- Dead Run, a Vehicle Journey without service"""@en ;
                rdfs:label "Vehicle Journey"@en .


:VehicleMode rdfs:comment "A characterisation of the public transport operation according to the means of transport (bus, tram, metro, train, ferry, ship)."@en ;
             rdfs:label "Vehicle Mode"@en .


:WireJunction rdfs:comment "A type of INFRASTRUCTURE POINT used to describe a wire network."@en ;
              rdfs:label "Wire Junction"@en .


:aViewOf rdfs:comment "This property allows relating a Point with the Points in Link Sequence where it appears"@en ;
         rdfs:label "a View Of"@en .


:accessMode rdfs:label "accessMode"@en .


:accessPTS rdfs:comment """The physical spatial possibility for a passenger to access or leave the Public Transport System. The link may be used during a Trip for :
- The walking movement of the Passenger from a Place (Origin of the Trip) to a ScheduledStopPoint (origin of the Public Transport Trip) or;
- The walking movement of the Passenger from a Scheduled Stop Point (destination of the Public Transport Trip) to a Place (destination of the Trip)"""@en ;
           rdfs:label "accessPTS"@en .


:allowedLineDirections rdfs:label "allowedLineDirections"@en .


:arrivalDayOffset rdfs:comment "Arrival Day Offset (e.g., for a TimeTabledPassingTime)"@en ;
                  rdfs:label "arrival day offset"@en .


:arrivalTime rdfs:comment "Arrival time (e.g., for a Service Journey in a Timing Point)"@en ;
             rdfs:label "arrival Time"@en .


:beginsConnection rdfs:label "beginsConnection"@en .


:belongingTo rdfs:comment "This property sets the relationship between Vehicle Type and Vehicle Mode"@en ;
             rdfs:label "belonging To"@en .


:blockPart rdfs:label "blockPart"@en .


:canAlight rdfs:label "canAlight"@en .


:canBoard rdfs:label "canBoard"@en .


:changeOfDestinationDisplay rdfs:comment "This property allows describing whether there will be a change of the destination display at this point"@en ;
                            rdfs:label "change Of Destination Display"@en .


:changeOfServiceRequirements rdfs:comment "This property allows describing whether there will be a change of the service requirements at this point"@en ;
                             rdfs:label "change Of Service Requirements"@en .


:characterisedBy rdfs:comment "This property is the relationship of a Journey and the Accessibility Assessment"@en ;
                 rdfs:label "characterised By"@en .


:classifiedBy rdfs:comment "This property allows relating a Line with the transport modes which are used to operate it"@en ;
              rdfs:label "classified by"@en .


:composedOf rdfs:comment "This property relates a Journey Frequency Group with the Vehicle Journeys that it is composed of"@en ;
            rdfs:label "composed of"@en .


:composedOfLink rdfs:comment "This property allows grouping a Link Sequences."@en .


:date rdfs:comment "This property sets up the date for the Day Type Assignment"@en ;
      rdfs:label "date"@en .


:day rdfs:comment "This property relates a Day Of Week with a Day Type which is defined in KOS day-type"@en ;
     rdfs:label "day"@en .


:dayTypeAssignment rdfs:comment "The assignment of operational characteristics, expressed by DayType, to a particular OperatingDay within a ServiceCalendar"@en ;
                   rdfs:label "dayTypeAssignment"@en .


:defaultDeadRunRunTime rdfs:label "defaultDeadRunRunTime"@en .


:defaultInterchange rdfs:label "defaultInterchange"@en .


:definedAs rdfs:comment "This property sets the relationship between Property Of Day and the SKOS Concept Scheme for days of the week"@en ;
           rdfs:label "defined As"@en .


:defines rdfs:comment "This property relates a Rhythmical Journey Group with a Template Vehicle Journey"@en ;
         rdfs:label "defines"@en .


:departureDayOffset rdfs:comment "Departure Day Offset (e.g., for a TimeTabledPassingTime)"@en ;
                    rdfs:label "departure day offset"@en .


:departureTime rdfs:comment "Departure Time (e.g., for a Service Journey in a Timing Point)"@en ,
                            "departure time of vehicle journey."@en ;
               rdfs:label "departure Time"@en .


:describedBy rdfs:comment "This property asign a DayType to the specific Property of Day"@en ;
             rdfs:label "described By"@en .


:destinationDisplay rdfs:label "destination display"@en .


:destinationStop rdfs:label "destinationStop"@en .


:directionType rdfs:comment "This property allows describing the type of direction for a service journey"@en ;
               rdfs:label "direction Type"@en .


:directionType_old rdfs:label "direction Type"@en .


:distanceFromStart rdfs:comment "For a Point in a Link Sequence (or alike), this property represents the distance from the start of the corresponding Journey Pattern or alike."@en ;
                   rdfs:label "distance from start"@en .


:endOf rdfs:comment "A point of end"@en .


:endOfBlock rdfs:comment "Property to relate a Parking Point to the end of a Block"@en ;
            rdfs:label "end of block"@en .


:endingAt rdfs:comment "Property to connect an Operating Period to the related Operating Days, indicating when it ends"@en ;
          rdfs:label "ending at"@en .


:endsConnection rdfs:comment "Connection End, one end of a connection in Transmodel v6.0"@en ;
                rdfs:label "endsConnection"@en .


:endsConnectionDefault rdfs:label "endsConnectionDefault"@en .


:firstDayOffset rdfs:comment "offset of end time date from start time. In TransModel, there is only a day offset specified."@en ;
                rdfs:label "first day offset"@en .


:firstDepartureTime rdfs:comment "Time of the first departure in a Journey Frequency Group"@en ;
                    rdfs:label "first departure time"@en .


:followsDeadRunTime rdfs:label "followsDeadRunPattern"@en .


:followsJourneyPattern rdfs:label "followsJourneyPattern"@en .


:for rdfs:comment "A general property that allows associating a Stop Assignment to a Scheduled Stop Point, Quay, Boarding Position and/or Stop Place"@en ;
     rdfs:label "for"@en .


:forAlighting rdfs:comment "This property allows describing whether the stop may be used for alighting"@en ;
              rdfs:label "for Alighting"@en .


:forBoarding rdfs:comment "This property allows describing whether the stop may be used for boarding"@en ;
             rdfs:label "for Boarding"@en .


:forServicedOrganisation rdfs:comment "TODO: Add range tmorg:ServicedOrganisation"@en ,
                                      "This property connects an Organisation Day Type to a Service Organisation, indicating that such Day Type is for providing service to the corresponding Organisation"@en ;
                         rdfs:label "for serviced organisation"@en .


:headway rdfs:label "headway"@en .


:holidayType rdfs:comment "This propery sets the relationship with holiday type defined in the KOS day-type"@en ;
             rdfs:label "holiday Type"@en .


:holidayType-old rdfs:comment "TODO: In journeys/daytype-properties there is the top concept holiday-type which must be the skos:Concept range of this property"@en ,
                              "TODO: It is also a property of PropertyOfDay"@en ,
                              "This propery defines the type of holiday of the Operating Period"@en ;
                 rdfs:label "holiday Type"@en .


:inLinkSequence rdfs:comment "This property allows relating a Point in Link Sequence with the corresponding Link Sequence"@en ;
                rdfs:label "in Link Sequence"@en .


:isAvailable rdfs:comment "This property says if a Day Type Assignment is available or not"@en ;
             rdfs:label "is Available"@en .


:isDefinedBy rdfs:comment "This property relates a Template Vehicle Journey with the Rhythmical Journey Group that defines it"@en ;
             rdfs:label "is defined by"@en .


:isFlexible rdfs:comment "This property is associated to a Stop Point in Journey Pattern to represent whether it is a flexible stop or not"@en ;
            rdfs:label "is flexible"@en .


:isServiceDay rdfs:label "Property that indicates whether a Transport Service is required for an Organisation on this Day Type."@en ,
                         "is service day"@en .


:isWaitPoint rdfs:comment "Se describe si un Punto de Control es un Punto de Espera"@es ,
                          "This property allows describing whether a Timing Point is a wait point"@en ;
             rdfs:label "is Wait Point"@en .


:journeyPatternMadeUpOf rdfs:comment "A Journey Pattern is Made Up Of Stop Point In Journey Pattern"@en ,
                                     "TODO: change to madeUpOf"@en ;
                        rdfs:label "journey Pattern Made Up Of"@en .


:journeyPatternPoint rdfs:label "journeyPatternPoint"@en .


:journeyPatternRunTime rdfs:label "journeyRunTime"@en .


:lastDayOffset rdfs:comment "Time of the last departure in a Journey Frequency Group"@en ;
               rdfs:label "last departure time"@en .


:lastDepartureTime rdfs:comment "Time of the last departure in a Journey Frequency Group"@en ;
                   rdfs:label "last departure time"@en .


:layover rdfs:label "layover"@en .


:lineName rdfs:label "lineName"@en .


:lineNumber rdfs:label "lineNumber"@en .


:madeUpOf rdfs:comment "This property allows relating a Link Sequence with the set of Points in Link Sequence that make it up"@en ;
          rdfs:label "made Up Of"@en .


:madeUsing rdfs:comment "This property connects a Service Journey to the Service Facility Set that is making it possible"@en ;
           rdfs:label "made Using"@en .


:maximumHeadwayInterval rdfs:comment "Maximum headway interval for a Headway Interval of a Headway Journey Group."@en ;
                        rdfs:label "maximum headway interval"@en .


:minimumHeadwayInterval rdfs:comment "Minimum headway interval for a Headway Interval of a Headway Journey Group."@en ;
                        rdfs:label "minimum headway interval"@en .


:monitored rdfs:comment "This property defines whether the journey is monitored or not"@en ;
           rdfs:label "monitored"@en .


:on rdfs:comment "This property allows relating an entity with the entity where it appears. For instance, a Journey Pattern on (onRoute) a Route, a Route on (onLine) a Line."@en ;
    rdfs:label "on"@en .


:onLine rdfs:comment "CHECK La relación está al revés, habrá que poner otro nombre que exprese mejor la relación."@es ,
                     "This property allows relating a Route with a Line where it appears"@en ;
        rdfs:label "on Line"@en .


:onRoute rdfs:comment "CHECK La relación está al revés, habrá que poner otro nombre que exprese mejor la relación."@es ,
                      "This property allows relating a Journey Pattern with a Route where it appears"@en ;
         rdfs:label "on Route"@en .


:operatedBy rdfs:comment "This property sets the relationship between a Vehicle Journey and a Vehicle Type"@en ;
            rdfs:label "operated By"@en .


:operatingPeriod rdfs:comment "operating period"@en ,
                              "operating period assigned to a Day Type Assignment"@en .


:order rdfs:comment "Order of a Point in Link Sequence, or in a Point on Route within sequence, or in any other type of situation where the order or points are relevant"@en ;
       rdfs:label "order"@en .


:originStop rdfs:label "originStop"@en .


:overriding rdfs:comment "This property is used to specify the Passenger Stop Assignment that a Dynamic Stop Assignment overrides"@en ;
            rdfs:label "overriding"@en .


:passengerConnection rdfs:label "passengerConnection"@en .


:passesAt rdfs:comment "TODO: Check which domain and range to use"@en ,
                       "This property sets the relationship between a Point In Journey Pattern or a Service Journey and a Timetabled Passing Time"@en ;
          rdfs:label "passes at"@en .


:passingTimeTimingPoint rdfs:label "passingTimeTimingPoint" .


:prescribing rdfs:comment "This property relates a Point in Journey Pattern with a Destination Display"@en ;
             rdfs:label "prescribing"@en .


:presentedBy rdfs:comment "This property is used to connect a Line with its corresponding Presentation"@en ;
             rdfs:label "presented by"@en .


:primarilyAdvertisedWith rdfs:comment "This property relates where is primarily advertised the Journey Pattern in a Destination Display"@en ;
                         rdfs:label "primarily Advertised With"@en .


:requestStop rdfs:comment "This property allows describing whether the stop is a Request Stop"@en ;
             rdfs:label "request Stop"@en .


:routeOnLine rdfs:label "route On Line"@en .


:runBy rdfs:comment "A Line is run by an Operator"@en ;
       rdfs:label "run By"@en .


:runTimeOverrides rdfs:label "journeyRunTimeOverrides"@en .


:runsOn rdfs:comment "This property relates a Vehicle Journey with the Journey Frequency Group(s) that it belongs to"@en ;
        rdfs:label "runs On"@en .


:runtime rdfs:label "runtime"@en .


:scheduledHeadwayInterval rdfs:comment "Scheduled headway interval for a Headway Interval of a Headway Journey Group."@en ;
                          rdfs:label "scheduled headway interval"@en .


:scheduledStopPoint rdfs:label "scheduledStopPoint"@en .


:season rdfs:comment "TODO: In journeys/daytype-properties there is the skos:Concept top concept season-type which must be the range of this property"@en ,
                     "This property states the season of a Operating Period"@en ;
        rdfs:label "season"@en .


:serviceJourneyUsingPattern rdfs:comment "A Service Journey has (service Journey Pattern) a Service Journey Pattern"@en ;
                            rdfs:label "service Journey Pattern"@en .


:specifying rdfs:comment "The assignment of operational characteristics, expressed by DayType, to a particular OperatingDay within a ServiceCalendar"@en ;
            rdfs:label "specifying"@en .


:startOf rdfs:comment "A point of start"@en .


:startOfBlock rdfs:comment "Property to relate a Parking Point to the start of a Block"@en ;
              rdfs:label "start Of Block"@en .


:startTime rdfs:label "startTime"@en .


:startingAt rdfs:comment "Property to connect an Operating Period to the related Operating Days, indicating when it starts"@en ;
            rdfs:label "starting At"@en .


:stopUse rdfs:comment "This property allows describing the type of use of a stop (e.g., access, interchange only, pass through)"@en ;
         rdfs:label "stop Use"@en .


:stopsAt rdfs:label "stopsAt"@en .


:time rdfs:label "time"@en .


:timeLink rdfs:comment "Sequences of TimePoints"@en ;
          rdfs:label "timeLink"@en .


:timedFrom rdfs:comment "The relationship between a sort of Journey and a sort of Timing Point"@en ;
           rdfs:label "timedFrom"@en .


:timingLink rdfs:label "timingLinkPoint"@en .


:timingLinkInJourneyPattern rdfs:label "timingLinkInJourneyPattern"@en .


:typeOfFlexibleService rdfs:label "typeOfFlexibleService" .


:usedToDefine rdfs:comment "This property sets the relation between a Time Band or an Operating Day with a Day Type Assignment"@en ;
              rdfs:label "used To Define"@en .


:vehicleJourney rdfs:comment "A Vehicle makes (vehicleJourney) a Vehicle Journey"@en ;
                rdfs:label "vehicle Journey"@en .


:vehicleJourneyPart rdfs:label "vehicleJourneyPart"@en .


:vehicleJourneyRoute rdfs:label "vehicleJourneyRoute"@en .


:vehicleJourneyRunTimeOverrides rdfs:label "vehicleJourneyRunTimeOverrides"@en .


:vehicleJourneys rdfs:comment "The Journey of a Vehicle is a VehicleJourney"@en ;
                 rdfs:label "vehicleJourneys"@en .


:vehicleModeId rdfs:comment "This property sets the relationship between a Vehicle Mode and the type of Vehicle used defined in the kos/journeys/all-modes.ttl"@en ;
               rdfs:label "vehicle Mode ID"@en .


:vehiclePassingTime rdfs:label "vehiclePassingTime"@en .


:viaFlag rdfs:comment "This property detemines whether a Route Point is flagged as a via point"@en ;
         rdfs:label "via flag"@en .


:viewedAs rdfs:comment "This property allows connecting a Point in Link Sequence with the corresponding Point"@en ;
          rdfs:label "viewed As"@en .


:waitTime rdfs:label "waitTime"@en .


:workedOn rdfs:comment "This property sets the relationship between Vehicle Journey and Day Type."@en ;
          rdfs:label "worked On"@en .


<https://w3id.org/mobility/transmodel/commons#ComplexFeature> rdfs:comment "An aggregate of Simple Features and/or other Complex features"@en .


<https://w3id.org/mobility/transmodel/commons#SimpleFeature> rdfs:comment "An abstract representation of elementary objects related to the spatial representation of the network. POINTs (0-dimensional objects), LINKs (1-dimensional objects) and ZONEs (2-dimensional objects) may be viewed as Simple Features."@en .


<https://w3id.org/mobility/transmodel/commons#Zone> rdfs:comment "A two-dimensional PLACE within the service area of a public transport operator (administrative zone, TARIFF ZONE, ACCESS ZONE, etc.)."@en ,
                                                        "La Zona es un Lugar (Place) de dos dimensiones que ese encuentra en el área que sirve un operador de transporte público. Puede ser una zona administrativa, una zona tarifaria, una zona de acceso o algo más concreto."@es ,
                                                        "Zone"@en .


<https://w3id.org/mobility/transmodel/facilities#AccessibilityAssessment> rdfs:comment "Accessibility Assessment"@en ;
                                                                 rdfs:label "Accessibility Assessment"@en .


<https://w3id.org/mobility/transmodel/facilities#ServiceFacilitySet> rdfs:label "Service Facility Set"@en .


<https://w3id.org/mobility/transmodel/facilities#VehicleType> rdfs:comment "A classification of public transport vehicles according to the vehicle scheduling requirements in mode and capacity (e.g. standard bus, double-deck, ...)."@en ;
                                                     rdfs:label "Vehicle Type"@en .


<https://w3id.org/mobility/transmodel/facilities#journeyPatternAdvertisedFor> rdfs:comment "A Journey Pattern is advertised in a Destination Display"@en ,
                                                                                  "TODO: change to aViewOf"@en ;
                                                                     rdfs:label "journey Pattern Advertised For"@en .


<https://w3id.org/mobility/transmodel/organisations#Operator> rdfs:comment "A company providing Public Transport Services. In GTFS, this is represented as a TransitAgency"@en ,
                                                                  "The class comes from tm-organisations.owl"@en ;
                                                     rdfs:label "Operator"@es .


<https://w3id.org/mobility/transmodel/organisations#passengerJourney> rdfs:comment "A Passenger makes (journey) a Trip"@en ;
                                                             rdfs:label "passengerJourney"@en .


<https://w3id.org/mobility/transmodel/organisations#serviceJourneyServedByVehicleJourney> rdfs:comment "A Service Journey is served by Vehicle Journeys"@en ;
                                                                                 rdfs:label "service Journey Served By Vehicle Journey"@en .


<https://w3id.org/mobility/transmodel/organisations#trip> rdfs:comment "A Trip is made of ServiceJourneys"@en ;
                                                 rdfs:label "trip"@en .


###  Generated by the OWL API (version 5.1.18) https://github.com/owlcs/owlapi/
